@prefix : <http://buildvoc.co.uk/resource/> .
@prefix dc: <http://purl.org/dc/elements/1.1/> .
@prefix dcat: <http://www.w3.org/ns/dcat#> .
@prefix dct: <http://purl.org/dc/terms/> .
@prefix grddl: <http://www.w3.org/2003/g/data-view#> .
@prefix ns: <http://www.w3.org/2003/06/sw-vocab-status/ns#> .
@prefix olo: <http://purl.org/ontology/olo/core#> .
@prefix owl: <http://www.w3.org/2002/07/owl#> .
@prefix rdf: <http://www.w3.org/1999/02/22-rdf-syntax-ns#> .
@prefix rdfs: <http://www.w3.org/2000/01/rdf-schema#> .
@prefix skos: <http://www.w3.org/2004/02/skos/core#> .
@prefix skosxl: <http://www.w3.org/2008/05/skos-xl#> .
@prefix xsd: <http://www.w3.org/2001/XMLSchema#> .

<http://buildvoc.co.uk/resource/> a owl:Ontology .

:c_3da44764 skos:narrower :c_08eb88d2, :c_7abc215a, :c_c53e946f .

:c_79a3679f dc:source :c_6c82c09f .

:c_6c82c09f a skos:Concept;
  dc:publisher "Department for Communities and Local Government"@en, <http://viaf.org/viaf/143434596>;
  dc:subject """Building Regulations 2010: Approved Documents B
"""@en;
  dct:created "2019-11-30T07:32:03.382Z"^^xsd:dateTime;
  skos:broader :c_d4480e31;
  skos:definition "Presents the functional requirements for complying with fire safety in buildings other than dwellings in the building regulations. The sections cover: B1 - Means of warning and escape, B2 - Internal fire spread (linings), B3 - Internal fire spread (structure), B4 - External fire spread and B5 - Access and facilities for the fire service. Also includes Regulations 6(3), 7(2) and 38. Volume 1 deals with dwellings and blocks of flats and Volume 2 deals with all other types of building covered by the Building Regulations."@en;
  skos:inScheme :conceptScheme_751925ed;
  skos:prefLabel "fire safety - volume 2: buildings other than dwellings. 2019 edition - for use in england"@en .

:c_ca00c020 a skos:Concept;
  dc:publisher "Department for Communities and Local Government"@en, <http://viaf.org/viaf/143434596>;
  dc:subject """Building Regulations 2010: Approved Documents B
"""@en;
  dct:created "2019-11-30T07:34:38.949Z"^^xsd:dateTime;
  dct:modified "2020-10-23T17:17:44.557Z"^^xsd:dateTime;
  skos:broader :c_d4480e31;
  skos:definition "Presents the functional requirements for complying with fire safety in dwellings in the building regulations. The sections cover: B1 - Means of warning and escape, B2 - Internal fire spread (linings), B3 - Internal fire spread (structure), B4 - External fire spread and B5 - Access and facilities for the fire service. Also includes Regulations 6(3), 7(2) and 38. Approved Document B (fire safety) has been published in two volumes. Volume 1 deals with dwellings and blocks of flats and Volume 2 deals with all other types of building covered by the Building Regulations."@en;
  skos:example <https://assets.publishing.service.gov.uk/government/uploads/system/uploads/attachment_data/file/832631/Approved_Document_B__fire_safety__volume_1_-_2019_edition.pdf>;
  skos:inScheme :conceptScheme_751925ed;
  skos:prefLabel "fire safety - volume 1: dwellings. 2019 edition - for use in england"@en .

:c_6d2c7baa a skos:Concept;
  dc:publisher """Welsh Government
"""@en;
  dc:subject """Building Regulations 2010: Approved Documents B2
"""@en;
  dct:created "2019-11-30T07:23:25.579Z"^^xsd:dateTime;
  rdfs:seeAlso "https://gov.wales/sites/default/files/publications/2019-05/building-regulations-guidance-part-b-fire-safety-volume-2-buildings-other-than-dwellinghouses.pdf"@en;
  skos:broader :c_d4480e31;
  skos:definition "Provides practical guidance for complying with building regulations on matters relating to materials and workmanship with examples and solutions for different building situations. Approved document B2 deals with fire safety in buildings other than dwellinghouses and covers: Sections B1 - Means of warning and escape, B2 - Internal fire spread (linings), B3 - Internal fire spread (structure), B4 - External fire spread and B5 - Access and facilities for the fire and rescue service. Approved Document B (fire safety) has been published in two volumes. Volume 1 deals with dwellinghouses and Volume 2 deals with all other types of building covered by the Building Regulations."@en;
  skos:inScheme :conceptScheme_751925ed .

:c_7ffd0e94 a skos:Concept;
  dc:publisher """Welsh Government
"""@en;
  dct:created "2019-11-30T06:49:58.405Z"^^xsd:dateTime;
  dct:subject """Building Regulations 2010: Approved Documents B1
"""@en;
  rdfs:seeAlso "<https://gov.wales/sites/default/files/publications/2019-05/building-regulations-guidance-part-b-fire-safety-volume-1-dwellinghouses.pdf>"@en;
  skos:broader :c_d4480e31;
  skos:definition "Provides practical guidance for complying with building regulations on matters relating to materials and workmanship with examples and solutions for different building situations. Approved document B1 deals with fire safety in dwellinghouses and covers: Sections B1 - Means of warning and escape, B2 - Internal fire spread (linings), B3 - Internal fire spread (structure), B4 - External fire spread and B5 - Access and facilities for the fire and rescue service. Approved Document B (fire safety) has been published in two volumes. Volume 1 deals with dwellinghouses and Volume 2 deals with all other types of building covered by the Building Regulations. Where very large (over 18m in height) or unusual dwellinghouses are proposed some of the guidance in Volume 2 may be needed to supplement that given by Volume 1."@en;
  skos:inScheme :conceptScheme_751925ed .

:xl_en_d2f47531 dct:modified "2019-11-30T07:27:51.385Z"^^xsd:dateTime;
  skosxl:literalForm "building regulations guidance"@en .

:c_f9b32acf a skos:Concept;
  dct:created "2018-03-28T19:03:52.286Z"^^xsd:dateTime;
  skos:closeMatch <http://eurovoc.europa.eu/3134>;
  skos:inScheme :conceptScheme_751925ed;
  skos:narrower :c_00d0e0e8, :c_0e0d001c, :c_10c7fd62, :c_1abb8332, :c_2658862b, :c_3518fece,
    :c_5b4555d8, :c_64b1d307, :c_6b24d6e2, :c_86cfaae6, :c_c83014a4, :c_e3cebf52;
  skos:prefLabel "building regulation"@en;
  skos:topConceptOf :conceptScheme_751925ed .

:c_132d79ca dc:source :c_6c82c09f, :c_ca00c020 .

:c_727adfdb dc:source :c_ca00c020 .

:c_5724a233 dc:source :c_ca00c020;
  dct:modified "2019-12-21T07:22:01.689Z"^^xsd:dateTime .

:c_b44f46e0 dc:source :c_ca00c020;
  skos:prefLabel "specified attachment"@en .

:c_a4eaf123 dc:source :c_ca00c020;
  skos:definition "(fire-protecting) A ceiling suspended below a floor that adds to the fire resistance of the floor."@en .

:c_502a871c skos:changeNote "changed from guidance documents "@en;
  skos:prefLabel "building regulations guidance"@en .

:c_228ee3b0 dc:publisher """HM Government
"""@en;
  dct:created "2019-11-30T11:58:19.854Z"^^xsd:dateTime;
  skos:definition "A room that the only escape route from an inner room passes through."@en;
  skos:prefLabel "access room"@en .

:c_da6168d8 dct:created "2019-12-12T20:41:23.654Z"^^xsd:dateTime;
  skos:broader :c_13911a49;
  skos:prefLabel "dwelling"@en-GB .

:c_7fc5469b skos:definition "A space enclosed by elements of a building (including a suspended ceiling) or contained within an element, but that is not a room, cupboard, circulation space, protected shaft, or space within a flue, chute, duct, pipe or conduit."@en;
  skos:inScheme :conceptScheme_751925ed;
  skos:prefLabel "cavity"@en .

:c_6284471b a skos:Concept .

:xl_en_42f4c7a1 a skosxl:Label;
  skosxl:literalForm "air"@en .

:c_56fef4b5 dc:source :c_6c82c09f;
  skos:inScheme :conceptScheme_751925ed .

:c_bed063fd skos:inScheme :conceptScheme_751925ed .

:xl_en_a3365120 skosxl:literalForm "notices, plans and certificates"@en .

:c_64b1d307 rdfs:isDefinedBy <http://www.legislation.gov.uk/uksi/2010/2214/part/7/made> .

:c_f5536b7d dct:modified "2019-12-13T23:33:59.284Z"^^xsd:dateTime .

:c_83464c52 dct:created "2019-12-12T20:50:45.745Z"^^xsd:dateTime .

:c_c83014a4 skos:prefLabel "control of building work"@en .

:c_33c0e1b5 dc:source :c_ca00c020;
  skos:inScheme :conceptScheme_751925ed .

:c_9b7f9eb7 dct:modified "2019-12-13T22:36:18.618Z"^^xsd:dateTime .

:c_4a90e0e1 dct:created "2019-12-13T23:19:04.145Z"^^xsd:dateTime;
  skos:definition "A building or part of a building, comprising one or more rooms, spaces or storeys, that is constructed to prevent the spread of fire to or from another part of the same building or an adjoining building."@en .

:c_b2cab8d9 skos:inScheme :conceptScheme_751925ed .

:c_4553c077 dct:created "2018-07-22T14:24:33.455Z"^^xsd:dateTime .

:c_feba40b2 dct:modified "2020-10-23T17:04:12.702Z"^^xsd:dateTime .

:c_e7e6b110 dc:source :c_ca00c020 .

:rdf:isPartOf dct:created "2018-03-29T13:50:40.287Z"^^xsd:dateTime .

:c_13911a49 skos:narrower :c_056e5a0a, :c_10ea4ecc, :c_4cb80404, :c_7d862abe, :c_858351ef,
    :c_a4eaf123, :c_b3f65603 .

:skos:narrower a owl:Class;
  rdfs:subClassOf owl:Thing .

:c_8258611b dc:source :c_6c82c09f .

:xl_en_2de5ebbe a skosxl:Label .

:conceptScheme_751925ed a skos:ConceptScheme;
  dc:contributor "British Standards Institution"@en;
  dc:creator "P Stacey"@en;
  dct:created "2018-04-07T19:41:18.052Z"^^xsd:dateTime;
  dct:license <http://creativecommons.org/licenses/by/4.0/>;
  dct:modified "2019-11-30T10:41:58.827Z"^^xsd:dateTime;
  skos:prefLabel "Drawing information"@en, "General"@en, "Information and communication"@en,
    "Labour"@en, "Legislation"@en, "Materials"@en, "Phases of development (construction)"@en .

:c_00d0e0e8 a skos:Concept;
  dct:created "2018-03-29T10:23:40.952Z"^^xsd:dateTime;
  rdfs:isDefinedBy <http://www.legislation.gov.uk/uksi/2010/2214/part/5/made>;
  skos:broader :c_f9b32acf;
  skos:inScheme :conceptScheme_751925ed;
  skos:notation "part 05";
  skos:prefLabel "self-certification schemes"@en;
  skosxl:prefLabel :xl_en_6f26398b .

:c_6c82c09f dct:modified "2020-10-23T17:18:08.995Z"^^xsd:dateTime .

:xl_en_6f26398b a skosxl:Label;
  dct:modified "2018-07-20T19:15:55.436Z"^^xsd:dateTime;
  skosxl:literalForm "self-certification schemes"@en .

:xl_en_91bd8550 skosxl:literalForm "attma"@en .

:c_38ba0f99 dct:created "2019-12-15T08:42:47.378Z"^^xsd:dateTime;
  skos:broader :c_13911a49 .

:xl_en_96c8608e a skosxl:Label;
  skosxl:literalForm "loi"@en .

:skosCollection_50d4bd2e skos:member :c_08eb88d2 .

:c_3e5063e6 skos:definition "A storey with a floor that, at some point, is more than 1200mm below the highest level of ground beside the outside walls. (However, see Appendix B, paragraph B26c, for situations where the storey is considered to be a basement only because of a sloping site.)"@en;
  skos:inScheme :conceptScheme_751925ed .

:c_34f295d5 rdfs:isDefinedBy <http://www.legislation.gov.uk/uksi/2010/2214/regulation/2>;
  skos:prefLabel "dwelling"@en .

:xl_en_45e6bbda a skosxl:Label .

:c_b3f65603 a skos:Concept;
  dct:modified "2020-10-26T07:36:45.280Z"^^xsd:dateTime;
  skos:definition "A flat that is a workplace for people who live there, its occupants, and for people who do not live on the premises."@en;
  skos:inScheme :conceptScheme_751925ed;
  skos:prefLabel "live/work unit"@en .

:c_10ea4ecc a skos:Concept;
  dct:created "2019-12-15T08:28:48.957Z"^^xsd:dateTime;
  dct:modified "2019-12-15T08:34:09.621Z"^^xsd:dateTime;
  skos:broader :c_13911a49;
  skos:definition "Structural means that provide one or more safe routes for people to go, during a fire, from any point in the building to a place of safety."@en;
  skos:inScheme :conceptScheme_751925ed;
  skos:prefLabel "means of escape"@en .

:c_056e5a0a dc:source :c_6c82c09f;
  dct:created "2019-12-15T08:25:31.904Z"^^xsd:dateTime;
  dct:modified "2019-12-15T08:34:09.992Z"^^xsd:dateTime;
  skos:note "Room from which escape is possible only by passing through another room (the access room)."@en .

:c_4cb80404 a skos:Concept;
  dc:source :c_6c82c09f, :c_ca00c020;
  dct:created "2019-12-15T08:34:53.951Z"^^xsd:dateTime;
  dct:modified "2019-12-15T08:38:34.953Z"^^xsd:dateTime;
  skos:broader :c_13911a49;
  skos:definition "The internal arrangement of a building in which more than one storey or level is contained in one undivided volume, e.g. split-level floors. For the purposes of this document there is a distinction between open spatial planning and an atrium space."@en;
  skos:inScheme :conceptScheme_751925ed;
  skos:prefLabel "open spatial planning"@en .

:c_f4139893 a skos:Concept;
  dc:source :c_6c82c09f, :c_ca00c020;
  dct:created "2019-12-21T06:28:24.441Z"^^xsd:dateTime;
  skos:broader :c_13911a49;
  skos:definition "A place of education for children between 2 and 19 years old. The term includes nursery schools, primary schools and secondary schools as defined in the Education Act 1996."@en;
  skos:inScheme :conceptScheme_751925ed;
  skos:prefLabel "school"@en .

:c_1f1f7725 a skos:Concept;
  dc:source :c_6c82c09f, :c_ca00c020;
  dct:created "2019-12-15T08:30:42.736Z"^^xsd:dateTime;
  dct:modified "2019-12-15T08:34:09.545Z"^^xsd:dateTime;
  skos:broader :c_13911a49;
  skos:definition """<ul><li>Width of a doorway, cubic capacity, area, height of a building and number of storeys are measured as shown in Appendix D, Diagrams D1 to D6.
<li>Occupant number, travel distance, escape route and stairs are measured as described in Appendix D, paragraphs D1 to D4.</ul>"""@en;
  skos:inScheme :conceptScheme_751925ed;
  skos:prefLabel "measurement"@en .

:c_35d3a535 a skos:Concept;
  dct:modified "2019-12-15T08:46:59.170Z"^^xsd:dateTime;
  skos:broader :c_13911a49;
  skos:definition "Includes pipe fittings and accessories. The definition of ‘pipe’ excludes a flue pipe and a pipe used for ventilating purposes, other than a ventilating pipe for an above-ground drainage system."@en;
  skos:inScheme :conceptScheme_751925ed;
  skos:prefLabel "pipe"@en .

:c_ee10273a skos:inScheme :conceptScheme_751925ed .

:c_7c12f560 dc:source :c_ca00c020;
  skos:definition "A stair that leads to a final exit to a place of safety and that is adequately enclosed with fire resisting construction. Included in the definition is any exit passageway between the foot of the stair and the final exit."@en .

:c_cc61a0f4 dct:modified "2019-12-21T06:27:11.448Z"^^xsd:dateTime .

:c_d5c15327 dct:modified "2019-12-15T08:47:29.723Z"^^xsd:dateTime;
  skos:definition "An electrical circuit that is protected against fire."@en .

:c_d32d8045 a skos:Concept;
  skos:prefLabel "single storey"@en .

:c_46be855e skos:broader :c_13911a49 .

:c_7d862abe a skos:Concept;
  dc:source :c_ca00c020;
  dct:created "2019-12-21T06:32:03.423Z"^^xsd:dateTime;
  skos:broader :c_13911a49;
  skos:definition "A device that closes a door, when open at any angle, against a door frame."@en;
  skos:inScheme :conceptScheme_751925ed;
  skos:prefLabel "self-closing device"@en .

:c_132d79ca skos:inScheme :conceptScheme_751925ed;
  skos:prefLabel "site"@en .

:c_7b85eda3 dct:modified "2019-12-21T06:27:12.227Z"^^xsd:dateTime;
  skos:definition "A corridor or lobby that is adequately protected from fire in adjoining areas by fire resisting construction."@en .

:c_b6083e42 dc:source :c_6c82c09f .

:c_b44f46e0 skos:definition """Includes any of the following. 
<ul><li>A balcony attached to an external wall.
<li>A device for reducing heat gain within a building by deflecting sunlight which is attached to an external wall. </ul>
A solar panel attached to an external wall."""@en .

:c_cb3d4c10 a skos:Concept .

:c_727adfdb a skos:Concept;
  skos:prefLabel "storey exit"@en .

:c_13543964 dct:modified "2019-12-21T06:27:12.116Z"^^xsd:dateTime .

:c_a4eaf123 dct:modified "2019-12-21T07:22:01.421Z"^^xsd:dateTime .

:c_c83014a4 skosxl:prefLabel :xl_en_786a7815 .

:xl_en_310fdd79 a skosxl:Label;
  skosxl:literalForm "sap"@en .

:c_c02d4d7d dct:modified "2019-12-28T07:15:27.051Z"^^xsd:dateTime;
  rdfs:isDefinedBy <http://www.legislation.gov.uk/uksi/2010/2214/regulation/2> .

:xl_en_76bd2153 a skosxl:Label;
  skosxl:literalForm """2.1.1
"""@en .

:c_b975b2d2 dc:source :c_6c82c09f .

:c_da6168d8 rdfs:isDefinedBy <http://www.legislation.gov.uk/uksi/2010/2214/regulation/2> .

:xl_en_b9ef8f0c a skosxl:Label;
  skosxl:literalForm "part r - physical infrastructure for high speed electronic communications networks"@en .

:c_7400b440 a skos:Concept;
  skos:prefLabel "purpose group"@en .

:c_06f29df7 a skos:Concept;
  dct:created "2018-03-28T19:12:00.921Z"^^xsd:dateTime;
  skos:inScheme :conceptScheme_751925ed;
  skos:prefLabel "regulation 7 - materials and workmanship"@en;
  skosxl:prefLabel :xl_en_f65b5e23 .

:c_502a871c a skos:Concept;
  dct:created "2018-03-28T19:04:56.970Z"^^xsd:dateTime;
  skos:inScheme :conceptScheme_751925ed;
  skos:topConceptOf :conceptScheme_751925ed;
  skosxl:prefLabel :xl_en_d2f47531 .

:c_f851b292 skos:prefLabel "habitable room"@en .

:c_86cfaae6 a skos:Concept;
  dct:created "2020-10-19T16:31:48.703Z"^^xsd:dateTime;
  skos:broader :c_f9b32acf;
  skos:inScheme :conceptScheme_751925ed;
  skos:prefLabel "building regulations 2010"@en .

:c_d10595f3 skos:inScheme :conceptScheme_751925ed .

:c_90aedbdc skos:narrower :c_e47ea7fb .

:c_76c8b363 skos:inScheme :conceptScheme_751925ed;
  skos:prefLabel "extract ventilation"@en .

:c_59a3ae21 skos:narrower :c_4d4c50dd, :c_eeea044b, :c_f851b292 .

:c_4fe84b3b skos:inScheme :conceptScheme_751925ed .

:c_feba40b2 dct:created "2020-10-23T17:02:27.325Z"^^xsd:dateTime .

:xl_en_f65b5e23 a skosxl:Label;
  skosxl:literalForm "regulation 7 - materials and workmanship"@en .

:c_13911a49 skos:narrower :c_1f1f7725, :c_da6168d8, :c_f4139893 .

:xl_en_45e6bbda skosxl:literalForm "construct spec"@en .

:c_f70bb786 dct:modified "2019-12-12T21:17:46.146Z"^^xsd:dateTime .

:c_9b7f9eb7 skos:prefLabel "firefighting lift"@en .

:xl_en_ca2d0e57 a skosxl:Label .

:c_858351ef a skos:Concept;
  dc:source :c_6c82c09f, :c_ca00c020;
  dct:modified "2019-12-15T08:34:09.479Z"^^xsd:dateTime;
  skos:definition "A boundary presumed to exist between two buildings on the same site."@en;
  skos:prefLabel "notional boundary"@en .

:c_10ea4ecc dc:source :c_ca00c020 .

:c_b3f65603 dc:source :c_ca00c020 .

:c_056e5a0a dc:source :c_ca00c020 .

:c_0e0d001c a skos:Concept;
  dct:created "2018-03-29T10:47:59.314Z"^^xsd:dateTime;
  dct:modified "2018-03-29T10:54:28.435Z"^^xsd:dateTime;
  skos:broader :c_f9b32acf;
  skos:definition "This Order reforms the law relating to fire safety in non-domestic premises. It replaces fire certification under the Fire Precautions Act 1971 with a general duty to ensure, so far as is reasonably practicable, the safety of employees, a general duty, in relation to non-employees to take such fire precautions as may reasonably be required in the circumstances to ensure that premises are safe and a duty to carry out a risk assessment."@en;
  skos:inScheme :conceptScheme_751925ed;
  skos:prefLabel "regulatory reform (fire safety) order 2005"@en;
  skos:related :c_a452ce73, :c_d4480e31;
  skosxl:prefLabel :xl_en_a359d04b .

:c_a452ce73 a skos:Concept;
  dc:source "Approved Document B (fire safety) volume 2: buildings other than dwellinghouses (2006 edition incorporating the 2010 and 2013 amendments)"@en;
  dct:created "2018-03-29T10:24:24.786Z"^^xsd:dateTime;
  dct:modified "2020-10-23T16:52:17.707Z"^^xsd:dateTime;
  skos:broader :c_10c7fd62;
  skos:definition "Regulation 16B requires that where building work is carried out which affects fire safety, and where the building affected will be covered by the Regulatory Reform (Fire Safety) Order 2005, the person carrying out the work must provide sufficient information for persons to operate and maintain the building in reasonable safety. This information will assist the eventual owner/ occupier/employer to meet their statutory duties under the Regulatory Reform (Fire Safety) Order."@en;
  skos:editorialNote "<ul>f. Details of all active fire safety measures, including: <ul><li>Sprinkler system(s) design, including isolating valves and control equipment; and <li>Smoke-control system(s) (or HVAC system with a smoke-control function) design, including mode of operation and control systems. <li>g. Any high-risk areas (e.g. heating machinery) and particular hazards, <li>h. As-built plans of the building showing the locations of the above. <li>i. Specifications of any fire safety equipment provided, including operational details, operators manuals, software, system zoning and routine inspection, testing and maintenance schedules. Records of any acceptance or commissioning tests. <li>j. Any provision incorporated into the building to facilitate the evacuation of disabled people. <li>k. Any other details appropriate for the specific building. </ul>"@en;
  skos:example <https://www.gov.uk/government/publications/fire-safety-approved-document-b>;
  skos:inScheme :conceptScheme_751925ed;
  skos:notation "38";
  skos:prefLabel "fire safety information (TBA)"@en;
  skosxl:prefLabel :xl_en_dde7f619 .

:c_d4480e31 a skos:Concept;
  dc:source "Building a Safer Future – Independent Review of Building Regulations and Fire Safety: Final Report"@en;
  dct:created "2018-03-28T19:09:47.835Z"^^xsd:dateTime;
  rdfs:seeAlso <http://eprints.bimcoordinator.co.uk/id/eprint/11>;
  skos:broader :c_502a871c;
  skos:definition "Guidance on ways to comply with the fire safety requirements in Part B of Schedule 1 to the Building Regulations 2010"@en;
  skos:inScheme :conceptScheme_751925ed;
  skos:prefLabel "part b - fire safety"@en .

:c_3da44764 skos:narrower :c_0af8118b, :c_58bdb729 .

:skosCollection_50d4bd2e dct:modified "2020-10-27T17:17:05.529Z"^^xsd:dateTime;
  skos:member :c_2689a172, :c_9243074f, :c_aae4241b, :c_cf85f340 .

:c_c07e16c5 skos:inScheme :conceptScheme_751925ed .

:xl_en_a359d04b a skosxl:Label;
  skosxl:literalForm "regulatory reform (fire safety) order 2005"@en .

:c_6b24d6e2 a skos:Concept;
  dct:created "2018-03-29T10:24:41.329Z"^^xsd:dateTime;
  rdfs:isDefinedBy <http://www.legislation.gov.uk/uksi/2010/2214/part/9/made>;
  skos:broader :c_f9b32acf;
  skos:inScheme :conceptScheme_751925ed;
  skos:notation "part 09"@en;
  skos:prefLabel "testing and commissioning (building regulation)"@en;
  skosxl:prefLabel :xl_en_e99200e0 .

:skosxl:hiddenLabel a owl:Class .

:xl_en_453bc190 a skosxl:Label;
  skosxl:literalForm """2.1.6
"""@en .

:xl_en_913b3693 a skosxl:Label .

:c_75ffd205 dct:created "2018-04-21T15:09:31.302Z"^^xsd:dateTime .

:xl_en_e99200e0 a skosxl:Label;
  skosxl:literalForm "testing and commissioning (building regulation)"@en .

:c_46be855e dct:created "2019-12-21T06:13:29.946Z"^^xsd:dateTime .

:xl_en_1445c137 a skosxl:Label;
  skosxl:literalForm "air tightness testing and measurement association certificate"@en .

:c_a4eaf123 dc:source :c_6c82c09f .

:c_79a3679f dct:modified "2019-12-13T23:33:59.692Z"^^xsd:dateTime .

:xl_en_1b847882 skosxl:literalForm "legal"@en .

:c_228ee3b0 skos:broader :c_13911a49;
  skos:inScheme :conceptScheme_751925ed .

:xl_en_80102184 skosxl:literalForm """2.1.10
"""@en .

:xl_en_ecb8813d skosxl:literalForm "health"@en .

:c_83464c52 dc:source :c_6c82c09f;
  skos:prefLabel "travel distance"@en-GB .

:c_58df2af5 skos:broader :c_86cfaae6;
  skos:note "Requirements Regulations 4 and 6"@en .

:skos:narrower dct:created "2018-03-29T09:44:53.326Z"^^xsd:dateTime .

:c_61f82d61 a skos:Concept;
  dc:source :c_6c82c09f, :c_ca00c020 .

:c_533afc9b dct:created "2018-07-20T21:00:25.877Z"^^xsd:dateTime .

:c_132d79ca dct:created "2019-12-21T06:56:02.209Z"^^xsd:dateTime;
  skos:broader :c_13911a49 .

:c_10030a9a skos:broader :c_13911a49;
  skos:prefLabel "boundary"@en-GB .

:c_10c7fd62 a skos:Concept;
  dct:created "2018-03-29T10:24:08.502Z"^^xsd:dateTime;
  dct:modified "2020-10-28T15:11:08.871Z"^^xsd:dateTime;
  rdfs:isDefinedBy <http://www.legislation.gov.uk/uksi/2010/2214/part/8/made>;
  skos:broader :c_f9b32acf;
  skos:inScheme :conceptScheme_751925ed;
  skos:notation "part 08"@en;
  skos:prefLabel "information to be provided by the person carrying out work"@en .

:c_727adfdb dc:source :c_6c82c09f;
  skos:broader :c_13911a49;
  skos:inScheme :conceptScheme_751925ed .

:c_04c52352 dc:source :c_6c82c09f .

:c_7d862abe dc:source :c_6c82c09f .

:c_c1a78f4b dc:source :c_6c82c09f .

:c_40560ccd a skos:Concept;
  dct:created "2019-12-21T06:48:21.375Z"^^xsd:dateTime;
  skos:broader :c_13911a49;
  skos:inScheme :conceptScheme_751925ed;
  skos:prefLabel "sheltered housing"@en .

:c_35d3a535 dct:created "2019-12-15T08:39:34.693Z"^^xsd:dateTime .

:c_13911a49 a skos:Concept;
  dct:created "2019-11-30T11:56:26.982Z"^^xsd:dateTime;
  rdfs:isDefinedBy :c_f9b32acf;
  skos:narrower :c_132d79ca, :c_34f295d5, :c_35d3a535, :c_38ba0f99, :c_3e5063e6, :c_40560ccd,
    :c_46be855e;
  skos:note "NOTE: Except for the items marked * (which are from the Building Regulations 2010), these definitions apply only to Approved Document B.<p>NOTE: The terms defined below are key terms used in this document only. Refer to BS 4422 for further guidance on the definitions of common terms used in the fire safety industry which are not listed below.</p>"@en .

:c_13543964 a skos:Concept;
  skos:inScheme :conceptScheme_751925ed;
  skos:prefLabel "protected entrance hall/landing"@en .

:xl_en_dde7f619 a skosxl:Label;
  dct:modified "2020-10-23T16:52:30.383Z"^^xsd:dateTime;
  skosxl:literalForm "fire safety information (TBA)"@en .

:c_3cae7829 dct:modified "2019-12-14T08:48:46.738Z"^^xsd:dateTime .

:xl_en_0049082b a skosxl:Label;
  skosxl:literalForm "bass"@en .

:c_b975b2d2 a skos:Concept;
  dct:created "2019-12-21T07:15:28.445Z"^^xsd:dateTime;
  skos:broader :c_13911a49;
  skos:inScheme :conceptScheme_751925ed;
  skos:prefLabel "thermoplastic material"@en .

:c_cb86c2ff dc:source :c_ca00c020 .

:rdf:isPartOf a rdf:Property .

:c_5ef03467 dc:source :c_ca00c020 .

:xl_en_a7c1ef29 a skosxl:Label .

:skosCollection_42952ecf dct:created "2018-08-11T08:35:23.556Z"^^xsd:dateTime .

:c_9a0f5e20 dc:source :c_6c82c09f;
  dct:modified "2019-12-14T08:48:46.832Z"^^xsd:dateTime .

:c_88af4873 dc:source :c_6c82c09f;
  skos:notation "B2"@en .

:c_c02d4d7d a skos:Concept;
  skos:inScheme :conceptScheme_751925ed;
  skos:prefLabel "building"@en .

:c_5724a233 dc:source :c_6c82c09f .

:c_56fef4b5 skos:broader :c_13911a49 .

:xl_en_6cb57c20 a skosxl:Label;
  skosxl:literalForm """2.1.3
"""@en .

:xl_en_91bd8550 a skosxl:Label .

:c_e162c613 dct:created "2018-05-26T11:01:47.267Z"^^xsd:dateTime .

:xl_en_c14ad7c7 a skosxl:Label;
  skosxl:literalForm "part c - site preparation and resistance to contaminates and moisture"@en .

:c_da6168d8 a skos:Concept;
  dct:modified "2020-10-28T15:18:43.693Z"^^xsd:dateTime;
  skos:definition "Includes a dwellinghouse and a flat."@en;
  skos:inScheme :conceptScheme_751925ed .

:c_9b7f9eb7 dc:source :c_ca00c020;
  skos:notation "B1"@en .

:c_b2cab8d9 dc:source :c_ca00c020;
  skos:definition "The maximum aggregate plan perimeter, found by vertical projection onto a horizontal plane. (See Section 15 of Approved Document B Volume 2.)"@en .

:c_a965ecce dc:source :c_6c82c09f;
  skos:notation "B2"@en;
  skos:prefLabel "perimeter (of a building)"@en-GB .

:c_b0f3b4fb a skos:Concept;
  dc:source :c_ca00c020;
  skos:notation "B1"@en .

:c_34f295d5 a skos:Concept;
  dct:created "2019-12-12T20:41:01.583Z"^^xsd:dateTime;
  dct:modified "2019-12-28T07:19:31.525Z"^^xsd:dateTime;
  skos:broader :c_13911a49;
  skos:inScheme :conceptScheme_751925ed;
  skos:notation "*B1"@en .

:c_3518fece a skos:Concept;
  dct:modified "2019-12-28T07:35:43.826Z"^^xsd:dateTime;
  rdfs:isDefinedBy <http://www.legislation.gov.uk/uksi/2010/2214/part/1/made>;
  skos:notation "part 01"@en .

:c_858351ef dct:created "2019-12-15T08:31:59.287Z"^^xsd:dateTime;
  skos:broader :c_13911a49;
  skos:inScheme :conceptScheme_751925ed .

:xl_en_44ca1675 a skosxl:Label .

:xl_en_3c41ea90 a skosxl:Label;
  skosxl:literalForm "lod"@en .

:xl_en_cff63d0f a skosxl:Label .

:c_6284471b dc:source :c_6c82c09f;
  skos:prefLabel "automatic release mechanism"@en .

:c_8258611b dc:source :c_ca00c020;
  skos:prefLabel "atrium (plural atria)"@en .

:xl_en_fd21eb9e a skosxl:Label;
  skosxl:literalForm """2.1.2
"""@en .

:c_3e5063e6 skos:broader :c_13911a49 .

:c_1abb8332 a skos:Concept;
  dct:created "2018-03-29T10:23:17.065Z"^^xsd:dateTime;
  dct:modified "2019-12-22T07:41:06.528Z"^^xsd:dateTime;
  rdfs:isDefinedBy <http://www.legislation.gov.uk/uksi/2010/2214/part/4/made>;
  skos:broader :c_f9b32acf;
  skos:inScheme :conceptScheme_751925ed;
  skos:notation "part 04";
  skos:prefLabel "supervision of building work otherwise than by local authorities"@en;
  skosxl:prefLabel :xl_en_d0cd7dda .

:c_6d2c7baa skos:prefLabel "fire safety - volume 2 - buildings other than dwellinghouses (2006 edition incorporating 2010, 2013 and 2016 amendments) (for use in wales)"@en .

:xl_en_f2eee9b5 skosxl:literalForm "cde"@en .

:c_33c0e1b5 a skos:Concept .

:xl_en_0a7cb84d a skosxl:Label;
  skosxl:literalForm "midp"@en .

:c_7ffd0e94 dct:modified "2020-10-23T17:17:29.027Z"^^xsd:dateTime;
  skos:prefLabel "fire safety - volume 1 dwellinghouses (2006 edition incorporating 2010 and 2016 amendments) (for use in wales)"@en .

:c_bed063fd dc:source :c_ca00c020 .

:c_38ba0f99 dct:modified "2019-12-15T08:46:58.872Z"^^xsd:dateTime;
  skos:definition "(also called an access or raised floor) A floor that is supported by a structural floor, but with an intervening cavity to house services."@en .

:conceptScheme_751925ed dc:description "Scope of controlled vocabulary to follow"@en .

:c_14b52896 dc:source :c_6c82c09f, :c_ca00c020;
  dct:modified "2019-12-14T08:48:46.962Z"^^xsd:dateTime .

:xl_en_1b847882 a skosxl:Label .

:c_7804ad6c dc:source :c_6c82c09f;
  dct:modified "2019-12-14T08:48:47.639Z"^^xsd:dateTime .

:c_59a3ae21 skos:narrower :c_830012c2 .

:c_d5c15327 a skos:Concept .

:c_6b24d6e2 dct:modified "2019-12-28T07:37:20.419Z"^^xsd:dateTime .

:xl_en_d1eea4cb a skosxl:Label;
  skosxl:literalForm "cml"@en .

:xl_en_7274bb0f a skosxl:Label;
  skosxl:literalForm "pim"@en .

:xl_en_24febe8b a skosxl:Label;
  skosxl:literalForm """2.1.9
"""@en .

:c_7400b440 skos:inScheme :conceptScheme_751925ed .

:c_1a6e1e92 a skos:Concept;
  dct:created "2018-03-28T19:10:14.402Z"^^xsd:dateTime;
  skos:inScheme :conceptScheme_751925ed;
  skos:prefLabel "part e - resistance to the passage of sound"@en;
  skosxl:prefLabel :xl_en_1fd9fca8 .

:c_8cba3c82 dct:modified "2020-10-23T17:08:13.914Z"^^xsd:dateTime;
  skos:broader :c_502a871c .

:xl_en_1fd9fca8 a skosxl:Label;
  skosxl:literalForm "part e - resistance to the passage of sound"@en .

:xl_en_d0cd7dda a skosxl:Label;
  dct:modified "2018-07-20T19:10:38.844Z"^^xsd:dateTime;
  skosxl:literalForm "supervision of building work otherwise than by local authorities"@en .

:c_f4139893 dct:modified "2019-12-28T06:54:53.684Z"^^xsd:dateTime;
  rdfs:isDefinedBy <http://www.legislation.gov.uk/ukpga/1996/56/section/4>;
  rdfs:seeAlso <http://www.legislation.gov.uk/ukpga/1996/56/section/4> .

:xl_en_1ec12f25 a skosxl:Label .

:c_1b060096 a skos:Concept;
  dct:created "2018-03-28T19:09:39.123Z"^^xsd:dateTime;
  dct:modified "2020-10-23T17:06:18.179Z"^^xsd:dateTime;
  skos:broader :c_502a871c;
  skos:inScheme :conceptScheme_751925ed;
  skos:prefLabel "part a - structure"@en;
  skosxl:prefLabel :xl_en_f9e89b8d .

:xl_en_f9e89b8d a skosxl:Label;
  skosxl:literalForm "part a - structure"@en .

:c_9e4931f7 a skos:Concept;
  dct:created "2019-12-13T23:09:23.909Z"^^xsd:dateTime;
  skos:broader :c_13911a49;
  skos:inScheme :conceptScheme_751925ed;
  skos:prefLabel "cavity barrier"@en .

:c_13911a49 skos:narrower :c_33c0e1b5, :c_56fef4b5, :c_83464c52, :c_9b7f9eb7, :c_9e4931f7,
    :c_f5536b7d, :c_f70bb786 .

:c_c02d4d7d skos:notation "*"@en .

:c_83464c52 a skos:Concept;
  dct:modified "2020-10-28T15:13:23.569Z"^^xsd:dateTime;
  skos:broader :c_13911a49;
  skos:definition "(unless otherwise specified, e.g. as in the case of flats) The distance that a person would travel from any point within the floor area to the nearest storey exit, determined by the layout of walls, partitions and fittings."@en;
  skos:notation "B2"@en .

<http://buildvoc.co.uk/resource/> owl:imports <http://www.w3.org/ns/dcat> .

:xl_en_a7c1ef29 dct:modified "2018-07-20T19:12:10.682Z"^^xsd:dateTime;
  skosxl:literalForm "water efficiency"@en .

:c_52aaa84e dct:created "2018-07-24T17:09:26.522Z"^^xsd:dateTime .

:c_277602e6 dct:created "2018-08-11T09:08:09.653Z"^^xsd:dateTime .

:c_4a90e0e1 dc:source :c_ca00c020 .

:c_7d862abe skos:note "NOTE: If the door is in a cavity barrier, rising butt hinges (which are different from the self-closing device mentioned above) are acceptable."@en .

:xl_en_ca2d0e57 skosxl:literalForm "bep"@en .

:xl_en_8715993d a skosxl:Label .

:c_5ef03467 dc:source :c_6c82c09f;
  dct:modified "2019-12-13T23:33:58.622Z"^^xsd:dateTime;
  skos:definition "One of two or more exits, each of which is separate from the other."@en .

:c_04c52352 a skos:Concept;
  dct:created "2019-12-21T06:34:39.568Z"^^xsd:dateTime;
  skos:broader :c_13911a49;
  skos:inScheme :conceptScheme_751925ed;
  skos:prefLabel "separated part"@en-GB .

:c_64b1d307 a skos:Concept;
  skos:broader :c_f9b32acf;
  skos:inScheme :conceptScheme_751925ed;
  skos:notation "part 07" .

:c_dc99fe05 dct:created "2018-04-07T19:42:55.911Z"^^xsd:dateTime .

:c_b44f46e0 a skos:Concept;
  dc:source :c_6c82c09f;
  dct:modified "2019-12-21T07:22:01.754Z"^^xsd:dateTime .

:c_da6168d8 skos:note "NOTE: A dwelling is a unit where one or more people live (whether or not as a sole or main residence) in either of the following situations.<ul><li> A single person or people living together as a family.<li> A maximum of six people living together as a single household, including where care is provided for residents.</ul>"@en .

:c_13543964 dct:created "2019-12-21T06:12:19.585Z"^^xsd:dateTime;
  skos:broader :c_13911a49 .

:c_132d79ca dct:modified "2019-12-21T07:22:01.802Z"^^xsd:dateTime;
  skos:definition """ 
(of a building) The land occupied by the building, up to the boundaries with land in other ownership."""@en .

:c_b304ed8a dct:modified "2019-12-28T07:20:58.374Z"^^xsd:dateTime;
  rdfs:isDefinedBy <http://www.legislation.gov.uk/uksi/2010/2214/regulation/2> .

:skosxl:hiddenLabel dct:created "2018-03-28T15:40:48.579Z"^^xsd:dateTime .

:c_9e8d26ab dc:source :c_6c82c09f .

:c_b4ccd5f2 rdfs:isDefinedBy <http://www.legislation.gov.uk/uksi/2010/2214/regulation/2> .

:xl_en_6bbf3d9b a skosxl:Label;
  skosxl:literalForm "part d - toxic substances"@en .

:c_10ea4ecc dc:source :c_6c82c09f .

:c_b3f65603 dc:source :c_6c82c09f .

:c_56fef4b5 dct:created "2019-12-21T07:19:11.868Z"^^xsd:dateTime;
  skos:definition """(in relation to a side or external wall of a building) All of the following are classed as unprotected areas.
<ul><li>Any part of the external wall that has less than the relevant fire resistance set out in Section 13.
<li>	Any part of the external wall constructed of material more than 1mm thick if that material does not have a class B-s3, d2 rating or better, which is attached or applied, whether for cladding or any other purpose. 
<li>	Windows, doors or other openings. This does not include windows that are designed and glazed to give the necessary level of fire resistance and that are not openable.</ul>"""@en .

:c_28013078 a skos:Concept;
  dc:source :c_ca00c020;
  skos:inScheme :conceptScheme_751925ed .

:xl_en_400b0017 a skosxl:Label .

:c_34f295d5 dc:source :c_ca00c020;
  skos:definition "Includes a dwellinghouse and a flat."@en;
  skos:note "NOTE: A dwelling is a unit where one or more people live (whether or not as a sole or main residence) in either of the following situations.<ul><li> A single person or people living together as a family.<li> A maximum of six people living together as a single household, including where care is provided for residents.</ul>"@en .

:c_9b7f9eb7 skos:definition "A lift with additional protection and with controls that enable it to be used by the fire and rescue service when fighting a fire. (See Section 15.)"@en .

:c_88af4873 skos:prefLabel "firefighting lift (b2)"@en .

:c_b2cab8d9 dct:created "2019-12-12T20:47:12.799Z"^^xsd:dateTime;
  dct:modified "2019-12-13T22:39:26.964Z"^^xsd:dateTime;
  skos:broader :c_13911a49;
  skos:notation "B1"@en .

:c_e3cebf52 a skos:Concept;
  dct:modified "2019-12-28T07:36:46.720Z"^^xsd:dateTime;
  skos:broader :c_f9b32acf;
  skos:inScheme :conceptScheme_751925ed;
  skos:notation "part 03"@en;
  skos:prefLabel "notices, plans and certificates"@en;
  skosxl:prefLabel :xl_en_a3365120 .

:xl_en_a3365120 dct:modified "2018-07-20T19:09:32.114Z"^^xsd:dateTime .

:c_a965ecce a skos:Concept;
  dct:created "2019-12-12T20:47:00.103Z"^^xsd:dateTime;
  dct:modified "2020-10-28T15:19:02.690Z"^^xsd:dateTime;
  skos:broader :c_13911a49;
  skos:definition "The maximum aggregate plan perimeter, found by vertical projection onto a horizontal plane. (See Section 15.)"@en;
  skos:inScheme :conceptScheme_751925ed .

:c_be34e7b3 dc:source :c_6c82c09f .

:c_8258611b skos:note "NOTE: Enclosed lift wells, enclosed escalator wells, building services ducts and stairs are not classified as atria."@en .

:xl_en_44ca1675 skosxl:literalForm "aim"@en .

:xl_en_3e905d0b a skosxl:Label;
  skosxl:literalForm "part k - protection from falling, collision and impact"@en .

:c_f5536b7d dc:source :c_ca00c020;
  dct:created "2019-12-13T23:11:41.791Z"^^xsd:dateTime;
  skos:broader :c_13911a49;
  skos:inScheme :conceptScheme_751925ed;
  skos:prefLabel "ceiling"@en .

:c_7fc5469b dct:created "2019-12-13T23:07:38.815Z"^^xsd:dateTime;
  skos:broader :c_13911a49 .

:skosCollection_50d4bd2e skos:member :c_366cf430, :c_547611a3, :c_6e741d9b, :c_c92ba3dc,
    :c_fe309bb8 .

:c_c83014a4 a skos:Concept;
  dct:created "2018-03-29T10:22:54.432Z"^^xsd:dateTime;
  rdfs:isDefinedBy <http://www.legislation.gov.uk/uksi/2010/2214/part/2/made>;
  skos:broader :c_f9b32acf;
  skos:inScheme :conceptScheme_751925ed;
  skos:notation "part 02"@en .

:xl_en_786a7815 a skosxl:Label;
  dct:modified "2018-07-20T19:07:39.287Z"^^xsd:dateTime;
  skosxl:literalForm "control of building work"@en .

:c_b0f3b4fb dct:created "2019-12-12T20:50:36.136Z"^^xsd:dateTime;
  dct:modified "2019-12-13T22:42:18.989Z"^^xsd:dateTime;
  skos:broader :c_13911a49;
  skos:inScheme :conceptScheme_751925ed .

:c_33c0e1b5 dct:created "2019-12-13T23:16:16.374Z"^^xsd:dateTime;
  dct:modified "2019-12-13T23:33:59.393Z"^^xsd:dateTime;
  skos:broader :c_13911a49;
  skos:definition "A walkway, open to the air on one or more sides, that forms part of the escape route from more than one flat."@en .

:c_bed063fd a skos:Concept;
  dct:created "2019-12-13T23:17:32.193Z"^^xsd:dateTime;
  dct:modified "2020-10-26T07:33:12.073Z"^^xsd:dateTime;
  skos:definition "An escape stair that serves more than one flat."@en;
  skos:prefLabel "common stair"@en .

:xl_en_f259c22d a skosxl:Label;
  skosxl:literalForm "part j - combustion appliances and fuel storage systems"@en .

:xl_en_718751b0 a skosxl:Label;
  skosxl:literalForm """2.1.8
"""@en .

:c_6284471b dc:source :c_ca00c020 .

:c_3e5063e6 a skos:Concept;
  dc:source :c_ca00c020;
  dct:created "2019-12-13T23:02:15.181Z"^^xsd:dateTime;
  dct:modified "2019-12-13T23:33:58.928Z"^^xsd:dateTime .

:c_727adfdb dct:created "2019-12-21T07:12:19.397Z"^^xsd:dateTime;
  skos:definition "A final exit, or a doorway that gives direct access into a protected stairway, firefighting lobby or external escape route."@en .

:c_13911a49 skos:broader :c_ca00c020;
  skos:inScheme :conceptScheme_751925ed;
  skos:narrower :c_04c52352, :c_13543964, :c_228ee3b0, :c_727adfdb, :c_7fc5469b, :c_b0f3b4fb,
    :c_b6083e42, :c_bed063fd;
  skos:prefLabel "appendix a: key terms (adb)"@en .

:xl_en_0460024f a skosxl:Label;
  skosxl:literalForm "part l - conservation of fuel and power"@en .

:c_b6083e42 a skos:Concept;
  dc:source :c_ca00c020;
  dct:created "2019-11-30T12:49:44.067Z"^^xsd:dateTime;
  dct:isPartOf :c_6c82c09f, :c_ca00c020;
  skos:broader :c_13911a49;
  skos:definition "Escape routes that are sufficiently separated by direction and space or by fire resisting construction to ensure that one is still available if the other is affected by fire."@en;
  skos:inScheme :conceptScheme_751925ed;
  skos:prefLabel "alternative escape routes"@en;
  skos:scopeNote "NOTE: A second stair, balcony or flat roof which enables a person to reach a place free from danger from fire is considered an alternative escape route for the purposes of a dwellinghouse."@en .

:c_10030a9a a skos:Concept;
  dc:source :c_6c82c09f, :c_ca00c020;
  dct:modified "2020-10-28T15:19:35.891Z"^^xsd:dateTime .

:c_c02d4d7d dc:source :c_6c82c09f, :c_ca00c020;
  skos:broader :c_13911a49;
  skos:definition "Any permanent or temporary building but not any other kind of structure or erection. A reference to a building includes a reference to part of a building."@en .

:c_2658862b a skos:Concept;
  dct:created "2018-03-29T10:24:48.041Z"^^xsd:dateTime;
  rdfs:isDefinedBy <http://www.legislation.gov.uk/uksi/2010/2214/part/10/made>;
  skos:broader :c_f9b32acf;
  skos:inScheme :conceptScheme_751925ed;
  skos:notation "part 10"@en;
  skos:prefLabel "miscellaneous"@en;
  skosxl:prefLabel :xl_en_005f9565 .

:xl_en_005f9565 a skosxl:Label;
  dct:modified "2018-07-20T19:14:26.688Z"^^xsd:dateTime;
  skosxl:literalForm "miscellaneous"@en .

:xl_en_913b3693 skosxl:literalForm "plqs"@en .

:c_3518fece skos:broader :c_f9b32acf;
  skos:inScheme :conceptScheme_751925ed;
  skos:prefLabel "general"@en .

:xl_en_1ec12f25 skosxl:literalForm "oir"@en .

:c_4a90e0e1 a skos:Concept;
  dc:source :c_6c82c09f;
  dct:modified "2019-12-13T23:33:59.592Z"^^xsd:dateTime;
  skos:broader :c_13911a49;
  skos:inScheme :conceptScheme_751925ed;
  skos:note "NOTE: A roof space above the top storey of a compartment is included in that compartment. (See also ‘Separated part’.)"@en;
  skos:prefLabel "compartment (fire)"@en .

:c_9e8d26ab dc:source :c_ca00c020 .

:c_b44f46e0 dct:created "2019-12-21T06:58:14.334Z"^^xsd:dateTime;
  skos:broader :c_13911a49;
  skos:inScheme :conceptScheme_751925ed .

:xl_en_f987d3fd a skosxl:Label;
  skosxl:literalForm "smp"@en .

:xl_en_e99200e0 dct:modified "2018-07-20T21:02:30.704Z"^^xsd:dateTime .

:c_47c790ae dc:source :c_6c82c09f .

:c_64b1d307 dct:created "2018-03-29T10:23:57.951Z"^^xsd:dateTime;
  skos:prefLabel "water efficiency"@en;
  skosxl:prefLabel :xl_en_a7c1ef29 .

:c_f70bb786 a skos:Concept .

:c_04c52352 dct:modified "2020-10-28T15:16:12.379Z"^^xsd:dateTime;
  skos:definition "(of a building) Part of a building that is separated from another part of the same building by a compartment wall. The wall runs the full height of the part and is in one vertical plane. (See Appendix D, Diagram D5.)"@en .

:c_3da44764 dct:modified "2020-10-27T17:16:15.520Z"^^xsd:dateTime;
  skos:narrower :c_aae4241b, :c_cf85f340 .

<http://buildvoc.co.uk/resource/> owl:imports <http://purl.org/dc/elements/1.1/>,
    <http://purl.org/dc/terms/> .

:c_228ee3b0 dc:source :c_6c82c09f, :c_ca00c020;
  dct:isPartOf :c_6c82c09f, :c_ca00c020 .

:c_79a3679f dc:source :c_ca00c020 .

:c_ca00c020 skos:exactMatch <http://www.worldcat.org/oclc/1120217476> .

:c_00d0e0e8 dct:modified "2019-12-22T07:43:19.271Z"^^xsd:dateTime .

:c_2a34c0b8 a skos:Concept;
  dct:created "2018-03-28T19:11:31.113Z"^^xsd:dateTime;
  skos:inScheme :conceptScheme_751925ed;
  skos:prefLabel "part p - electrical safety"@en;
  skosxl:prefLabel :xl_en_2a32cf6f .

:c_1a6e1e92 dct:modified "2020-10-23T17:08:24.565Z"^^xsd:dateTime;
  skos:broader :c_502a871c .

:xl_en_2a32cf6f a skosxl:Label;
  skosxl:literalForm "part p - electrical safety"@en .

:c_b4ccd5f2 dct:modified "2019-12-28T07:24:42.666Z"^^xsd:dateTime .

:c_d5c15327 skos:inScheme :conceptScheme_751925ed;
  skos:prefLabel "protected circuit"@en .

:c_6d2c7baa dct:modified "2020-10-23T17:17:55.380Z"^^xsd:dateTime .

:xl_en_80102184 a skosxl:Label .

:xl_en_74ce780a a skosxl:Label;
  skosxl:literalForm """2
"""@en .

:conceptScheme_751925ed dc:contributor """HM Government
"""@en .

:c_2ca1576c a skos:Concept;
  dct:created "2018-03-28T19:10:21.168Z"^^xsd:dateTime;
  skos:broader :c_502a871c;
  skos:inScheme :conceptScheme_751925ed;
  skos:prefLabel "part f - ventilation"@en;
  skosxl:prefLabel :xl_en_a94d8a2b .

:c_62cc4d78 skos:broader :c_59a3ae21 .

:xl_en_a94d8a2b a skosxl:Label;
  skosxl:literalForm "part f - ventilation"@en .

:c_46be855e a skos:Concept;
  skos:definition "A shaft that enables people, air or objects to pass from one compartment to another, and which is enclosed with fire resisting construction."@en;
  skos:inScheme :conceptScheme_751925ed;
  skos:prefLabel "protected shaft"@en .

:c_40560ccd dct:modified "2019-12-21T06:53:32.043Z"^^xsd:dateTime;
  skos:definition "Includes two or more dwellings in the same building or on adjacent sites, designed and constructed as residential accommodation for vulnerable or elderly people who receive, or will receive, a support service."@en .

:c_28013078 dc:source :c_6c82c09f;
  dct:created "2019-12-13T23:06:17.075Z"^^xsd:dateTime;
  dct:modified "2020-10-25T07:07:36.633Z"^^xsd:dateTime;
  skos:broader :c_13911a49;
  skos:definition "A term that includes both local authority building control and approved inspectors."@en;
  skos:prefLabel "building control body (tba)"@en .

:c_7fc5469b a skos:Concept;
  dc:source :c_6c82c09f, :c_ca00c020;
  dct:modified "2019-12-13T23:33:59.168Z"^^xsd:dateTime .

:c_9e4931f7 dc:source :c_6c82c09f;
  skos:definition "A construction within a cavity, other than a smoke curtain, to perform either of the following functions.<ul><li>Close a cavity to stop smoke or flame entering.<li>Restrict the movement of smoke or flame within a cavity.</ul>"@en .

:c_f5536b7d dc:source :c_6c82c09f;
  skos:definition "Part of a building that encloses a room, protected shaft or circulation space and is exposed overhead. "@en .

:c_e7e6b110 dc:source :c_6c82c09f;
  skos:prefLabel "circulation space"@en .

:c_33c0e1b5 dc:source :c_6c82c09f .

:c_bed063fd dc:source :c_6c82c09f;
  skos:broader :c_13911a49 .

:c_13911a49 skos:broader :c_6c82c09f;
  skos:narrower :c_10030a9a, :c_28013078, :c_28e7c922, :c_4a90e0e1, :c_5724a233, :c_5ef03467,
    :c_79a3679f, :c_88af4873, :c_a965ecce, :c_b44f46e0, :c_b975b2d2, :c_c02d4d7d .

:skosxl:hiddenLabel rdfs:subClassOf owl:Thing .

:c_c83014a4 dct:modified "2019-12-21T09:55:20.492Z"^^xsd:dateTime .

:xl_en_2de5ebbe skosxl:literalForm "sb-imp"@en .

:c_cb3d4c10 dc:source :c_6c82c09f .

:c_7c12f560 a skos:Concept;
  skos:broader :c_13911a49;
  skos:inScheme :conceptScheme_751925ed;
  skos:prefLabel "protected stairway"@en .

:xl_en_8c98a903 a skosxl:Label;
  skosxl:literalForm """2.1.11
"""@en .

:c_b975b2d2 skos:definition "Any synthetic polymeric material that has a softening point below 200°C if tested to BS EN ISO 306 Method A120. Specimens for this test may be fabricated from the original polymer where the thickness of material of the end product is less than 2.5mm."@en .

:c_13543964 skos:definition "A circulation area, consisting of a hall or space in a flat, that is enclosed with fire resisting construction other than an external wall of a building."@en .

:c_3e5063e6 dc:source :c_6c82c09f;
  skos:prefLabel "basement storey"@en .

:c_b65b6f3f dct:created "2018-07-22T13:43:09.626Z"^^xsd:dateTime .

:c_6c82c09f skos:example <https://assets.publishing.service.gov.uk/government/uploads/system/uploads/attachment_data/file/832633/Approved_Document_B__fire_safety__volume_2_-_2019_edition.pdf> .

:c_706598d3 dc:source :c_6c82c09f .

:c_c02d4d7d dct:created "2019-12-13T23:04:41.568Z"^^xsd:dateTime .

:c_7b85eda3 dc:source :c_ca00c020 .

:c_10030a9a dct:created "2019-12-13T23:03:38.460Z"^^xsd:dateTime;
  skos:definition "The boundary of the land that belongs to a building, or, where the land abuts a road, railway, canal or river, the centre line of that road, railway, canal or river."@en;
  skos:inScheme :conceptScheme_751925ed .

:xl_en_ecb8813d a skosxl:Label .

:skosCollection_4ff8449c dct:created "2018-04-07T20:06:25.388Z"^^xsd:dateTime .

:skosCollection_50d4bd2e skos:member :c_0af8118b, :c_4775ba65, :c_58bdb729, :c_7abc215a,
    :c_c984b189, :c_d996e4f9 .

:c_e3cebf52 dct:created "2018-03-29T10:23:06.927Z"^^xsd:dateTime;
  rdfs:isDefinedBy <http://www.legislation.gov.uk/uksi/2010/2214/part/3/made> .

:c_b2cab8d9 a skos:Concept;
  skos:prefLabel "perimeter (of a building)"@en .

:c_5b4555d8 dct:modified "2019-12-22T07:44:14.524Z"^^xsd:dateTime .

:xl_en_74b321d9 skosxl:literalForm "pip"@en .

:c_58df2af5 a skos:Concept;
  skos:prefLabel "schedule 1"@en .

:c_b0f3b4fb skos:definition "(unless otherwise specified, e.g. as in the case of flats) The distance that a person would travel from any point within the floor area to the nearest storey exit, determined by the layout of walls, partitions and fittings."@en .

:c_34f295d5 rdfs:seeAlso <http://www.legislation.gov.uk/uksi/2010/2214/regulation/2>;
  skos:editorialNote "NOTE: Except for the items marked * (which are from the Building Regulations 2010), these definitions apply only to Approved Document B.<p>NOTE: The terms defined below are key terms used in this document only. Refer to BS 4422 for further guidance on the definitions of common terms used in the fire safety industry which are not listed below.</p>"@en .

:c_da6168d8 skos:editorialNote "NOTE: Except for the items marked * (which are from the Building Regulations 2010), these definitions apply only to Approved Document B.<p>NOTE: The terms defined below are key terms used in this document only. Refer to BS 4422 for further guidance on the definitions of common terms used in the fire safety industry which are not listed below.</p>"@en;
  skos:notation "*B2"@en .

:c_2658862b dct:modified "2019-12-28T07:36:30.761Z"^^xsd:dateTime .

:c_f70bb786 dct:created "2019-12-12T20:17:42.317Z"^^xsd:dateTime;
  skos:broader :c_13911a49;
  skos:definition "A fire resisting wall or floor to separate one fire compartment from another."@en;
  skos:inScheme :conceptScheme_751925ed;
  skos:notation "B2"@en;
  skos:note "NOTE: Provisions relating to construction are given in Section 8."@en;
  skos:prefLabel "compartment wall or floor"@en .

:xl_en_d34f5762 skosxl:literalForm "P"@en .

:c_28e7c922 a skos:Concept;
  dct:created "2019-12-15T08:40:53.169Z"^^xsd:dateTime;
  dct:modified "2019-12-15T08:46:58.969Z"^^xsd:dateTime;
  skos:broader :c_13911a49;
  skos:definition """A room such as any of the following.
<ul><li>Oil-filled transformer room.
<li>Switch gear room.
<li>Boiler room.
<li>Storage space for fuel or other highly flammable substance(s).
<li>Room that houses a fixed internal combustion engine.</ul>"""@en;
  skos:inScheme :conceptScheme_751925ed;
  skos:prefLabel "place of special fire hazard"@en .

:c_38ba0f99 a skos:Concept;
  skos:inScheme :conceptScheme_751925ed;
  skos:prefLabel "platform floor"@en .

:xl_en_511d9a71 a skosxl:Label;
  skosxl:literalForm "basmp"@en .

:c_6cbca36f dct:created "2018-08-20T10:00:12.829Z"^^xsd:dateTime .

:xl_en_32357ece a skosxl:Label .

:c_4fe84b3b skos:prefLabel "gross internal volume"@en .

:c_7a2d826e dc:source :c_6c82c09f .

:xl_en_f38b7b49 a skosxl:Label;
  skosxl:literalForm """2.1.7
"""@en .

:xl_en_9717bf9a a skosxl:Label;
  skosxl:literalForm "plans"@en .

:c_04c52352 dc:source :c_ca00c020 .

:xl_en_cff63d0f skosxl:literalForm "tidp"@en .

:xl_en_7699a05e a skosxl:Label;
  skosxl:literalForm "part g - sanitation, hot water safety and water efficiency"@en .

:c_79a3679f a skos:Concept;
  dct:created "2019-12-13T23:25:23.779Z"^^xsd:dateTime;
  skos:broader :c_13911a49;
  skos:definition "A design of a building containing flats, in which each flat is approached via a common horizontal internal access or circulation space, which may include a common entrance hall."@en;
  skos:inScheme :conceptScheme_751925ed;
  skos:prefLabel "corridor access"@en .

:c_228ee3b0 dct:modified "2020-10-26T07:27:03.595Z"^^xsd:dateTime .

:c_b44f46e0 skos:editorialNote "NOTE: Except for the items marked * (which are from the Building Regulations 2010), these definitions apply only to Approved Document B.<p>NOTE: The terms defined below are key terms used in this document only. Refer to BS 4422 for further guidance on the definitions of common terms used in the fire safety industry which are not listed below.</p>"@en;
  skos:notation "*"@en .

:c_5724a233 a skos:Concept;
  dct:created "2019-12-21T07:05:05.556Z"^^xsd:dateTime;
  skos:broader :c_13911a49;
  skos:definition """Includes any of the following.
<ul><li>Any gallery in an assembly building (purpose group 5).
<li>Any gallery in any other type of building if its area is more than half that of the space into which it projects.
<li>A roof, unless it is accessible only for maintenance and repair.</ul>"""@en;
  skos:inScheme :conceptScheme_751925ed;
  skos:note "NOTE: The building is regarded as a multi-storey building if both of the following apply.<ul><li>There is more than one gallery. <li>The total aggregate area of all the galleries in one space is more than half the floor area of that space.</ul>"@en;
  skos:prefLabel "storey"@en .

:c_42d467db a skos:Concept;
  dct:created "2018-03-28T19:10:37.917Z"^^xsd:dateTime;
  skos:broader :c_502a871c;
  skos:inScheme :conceptScheme_751925ed;
  skos:prefLabel "part h - drainage and waste disposal"@en;
  skosxl:prefLabel :xl_en_8587f86b .

:c_73c4361e a skos:Concept;
  dct:created "2018-03-28T19:10:28.620Z"^^xsd:dateTime;
  skos:broader :c_502a871c;
  skos:inScheme :conceptScheme_751925ed;
  skos:prefLabel "part g - sanitation, hot water safety and water efficiency"@en;
  skosxl:prefLabel :xl_en_7699a05e .

:c_44c61ce8 skos:prefLabel "ventilation 2010 edition incorporating 2010 and 2013 amendments"@en .

:xl_en_8587f86b a skosxl:Label;
  skosxl:literalForm "part h - drainage and waste disposal"@en .

:xl_en_1333d9a7 a skosxl:Label;
  skosxl:literalForm """2.1.6
"""@en .

:c_ee10273a dc:source :c_6c82c09f;
  dct:created "2019-12-21T06:21:43.979Z"^^xsd:dateTime;
  dct:modified "2019-12-21T06:27:11.530Z"^^xsd:dateTime;
  skos:broader :c_13911a49;
  skos:definition "The boundary or notional boundary that one side of the building faces and/or coincides with, and that is parallel or at an angle of a maximum of 80 degrees to that side of the building."@en .

:c_13911a49 skos:narrower :c_cc61a0f4, :c_e7e6b110, :c_ee10273a .

:c_cc61a0f4 a skos:Concept;
  dc:source :c_6c82c09f, :c_ca00c020;
  dct:created "2019-12-21T06:23:21.636Z"^^xsd:dateTime;
  skos:broader :c_13911a49;
  skos:definition "A dome light, lantern light, skylight, ridge light, glazed barrel vault or other element to admit daylight through a roof."@en;
  skos:inScheme :conceptScheme_751925ed;
  skos:prefLabel "rooflight"@en .

:c_83464c52 skos:inScheme :conceptScheme_751925ed .

:xl_en_400b0017 skosxl:literalForm "part m - access to and use of buildings"@en .

:c_88af4873 a skos:Concept;
  dct:created "2019-12-12T20:43:47.043Z"^^xsd:dateTime;
  dct:modified "2020-10-28T14:52:08.828Z"^^xsd:dateTime;
  skos:broader :c_13911a49;
  skos:definition "A lift with additional protection and with controls that enable it to be used by the fire and rescue service when fighting a fire. (See Section 17.)"@en;
  skos:inScheme :conceptScheme_751925ed .

:c_9b7f9eb7 a skos:Concept;
  dct:created "2019-12-12T20:43:57.040Z"^^xsd:dateTime;
  skos:broader :c_13911a49;
  skos:inScheme :conceptScheme_751925ed .

:xl_en_8715993d skosxl:literalForm "cobie"@en .

:xl_en_a3365120 a skosxl:Label .

:c_7c12f560 dc:source :c_6c82c09f;
  dct:modified "2019-12-21T06:27:11.881Z"^^xsd:dateTime .

:c_46be855e dc:source :c_6c82c09f, :c_ca00c020;
  dct:modified "2019-12-21T06:27:12.018Z"^^xsd:dateTime .

:c_13543964 dc:source :c_6c82c09f, :c_ca00c020 .

:c_7400b440 dc:source :c_6c82c09f, :c_ca00c020 .

:c_7b85eda3 dc:source :c_6c82c09f .

:xl_en_bdc8faa4 a skosxl:Label;
  skosxl:literalForm """2.1.5
"""@en .

:c_5ffbc967 a skos:Concept;
  dct:created "2018-03-28T19:11:39.728Z"^^xsd:dateTime;
  skos:broader :c_502a871c;
  skos:inScheme :conceptScheme_751925ed;
  skos:prefLabel "part q - security"@en;
  skosxl:prefLabel :xl_en_93b6dba8 .

:c_679215e0 dct:created "2020-10-25T05:17:58.202Z"^^xsd:dateTime .

:c_fec1533e a skos:Concept;
  dct:created "2018-03-28T19:10:47.855Z"^^xsd:dateTime;
  skos:broader :c_502a871c;
  skos:inScheme :conceptScheme_751925ed;
  skos:prefLabel "part j - combustion appliances and fuel storage systems"@en;
  skosxl:prefLabel :xl_en_f259c22d .

:c_152c4bbc skos:narrower :c_01839084 .

:c_8cba3c82 a skos:Concept;
  dct:created "2018-03-28T19:10:07.222Z"^^xsd:dateTime;
  skos:inScheme :conceptScheme_751925ed;
  skos:prefLabel "part d - toxic substances"@en;
  skosxl:prefLabel :xl_en_6bbf3d9b .

:c_b7bccf3d a skos:Concept;
  dct:created "2018-03-28T19:11:51.452Z"^^xsd:dateTime;
  skos:broader :c_502a871c;
  skos:inScheme :conceptScheme_751925ed;
  skos:prefLabel "part r - physical infrastructure for high speed electronic communications networks"@en;
  skosxl:prefLabel :xl_en_b9ef8f0c .

:c_0109c085 skos:inScheme :conceptScheme_751925ed .

:c_a20cbb62 a skos:Concept;
  dct:created "2018-03-28T19:11:17.122Z"^^xsd:dateTime;
  skos:broader :c_502a871c;
  skos:inScheme :conceptScheme_751925ed;
  skos:prefLabel "part m - access to and use of buildings"@en;
  skosxl:prefLabel :xl_en_400b0017 .

:c_be604dfa a skos:Concept;
  dct:created "2018-03-28T19:10:59.073Z"^^xsd:dateTime;
  skos:broader :c_502a871c;
  skos:inScheme :conceptScheme_751925ed;
  skos:prefLabel "part k - protection from falling, collision and impact"@en;
  skosxl:prefLabel :xl_en_3e905d0b .

:skosCollection_50d4bd2e skos:member :c_1d89066b, :c_2ca7a450, :c_8883ce73 .

:c_f68328a2 a skos:Concept;
  dct:created "2018-03-28T19:11:07.411Z"^^xsd:dateTime;
  skos:broader :c_502a871c;
  skos:inScheme :conceptScheme_751925ed;
  skos:prefLabel "part l - conservation of fuel and power"@en;
  skosxl:prefLabel :xl_en_0460024f .

:c_ae74ec82 dct:modified "2020-10-26T06:52:56.572Z"^^xsd:dateTime .

:c_e186f594 a skos:Concept;
  dct:created "2018-03-28T19:09:58.476Z"^^xsd:dateTime;
  dct:modified "2020-10-23T17:06:53.653Z"^^xsd:dateTime;
  skos:broader :c_502a871c;
  skos:inScheme :conceptScheme_751925ed;
  skos:prefLabel "part c - site preparation and resistance to contaminates and moisture"@en;
  skosxl:prefLabel :xl_en_c14ad7c7 .

:c_2a34c0b8 skos:broader :c_502a871c .

:c_835978b6 dct:modified "2020-10-27T08:47:32.078Z"^^xsd:dateTime .

:c_c66a31b4 dct:modified "2020-10-27T16:10:33.573Z"^^xsd:dateTime .

:xl_en_d2f47531 a skosxl:Label .

:c_f5536b7d a skos:Concept;
  skos:note "NOTE: The soffit of a rooflight, but not the frame, is included as part of the surface of the ceiling. An upstand below a rooflight is considered as a wall."@en .

:c_e7e6b110 a skos:Concept;
  dct:created "2019-12-13T23:13:42.083Z"^^xsd:dateTime;
  dct:modified "2020-10-26T07:20:05.119Z"^^xsd:dateTime;
  skos:broader :c_13911a49;
  skos:definition "A space (including a protected stairway) mainly used as a means of access between a room and an exit from the building or compartment."@en;
  skos:inScheme :conceptScheme_751925ed .

:c_cb3d4c10 dc:source :c_ca00c020;
  dct:created "2019-12-21T06:24:42.742Z"^^xsd:dateTime;
  dct:modified "2019-12-21T06:27:11.372Z"^^xsd:dateTime;
  skos:broader :c_13911a49;
  skos:definition "An enclosed space within a building that is not used solely as a circulation space. The term includes not only conventional rooms, but also cupboards that are not fittings and large spaces such as warehouses and auditoria. The term does not include cavities such as ducts, ceiling cavities and roof spaces."@en;
  skos:inScheme :conceptScheme_751925ed;
  skos:prefLabel "room"@en .

:c_13911a49 skos:narrower :c_61f82d61, :c_6284471b, :c_7400b440, :c_7b85eda3, :c_7c12f560,
    :c_8258611b, :c_b2cab8d9, :c_cb3d4c10, :c_d32d8045, :c_d5c15327 .

:c_ee10273a a skos:Concept;
  dc:source :c_ca00c020;
  skos:prefLabel "relevant boundary"@en .

:c_b3f65603 dct:created "2019-12-15T08:27:29.025Z"^^xsd:dateTime;
  skos:broader :c_13911a49 .

:c_9e4931f7 dc:source :c_ca00c020;
  dct:modified "2019-12-13T23:33:59.230Z"^^xsd:dateTime .

:c_56fef4b5 a skos:Concept;
  dct:modified "2019-12-21T07:22:01.287Z"^^xsd:dateTime;
  skos:prefLabel "unprotected area"@en .

:c_64b1d307 dct:modified "2019-12-22T07:45:01.333Z"^^xsd:dateTime .

:c_61f82d61 dct:created "2019-12-13T22:48:54.196Z"^^xsd:dateTime;
  dct:modified "2019-12-13T23:33:58.730Z"^^xsd:dateTime;
  skos:broader :c_13911a49;
  skos:definition "A duct to deliver combustion air to a gas appliance."@en;
  skos:inScheme :conceptScheme_751925ed;
  skos:prefLabel "appliance ventilation duct"@en .

:c_6284471b dct:created "2019-12-13T22:51:41.721Z"^^xsd:dateTime;
  dct:modified "2019-12-13T23:33:58.863Z"^^xsd:dateTime;
  skos:broader :c_13911a49;
  skos:definition "A device that normally holds a door open, but closes it automatically if any one of the following occurs.<ul><ul>Smoke is detected by an automatic device of a suitable nature and quality in a suitable location.<li>A hand-operated switch, fitted in a suitable position, is operated.<li>The electricity supply to the device, apparatus or switch fails.<li>The fire alarm system, if any, is operated.</ul>"@en;
  skos:inScheme :conceptScheme_751925ed .

:c_793b849c dct:created "2018-08-11T13:05:19.050Z"^^xsd:dateTime .

:xl_en_74b321d9 a skosxl:Label .

:c_b975b2d2 dc:source :c_ca00c020;
  dct:modified "2019-12-21T07:22:01.349Z"^^xsd:dateTime .

:c_8258611b a skos:Concept;
  dct:created "2019-12-13T22:50:02.994Z"^^xsd:dateTime;
  dct:modified "2019-12-13T23:33:58.801Z"^^xsd:dateTime;
  skos:broader :c_13911a49;
  skos:definition "A continuous space that passes through one or more structural floors within a building, not necessarily vertically."@en;
  skos:inScheme :conceptScheme_751925ed .

:skosCollection_c85ed09f dct:created "2018-03-28T14:43:50.385Z"^^xsd:dateTime .

:c_3cae7829 dc:source :c_6c82c09f .

:c_5ef03467 a skos:Concept;
  dct:created "2019-12-13T22:46:11.837Z"^^xsd:dateTime;
  skos:broader :c_13911a49;
  skos:inScheme :conceptScheme_751925ed;
  skos:prefLabel "alternative exit"@en .

:c_58df2af5 dct:created "2019-12-21T10:17:39.618Z"^^xsd:dateTime;
  skos:inScheme :conceptScheme_751925ed;
  skos:narrower :c_56aca7cf .

:c_da6168d8 dc:source :c_6c82c09f .

:xl_en_32357ece skosxl:literalForm "eir"@en .

:c_3518fece dct:created "2019-12-22T07:35:30.866Z"^^xsd:dateTime .

:c_727adfdb dct:modified "2019-12-21T07:22:01.574Z"^^xsd:dateTime;
  skos:note "NOTE: If an institutional building is planned to enable progressive horizontal evacuation, a door in a compartment wall is considered a storey exit for the purposes of requirement B1."@en .

:c_a4eaf123 a skos:Concept;
  dct:created "2019-12-21T07:13:55.109Z"^^xsd:dateTime;
  skos:broader :c_13911a49;
  skos:inScheme :conceptScheme_751925ed;
  skos:prefLabel "suspended ceiling"@en .

:c_d5c15327 dc:source :c_6c82c09f, :c_ca00c020;
  dct:created "2019-12-15T08:44:56.144Z"^^xsd:dateTime;
  skos:broader :c_13911a49 .

:c_38ba0f99 dc:source :c_ca00c020 .

:c_28e7c922 dc:source :c_ca00c020 .

:c_35d3a535 dc:source :c_ca00c020 .

:c_7b85eda3 a skos:Concept;
  dct:created "2019-12-21T06:10:33.715Z"^^xsd:dateTime;
  skos:broader :c_13911a49;
  skos:inScheme :conceptScheme_751925ed;
  skos:prefLabel "protected corridor/lobby"@en .

:c_7c12f560 dct:created "2019-12-21T06:14:37.859Z"^^xsd:dateTime .

:c_33c0e1b5 skos:prefLabel "common balcony"@en .

:c_f70bb786 dc:source :c_6c82c09f .

:c_9e8d26ab dct:modified "2019-12-14T08:48:47.100Z"^^xsd:dateTime .

:xl_en_d34f5762 dct:modified "2018-06-01T23:31:11.865Z"^^xsd:dateTime .

:c_6c82c09f skos:exactMatch <http://www.worldcat.org/oclc/1120217476>;
  skos:narrower :c_4f2b64be .

:c_228ee3b0 a skos:Concept .

:c_b6083e42 dct:modified "2019-12-13T23:33:58.541Z"^^xsd:dateTime .

:c_cb86c2ff dc:source :c_6c82c09f .

:c_c07e16c5 skos:prefLabel "free area"@en .

:skosCollection_50d4bd2e skos:member :c_c53e946f .

:c_ca00c020 skos:topConceptOf :c_ca00c020 .

:c_5b4555d8 a skos:Concept;
  dct:created "2018-03-29T10:23:50.673Z"^^xsd:dateTime;
  rdfs:isDefinedBy <http://www.legislation.gov.uk/uksi/2010/2214/part/6/made>;
  skos:broader :c_f9b32acf;
  skos:inScheme :conceptScheme_751925ed;
  skos:notation "part 06"@en;
  skos:prefLabel "energy efficiency requirements"@en;
  skosxl:prefLabel :xl_en_1d7aac94 .

:xl_en_1d7aac94 a skosxl:Label;
  dct:modified "2018-07-20T19:11:40.210Z"^^xsd:dateTime;
  skosxl:literalForm "energy efficiency requirements"@en .

:xl_en_f2eee9b5 a skosxl:Label .

:xl_en_d4ddf75e a skosxl:Label;
  skosxl:literalForm "bim"@en .

:c_b0f3b4fb skos:prefLabel "travel distance"@en .

:c_7400b440 dct:created "2019-12-21T06:16:01.865Z"^^xsd:dateTime;
  dct:modified "2019-12-21T06:27:11.768Z"^^xsd:dateTime;
  skos:broader :c_13911a49;
  skos:definition "A classification of a building according to the purpose to which it is intended to be put. (See Table 0.1.)"@en .

:c_d32d8045 dc:source :c_6c82c09f, :c_ca00c020;
  dct:created "2019-12-21T06:49:49.146Z"^^xsd:dateTime;
  dct:modified "2019-12-21T06:53:32.122Z"^^xsd:dateTime;
  skos:broader :c_13911a49;
  skos:definition "building A building that consists of a ground storey only. Basements are not counted as storeys in a building (see Appendix D). A separated part that consists of a ground storey only, with a roof to which access is only provided for repair or maintenance, may be treated as a single storey building."@en;
  skos:inScheme :conceptScheme_751925ed .

:c_40560ccd dc:source :c_6c82c09f, :c_ca00c020 .

:c_132d79ca a skos:Concept .

:c_f479d1cb dct:created "2018-08-11T14:26:15.280Z"^^xsd:dateTime .

:xl_en_63b1eba4 a skosxl:Label;
  skosxl:literalForm """2.1.4
"""@en .

:xl_en_93b6dba8 a skosxl:Label;
  skosxl:literalForm "part q - security"@en .

:c_d4480e31 dct:modified "2020-10-28T15:11:21.052Z"^^xsd:dateTime .

:c_56fef4b5 dc:source :c_ca00c020;
  skos:note "NOTE: Recessed car parking areas as shown in Diagram A1 should not be regarded as unprotected areas."@en .

:c_cd2ba206 a skos:Concept;
  dc:source :c_6c82c09f, :c_ca00c020;
  dct:created "2019-12-14T06:21:42.550Z"^^xsd:dateTime;
  dct:modified "2019-12-14T06:53:28.582Z"^^xsd:dateTime;
  skos:broader :c_13911a49;
  skos:definition "An area from which escape is possible in one direction only."@en;
  skos:inScheme :conceptScheme_751925ed;
  skos:prefLabel "dead end"@en .

:c_13911a49 skos:narrower :c_47c790ae, :c_49a5a923, :c_7e4da283, :c_b304ed8a, :c_b4ccd5f2,
    :c_b67f0d40, :c_b98dbf2a, :c_c916e597, :c_cd2ba206, :c_f12e46ec, :c_f636fce4 .

:c_b4ccd5f2 a skos:Concept;
  dc:source :c_6c82c09f, :c_ca00c020;
  dct:created "2019-12-14T06:49:21.314Z"^^xsd:dateTime;
  rdfs:seeAlso <http://www.legislation.gov.uk/uksi/2010/2214/regulation/2>;
  skos:broader :c_13911a49;
  skos:definition """The external wall of a building includes all of the following. 
<ul><li>Anything located within any space forming part of the wall.
<li>Any decoration or other finish applied to any external (but not internal) surface forming part of the wall.
<li>Any windows and doors in the wall.
<li>Any part of a roof pitched at an angle of more than 70 degrees to the horizontal if that part of the roof adjoins a space within the building to which persons have access, but not access only for the purpose of carrying out repairs or maintenance.</ul>"""@en;
  skos:editorialNote "NOTE: Except for the items marked * (which are from the Building Regulations 2010), these definitions apply only to Approved Document B.<p>NOTE: The terms defined below are key terms used in this document only. Refer to BS 4422 for further guidance on the definitions of common terms used in the fire safety industry which are not listed below.</p>"@en;
  skos:inScheme :conceptScheme_751925ed;
  skos:notation "*"@en;
  skos:prefLabel "external wall"@en .

:c_f636fce4 a skos:Concept;
  dc:source :c_6c82c09f, :c_ca00c020;
  dct:created "2019-12-14T06:23:01.241Z"^^xsd:dateTime;
  dct:modified "2019-12-14T06:53:28.651Z"^^xsd:dateTime;
  skos:broader :c_13911a49;
  skos:definition "The shortest distance from any point within the floor area to the nearest storey exit, measured within the external enclosures of the building, and ignoring walls, partitions and fittings other than the enclosing walls and partitions to protected stairways."@en;
  skos:inScheme :conceptScheme_751925ed;
  skos:prefLabel "direct distance"@en .

:c_b304ed8a a skos:Concept;
  dc:source :c_6c82c09f, :c_ca00c020;
  dct:created "2019-12-14T06:25:02.042Z"^^xsd:dateTime;
  rdfs:seeAlso <http://www.legislation.gov.uk/uksi/2010/2214/regulation/2>;
  skos:broader :c_13911a49;
  skos:definition "Does not include a flat or a building containing a flat."@en;
  skos:editorialNote "NOTE: Except for the items marked * (which are from the Building Regulations 2010), these definitions apply only to Approved Document B.<p>NOTE: The terms defined below are key terms used in this document only. Refer to BS 4422 for further guidance on the definitions of common terms used in the fire safety industry which are not listed below.</p>"@en;
  skos:inScheme :conceptScheme_751925ed;
  skos:notation "*"@en;
  skos:prefLabel "dwellinghouse"@en .

:c_7e4da283 a skos:Concept;
  dc:source :c_6c82c09f, :c_ca00c020;
  dct:created "2019-12-14T06:31:19.918Z"^^xsd:dateTime;
  dct:modified "2019-12-14T06:53:29.065Z"^^xsd:dateTime;
  skos:broader :c_13911a49;
  skos:definition """Any of the following.
<ul><li>A member that forms part of the structural frame of a building, or any other beam or column.
<li>A loadbearing wall or loadbearing part of a wall.
<li>A floor.
<li>A gallery (but not a loading gallery, fly gallery, stage grid, lighting bridge, or any gallery provided for similar purposes or for maintenance and repair).
<li>An external wall.
<li>A compartment wall (including a wall that is common to two or more buildings).</ul>
"""@en;
  skos:inScheme :conceptScheme_751925ed;
  skos:note "NOTE: However, see the guidance to requirement B3, paragraph 7.3, for a list of structures that are not considered to be elements of structure."@en;
  skos:prefLabel "element of structure"@en .

:c_49a5a923 a skos:Concept;
  dc:source :c_6c82c09f, :c_ca00c020;
  dct:created "2019-12-14T06:34:27.645Z"^^xsd:dateTime;
  dct:modified "2019-12-14T06:53:29.138Z"^^xsd:dateTime;
  skos:broader :c_13911a49;
  skos:definition "Lighting for use when the power supply to the normal lighting fails."@en;
  skos:inScheme :conceptScheme_751925ed;
  skos:prefLabel "emergency lighting"@en .

:c_b67f0d40 a skos:Concept;
  dc:source :c_6c82c09f, :c_ca00c020;
  dct:created "2019-12-14T06:36:59.442Z"^^xsd:dateTime;
  dct:modified "2019-12-14T06:53:29.194Z"^^xsd:dateTime;
  skos:broader :c_13911a49;
  skos:definition "The part of the emergency lighting that is provided to ensure that the escape route is illuminated at all material times."@en;
  skos:inScheme :conceptScheme_751925ed;
  skos:prefLabel "escape lighting"@en .

:c_b98dbf2a a skos:Concept;
  dc:source :c_6c82c09f, :c_ca00c020;
  dct:created "2019-12-14T06:43:26.810Z"^^xsd:dateTime;
  dct:modified "2019-12-14T06:53:29.257Z"^^xsd:dateTime;
  skos:broader :c_13911a49;
  skos:definition "The route along which people can escape from any point in a building to a final exit."@en;
  skos:inScheme :conceptScheme_751925ed;
  skos:prefLabel "escape route"@en .

:c_c916e597 a skos:Concept;
  dc:source :c_6c82c09f, :c_ca00c020;
  dct:created "2019-12-14T06:44:56.922Z"^^xsd:dateTime;
  dct:modified "2019-12-14T06:53:29.333Z"^^xsd:dateTime;
  skos:broader :c_13911a49;
  skos:definition "A lift that may be used to evacuate people in a fire."@en;
  skos:inScheme :conceptScheme_751925ed;
  skos:prefLabel "evacuation lift"@en .

:c_f12e46ec a skos:Concept;
  dc:source :c_6c82c09f, :c_ca00c020;
  dct:created "2019-12-14T06:46:09.069Z"^^xsd:dateTime;
  dct:modified "2019-12-14T06:53:29.420Z"^^xsd:dateTime;
  skos:broader :c_13911a49;
  skos:definition "A protected passageway that connects a protected stairway to a final exit."@en;
  skos:inScheme :conceptScheme_751925ed;
  skos:note "NOTE: Exit passageways should be protected to the same standard as the stairway they serve."@en;
  skos:prefLabel "exit passageway"@en .

:c_da6168d8 rdfs:seeAlso <http://www.legislation.gov.uk/uksi/2010/2214/regulation/2> .

:c_ca00c020 skos:narrower :c_13911a49 .

:c_6c82c09f skos:narrower :c_13911a49 .

:c_c02d4d7d rdfs:seeAlso <http://www.legislation.gov.uk/uksi/2010/2214/regulation/2>;
  skos:editorialNote "NOTE: Except for the items marked * (which are from the Building Regulations 2010), these definitions apply only to Approved Document B.<p>NOTE: The terms defined below are key terms used in this document only. Refer to BS 4422 for further guidance on the definitions of common terms used in the fire safety industry which are not listed below.</p>"@en .

:c_47c790ae a skos:Concept;
  dc:source :c_ca00c020;
  dct:created "2019-12-14T08:08:45.280Z"^^xsd:dateTime;
  dct:modified "2019-12-14T08:48:47.736Z"^^xsd:dateTime;
  skos:broader :c_13911a49;
  skos:definition "The end of an escape route from a building that gives direct access to a street, passageway, walkway or open space, and is sited to ensure that people rapidly disperse away from the building so that they are no longer in danger from fire and/or smoke."@en;
  skos:inScheme :conceptScheme_751925ed;
  skos:note "NOTE: Windows are not acceptable as final exits."@en;
  skos:prefLabel "final exit"@en .

:c_cb86c2ff a skos:Concept;
  dct:created "2019-12-14T08:22:05.410Z"^^xsd:dateTime;
  dct:modified "2019-12-14T08:48:47.223Z"^^xsd:dateTime;
  skos:broader :c_13911a49;
  skos:definition "A door or shutter which, together with its frame and furniture as installed in a building, is intended (when closed) to resist the spread of fire and/or gaseous products of combustion and meets specified performance criteria to those ends."@en;
  skos:inScheme :conceptScheme_751925ed;
  skos:note "NOTE: A fire doorset may have one or more leaves. The term includes a cover or other form of protection to an opening in a fire resisting wall or floor, or in a structure that surrounds a protected shaft. A fire doorset is a complete door assembly, assembled on site or delivered as a completed assembly, consisting of the door frame, leaf or leaves, essential hardware, edge seals and glazing, and any integral side panels or fanlight panels in an associated door screen."@en;
  skos:prefLabel "fire doorset"@en .

:c_7804ad6c a skos:Concept;
  dc:source :c_ca00c020;
  dct:created "2019-12-14T08:10:24.678Z"^^xsd:dateTime;
  skos:broader :c_13911a49;
  skos:definition "Combination of components for giving an audible and/or other perceptible warning of fire."@en;
  skos:inScheme :conceptScheme_751925ed;
  skos:prefLabel "fire alarm system"@en .

:c_c8b52d92 a skos:Concept;
  dc:source :c_6c82c09f, :c_ca00c020;
  dct:created "2019-12-14T08:12:53.416Z"^^xsd:dateTime;
  dct:modified "2019-12-14T08:48:47.374Z"^^xsd:dateTime;
  skos:broader :c_13911a49;
  skos:definition "A fire damper which, in addition to the performance of the fire damper, resists the spread of smoke."@en;
  skos:inScheme :conceptScheme_751925ed;
  skos:prefLabel "fire and smoke damper"@en .

:c_13911a49 skos:narrower :c_14b52896, :c_1a7ea9e5, :c_362390fa, :c_3cae7829, :c_706598d3,
    :c_7804ad6c, :c_7a2d826e, :c_9a0f5e20, :c_9e8d26ab, :c_b980c88c, :c_c8b52d92, :c_cb86c2ff,
    :c_d8e990c2, :c_dd03e186 .

:c_1a7ea9e5 a skos:Concept;
  dc:source :c_6c82c09f, :c_ca00c020;
  dct:created "2019-12-14T08:11:47.430Z"^^xsd:dateTime;
  dct:modified "2019-12-14T08:48:47.468Z"^^xsd:dateTime;
  skos:broader :c_13911a49;
  skos:definition "A mechanical or intumescent device within a duct or ventilation opening that operates automatically and is designed to resist the spread of fire."@en;
  skos:inScheme :conceptScheme_751925ed;
  skos:prefLabel "fire damper"@en .

:c_9e8d26ab a skos:Concept;
  dct:created "2019-12-14T08:37:19.617Z"^^xsd:dateTime;
  skos:broader :c_13911a49;
  skos:definition "A protected lobby that provides access from a firefighting stair to the accommodation area and to any associated firefighting lift."@en;
  skos:inScheme :conceptScheme_751925ed;
  skos:prefLabel "firefighting lobby"@en .

:c_14b52896 a skos:Concept;
  dct:created "2019-12-14T08:38:57.474Z"^^xsd:dateTime;
  skos:broader :c_13911a49;
  skos:definition "A protected enclosure that contains a firefighting stair, firefighting lobbies and, if provided, a firefighting lift together with its machine room."@en;
  skos:inScheme :conceptScheme_751925ed;
  skos:prefLabel "firefighting shaft"@en .

:c_9a0f5e20 a skos:Concept;
  dc:source :c_ca00c020;
  dct:created "2019-12-14T08:40:17.510Z"^^xsd:dateTime;
  skos:broader :c_13911a49;
  skos:definition "A protected stairway that connects to the accommodation area through only a firefighting lobby."@en;
  skos:inScheme :conceptScheme_751925ed;
  skos:prefLabel "firefighting stair"@en .

:c_3cae7829 a skos:Concept;
  dc:source :c_ca00c020;
  dct:created "2019-12-14T08:41:43.182Z"^^xsd:dateTime;
  skos:broader :c_13911a49;
  skos:definition "The ability of a component or a building to satisfy, for a stated period of time, some or all of the appropriate criteria given in the relevant standard."@en;
  skos:inScheme :conceptScheme_751925ed;
  skos:prefLabel "fire resisting (Fire resistance)"@en .

:c_7a2d826e a skos:Concept;
  dc:source :c_ca00c020;
  dct:created "2019-12-14T08:43:50.303Z"^^xsd:dateTime;
  dct:modified "2020-10-26T07:31:03.576Z"^^xsd:dateTime;
  skos:broader :c_13911a49;
  skos:definition "A compartment wall, compartment floor, cavity barrier and construction that encloses a protected escape route and/or a place of special fire hazard."@en;
  skos:inScheme :conceptScheme_751925ed;
  skos:prefLabel "fire-separating element"@en .

:c_706598d3 a skos:Concept;
  dc:source :c_ca00c020;
  dct:created "2019-12-14T08:45:42.181Z"^^xsd:dateTime;
  dct:modified "2019-12-14T08:48:46.560Z"^^xsd:dateTime;
  skos:broader :c_13911a49;
  skos:definition "A seal provided to close an imperfection of fit or design tolerance between elements or components, to restrict the spread of fire and smoke."@en;
  skos:inScheme :conceptScheme_751925ed;
  skos:prefLabel "fire-stop (Fire-stopping)"@en .

:c_362390fa a skos:Concept;
  dc:rights :c_6c82c09f;
  dc:source :c_6c82c09f, :c_ca00c020;
  dct:created "2019-12-15T07:08:51.487Z"^^xsd:dateTime;
  dct:modified "2019-12-15T07:54:23.946Z"^^xsd:dateTime;
  skos:broader :c_13911a49;
  skos:definition "A flat is a separate and self-contained premises constructed or adapted for use for residential purposes and forming part of a building from some other part of which it is divided horizontally."@en;
  skos:editorialNote "NOTE: Except for the items marked * (which are from the Building Regulations 2010), these definitions apply only to Approved Document B.<p>NOTE: The terms defined below are key terms used in this document only. Refer to BS 4422 for further guidance on the definitions of common terms used in the fire safety industry which are not listed below.</p> "@en;
  skos:inScheme :conceptScheme_751925ed;
  skos:notation "*"@en;
  skos:prefLabel "flat"@en .

:c_abc6dc1e a skos:Concept;
  dc:source :c_6c82c09f, :c_ca00c020;
  dct:created "2019-12-15T07:39:20.183Z"^^xsd:dateTime;
  dct:modified "2019-12-21T06:41:26.072Z"^^xsd:dateTime;
  skos:broader :c_4f2b64be;
  skos:inScheme :conceptScheme_751925ed;
  skos:prefLabel "diagram d1 measurement of door width"@en .

:c_b980c88c a skos:Concept;
  dc:rights :c_6c82c09f;
  dc:source :c_6c82c09f, :c_ca00c020;
  dct:created "2019-12-15T07:11:52.263Z"^^xsd:dateTime;
  dct:modified "2019-12-15T07:54:23.704Z"^^xsd:dateTime;
  skos:broader :c_13911a49;
  skos:definition "A floor or balcony that does not extend across the full extent of a building’s footprint and is open to the floor below."@en;
  skos:inScheme :conceptScheme_751925ed;
  skos:prefLabel "gallery"@en .

:c_4f2b64be a skos:Concept;
  dct:created "2019-12-15T07:22:31.525Z"^^xsd:dateTime;
  dct:modified "2019-12-15T08:07:58.561Z"^^xsd:dateTime;
  skos:broader :c_6c82c09f, :c_ca00c020;
  skos:inScheme :conceptScheme_751925ed;
  skos:narrower :c_45ef22f5, :c_8d791a67, :c_abc6dc1e, :c_c1a78f4b, :c_cc92c6ff;
  skos:note "<ul><li>a. Double pitch roof<ul>b. Mansard type roof<li>c. Flat or monopitch roof</ul>"@en;
  skos:prefLabel "appendix d: methods of measurement"@en .

:c_dd03e186 a skos:Concept;
  dc:rights :c_6c82c09f;
  dc:source :c_6c82c09f, :c_ca00c020;
  dct:created "2019-12-15T07:13:02.940Z"^^xsd:dateTime;
  dct:modified "2020-10-28T15:16:00.585Z"^^xsd:dateTime;
  skos:broader :c_13911a49;
  skos:definition "A room used, or intended to be used, for people to live in (including, for the purposes of Approved Document B Volumes 1 and 2, a kitchen, but not a bathroom)."@en;
  skos:inScheme :conceptScheme_751925ed;
  skos:prefLabel "habitable room"@en-GB .

:c_d8e990c2 a skos:Concept;
  dc:rights :c_6c82c09f;
  dc:source :c_6c82c09f, :c_ca00c020;
  dct:created "2019-12-15T07:14:31.932Z"^^xsd:dateTime;
  dct:modified "2019-12-15T07:58:00.018Z"^^xsd:dateTime;
  rdfs:seeAlso :c_c1a78f4b, :c_cc92c6ff;
  skos:broader :c_13911a49;
  skos:definition """(of a building or storey for the purposes of Approved Document B Volumes 1 and 2) 
<ul><li>Height of a building is measured as shown in Appendix D, Diagram D4. 
<li>Height of the floor of the top storey above ground level is measured as shown in Appendix D, Diagram D6.</ul>"""@en;
  skos:inScheme :conceptScheme_751925ed;
  skos:prefLabel "height"@en .

:c_cc92c6ff a skos:Concept;
  dc:source :c_6c82c09f, :c_ca00c020;
  dct:created "2019-12-15T07:24:50.211Z"^^xsd:dateTime;
  dct:modified "2019-12-21T06:53:31.807Z"^^xsd:dateTime;
  skos:broader :c_4f2b64be;
  skos:inScheme :conceptScheme_751925ed;
  skos:prefLabel "diagram d4 height of building"@en .

:c_45ef22f5 a skos:Concept;
  dc:source :c_6c82c09f, :c_ca00c020;
  dct:created "2019-12-15T07:40:59.818Z"^^xsd:dateTime;
  dct:modified "2019-12-21T06:41:36.318Z"^^xsd:dateTime;
  skos:broader :c_4f2b64be;
  skos:inScheme :conceptScheme_751925ed;
  skos:note "<ul><li>a. cubic capacity of a building<li>b. Cubic capacity of compartments or separated part of a building</ul>"@en;
  skos:prefLabel "diagram d2 cubic capacity"@en .

:c_be34e7b3 a skos:Concept;
  dc:source :c_ca00c020;
  dct:created "2019-12-15T07:42:05.586Z"^^xsd:dateTime;
  dct:modified "2019-12-21T06:53:31.745Z"^^xsd:dateTime;
  skos:broader :c_4f2b64be;
  skos:inScheme :conceptScheme_751925ed;
  skos:note """<ul><li>a. Surface area: roofs and rooflights
In each case measure the visible area<li>b. Floor area:Room, garage, conservatory or outbuilding,measure to inner surface of enclosing walls<li>c. Floor area:Storey, part or compartment measure to inner surface of enclosing walls and include internal walls and partitions</ul>"""@en;
  skos:prefLabel "diagram d3 area"@en .

:c_8d791a67 a skos:Concept;
  dc:source :c_6c82c09f, :c_ca00c020;
  dct:created "2019-12-15T07:49:01.790Z"^^xsd:dateTime;
  dct:modified "2019-12-21T06:53:31.869Z"^^xsd:dateTime;
  skos:broader :c_4f2b64be;
  skos:inScheme :conceptScheme_751925ed;
  skos:note "NOTES:<ul><li>1. In assembly buildings (purpose group 5), a galleryis included as a storey, but not if it is a loading gallery, fly gallery, stage grid, lighting bridge, or any gallery provided for similar purposes, or for maintenance and repair<li>.2. In other purpose group buildings, galleries are not counted as a storey.<li>3.For the definition of basement, see Appendix A</ul>"@en;
  skos:prefLabel "diagram d5 number of storeys"@en .

:c_c1a78f4b a skos:Concept;
  dc:source :c_ca00c020;
  dct:created "2019-12-15T07:52:39.429Z"^^xsd:dateTime;
  dct:modified "2019-12-21T06:42:53.312Z"^^xsd:dateTime;
  skos:broader :c_4f2b64be;
  skos:inScheme :conceptScheme_751925ed;
  skos:prefLabel "diagram d6 height of top storey in building"@en .

:c_13911a49 dct:modified "2020-10-28T14:51:06.504Z"^^xsd:dateTime .

:c_7d862abe dct:modified "2019-12-21T06:40:53.066Z"^^xsd:dateTime .

:c_ca00c020 skos:narrower :c_4f2b64be .

:c_056e5a0a a skos:Concept;
  skos:broader :c_13911a49;
  skos:inScheme :conceptScheme_751925ed;
  skos:prefLabel "inner room"@en .

:c_ab93123b a skos:Concept;
  dct:created "2020-10-14T06:46:05.796Z"^^xsd:dateTime;
  skos:broader :c_f9b32acf;
  skos:inScheme :conceptScheme_751925ed;
  skos:prefLabel "materials and workmanship"@en .

:c_81ea9f13 a skos:Concept;
  dct:created "2020-10-14T06:48:21.650Z"^^xsd:dateTime;
  dct:modified "2020-10-26T07:25:25.914Z"^^xsd:dateTime;
  skos:broader :c_ab93123b;
  skos:inScheme :conceptScheme_751925ed .

:c_3bb1b1d6 a skos:Concept;
  dct:created "2020-10-14T06:48:55.431Z"^^xsd:dateTime;
  dct:modified "2020-10-14T06:51:57.561Z"^^xsd:dateTime;
  skos:broader :c_81ea9f13;
  skos:definition """The British Standards Institution is the UK national
standards body. BSI publishes European standards
in the UK as BS EN. Further information is available
at: www.bsigroup.co.uk """@en;
  skos:inScheme :conceptScheme_751925ed;
  skos:prefLabel "bsi"@en .

:c_3da44764 skos:narrower :c_2689a172, :c_3454d214, :c_366cf430, :c_8883ce73, :c_9243074f,
    :c_d996e4f9, :c_da4c39b1 .

:c_a86611c3 a skos:Concept;
  dct:created "2020-10-14T06:58:19.971Z"^^xsd:dateTime;
  dct:modified "2020-10-16T17:01:59.623Z"^^xsd:dateTime;
  skos:broader :c_12c47f28;
  skos:definition """The following meanings apply to terms
throughout this section:"""@en;
  skos:inScheme :conceptScheme_751925ed;
  skos:notation "2.3"@en;
  skos:prefLabel "definitions (ada)"@en .

:c_e943b612 a skos:Concept;
  dct:created "2020-10-16T16:35:40.410Z"^^xsd:dateTime;
  dct:modified "2020-10-16T16:39:48.540Z"^^xsd:dateTime;
  skos:broader :c_a86611c3;
  skos:definition """A wall designed and
constructed to afford lateral support to another
wall perpendicular to it, support being provided
from the base to the top of the wall."""@en;
  skos:inScheme :conceptScheme_751925ed;
  skos:prefLabel "buttressing wall"@en .

:c_12c47f28 a skos:Concept;
  dct:created "2020-10-16T16:31:14.686Z"^^xsd:dateTime;
  dct:modified "2020-10-25T05:32:03.824Z"^^xsd:dateTime;
  skos:broader :c_1b060096;
  skos:inScheme :conceptScheme_751925ed;
  skos:prefLabel "structure 2004 edition incorporating 2004,2010 and 2013 amendments"@en .

:c_4e975ede a skos:Concept;
  dct:created "2020-10-16T16:59:05.253Z"^^xsd:dateTime;
  skos:broader :c_e186f594;
  skos:definition """This document is one of a series that has been
approved by the First Secretary of State for the
purpose of providing practical guidance with
respect to the requirements of Schedule 1 to and
Regulation 7 of the Building Regulations 2010 (SI
2010/2214) for England and Wales."""@en;
  skos:inScheme :conceptScheme_751925ed;
  skos:prefLabel "site preparation and resistance to contaminants and moisture 2004 edition incorporating 2010 and 2013 amendments"@en .

:c_db47eea3 a skos:Concept;
  dct:created "2020-10-16T16:41:44.186Z"^^xsd:dateTime;
  dct:modified "2020-10-16T16:42:21.594Z"^^xsd:dateTime;
  skos:broader :c_a86611c3;
  skos:definition """The load assumed to be produced
by the intended occupancy or use, including
the weight of movable partitions, distributed,
concentrated, impact, inertia and snow loads,
but excluding wind loads."""@en;
  skos:inScheme :conceptScheme_751925ed;
  skos:prefLabel "imposed load"@en .

:c_cda2477f a skos:Concept;
  dct:created "2020-10-16T16:40:01.369Z"^^xsd:dateTime;
  dct:modified "2020-10-16T16:42:57.737Z"^^xsd:dateTime;
  skos:broader :c_a86611c3;
  skos:definition """The horizontal distance between
the two leaves of a cavity wall."""@en;
  skos:inScheme :conceptScheme_751925ed;
  skos:prefLabel "cavity width"@en .

:c_054f5d4e a skos:Concept;
  dct:created "2020-10-16T16:40:35.037Z"^^xsd:dateTime;
  dct:modified "2020-10-16T16:42:48.002Z"^^xsd:dateTime;
  skos:broader :c_a86611c3;
  skos:definition """A wall constructed as a
compartment wall to meet the requirements of
regulation B3(2)."""@en;
  skos:inScheme :conceptScheme_751925ed;
  skos:prefLabel "compartment wall"@en .

:c_25dbe396 a skos:Concept;
  dct:created "2020-10-16T16:41:12.480Z"^^xsd:dateTime;
  dct:modified "2020-10-16T16:42:35.513Z"^^xsd:dateTime;
  skos:broader :c_a86611c3;
  skos:definition """The load due to the weight of
all walls, permanent partitions, floors, roofs
and finishes including services, and all other
permanent construction."""@en;
  skos:inScheme :conceptScheme_751925ed;
  skos:prefLabel "dead load"@en .

:c_d44ed148 a skos:Concept;
  dct:created "2020-10-16T16:43:29.330Z"^^xsd:dateTime;
  dct:modified "2020-10-16T16:43:49.605Z"^^xsd:dateTime;
  skos:broader :c_a86611c3;
  skos:definition """A member which forms an integral part
of a wall, in the form of a thickened section at
intervals along the wall, so as to afford lateral
support to the wall to which it is bonded or
securely tied."""@en;
  skos:inScheme :conceptScheme_751925ed;
  skos:prefLabel "pier"@en .

:c_5fea650b a skos:Concept;
  dct:created "2020-10-16T16:44:07.193Z"^^xsd:dateTime;
  dct:modified "2020-10-16T16:44:28.367Z"^^xsd:dateTime;
  skos:broader :c_a86611c3;
  skos:definition """A wall or part of a wall which is
common to adjoining buildings, and constructed
to meet the requirements of regulation B3(2)."""@en;
  skos:inScheme :conceptScheme_751925ed;
  skos:prefLabel "separating wall"@en .

:c_48a520f8 a skos:Concept;
  dct:created "2020-10-16T16:44:39.652Z"^^xsd:dateTime;
  dct:modified "2020-10-16T16:45:12.189Z"^^xsd:dateTime;
  skos:broader :c_a86611c3;
  skos:definition """The distance between the longitudinal
centres of any two adjacent timber members of
the same type, measured in the plane of floor,
ceiling or roof structure."""@en;
  skos:inScheme :conceptScheme_751925ed;
  skos:prefLabel "spacing"@en .

:c_d54c6174 a skos:Concept;
  dct:created "2020-10-16T16:45:44.754Z"^^xsd:dateTime;
  dct:modified "2020-10-16T16:46:12.785Z"^^xsd:dateTime;
  skos:broader :c_a86611c3;
  skos:definition """The distance measured along the centre
line of a member between the centres of any two
adjacent bearings or supports."""@en;
  skos:inScheme :conceptScheme_751925ed;
  skos:prefLabel "span"@en .

:c_778ca063 a skos:Concept;
  dct:created "2020-10-16T16:46:30.436Z"^^xsd:dateTime;
  dct:modified "2020-10-16T16:47:04.924Z"^^xsd:dateTime;
  skos:broader :c_a86611c3;
  skos:definition """A wall to which lateral support is
afforded by a combination of buttressing walls,
piers or chimneys acting in conjunction with
floor(s) or roof."""@en;
  skos:inScheme :conceptScheme_751925ed;
  skos:prefLabel "supported wall"@en .

:c_ce403f47 a skos:Concept;
  dct:created "2020-10-16T16:47:37.008Z"^^xsd:dateTime;
  dct:modified "2020-10-16T16:48:47.813Z"^^xsd:dateTime;
  skos:broader :c_a86611c3;
  skos:definition """The load due to the effect of wind
pressure or suction."""@en;
  skos:inScheme :conceptScheme_751925ed;
  skos:prefLabel "wind load"@en .

:c_90aedbdc skos:narrower :c_0cdb0b97, :c_1aa022f8 .

:c_42d467db dct:modified "2020-10-25T05:18:33.206Z"^^xsd:dateTime;
  skos:narrower :c_679215e0 .

:c_597ee1e5 a skos:Concept;
  dct:created "2020-10-16T17:01:23.399Z"^^xsd:dateTime;
  dct:modified "2020-10-16T17:03:42.971Z"^^xsd:dateTime;
  skos:broader :c_4e975ede;
  skos:definition """The following meanings apply to terms
throughout this Approved Document:"""@en;
  skos:inScheme :conceptScheme_751925ed;
  skos:notation "0.12"@en;
  skos:prefLabel "definitions (adc)"@en .

:c_2618c4b3 a skos:Concept;
  dct:created "2020-10-16T17:04:51.739Z"^^xsd:dateTime;
  dct:modified "2020-10-16T17:05:21.774Z"^^xsd:dateTime;
  skos:broader :c_597ee1e5;
  skos:definition """Any substance13 which is or
may become harmful to persons or buildings,
including substances which are corrosive,
explosive, flammable, radioactive or toxic."""@en;
  skos:inScheme :conceptScheme_751925ed;
  skos:prefLabel "contaminant"@en .

:c_43d8f455 a skos:Concept;
  dct:created "2020-10-16T17:04:03.527Z"^^xsd:dateTime;
  dct:modified "2020-10-16T17:04:34.252Z"^^xsd:dateTime;
  skos:broader :c_597ee1e5;
  skos:definition """The building and all the land forming the site
subject to building operations which includes
land under the building and the land around it
which may have an effect on the building or its
users (see also paragraph 2.11)."""@en;
  skos:inScheme :conceptScheme_751925ed;
  skos:prefLabel "building and land associated with the building"@en .

:c_f5ae3ea1 a skos:Concept;
  dct:created "2020-10-16T17:05:42.497Z"^^xsd:dateTime;
  dct:modified "2020-10-16T17:06:10.910Z"^^xsd:dateTime;
  skos:broader :c_597ee1e5;
  skos:definition """Lower horizontal surface of any space in a
building including finishes that are laid as part of
the permanent construction."""@en;
  skos:inScheme :conceptScheme_751925ed;
  skos:prefLabel "floor"@en .

:c_3afc08f0 a skos:Concept;
  dct:created "2020-10-16T17:06:31.015Z"^^xsd:dateTime;
  dct:modified "2020-10-16T17:06:53.217Z"^^xsd:dateTime;
  skos:broader :c_597ee1e5;
  skos:definition """Water in liquid form, either as a
static water table or flowing through the ground."""@en;
  skos:inScheme :conceptScheme_751925ed;
  skos:prefLabel "groundwater"@en .

:c_586c25b3 a skos:Concept;
  dct:created "2020-10-16T17:07:11.530Z"^^xsd:dateTime;
  dct:modified "2020-10-16T17:07:34.990Z"^^xsd:dateTime;
  skos:broader :c_597ee1e5;
  skos:definition """Deposition of liquid
water from a vapour, occurring within or between
the layers of the building envelope."""@en;
  skos:inScheme :conceptScheme_751925ed;
  skos:prefLabel "interstitial condensation"@en .

:c_3736f311 a skos:Concept;
  dct:created "2020-10-16T17:07:50.007Z"^^xsd:dateTime;
  dct:modified "2020-10-16T17:08:13.940Z"^^xsd:dateTime;
  skos:broader :c_597ee1e5;
  skos:definition "Water in liquid, solid or gaseous form."@en;
  skos:inScheme :conceptScheme_751925ed;
  skos:prefLabel "moisture"@en .

:c_0c23af6b a skos:Concept;
  dct:created "2020-10-16T17:08:32.985Z"^^xsd:dateTime;
  dct:modified "2020-10-16T17:09:03.826Z"^^xsd:dateTime;
  skos:broader :c_597ee1e5;
  skos:definition """Moisture in any form falling from the
atmosphere, usually as rain, sleet, snow or hail."""@en;
  skos:inScheme :conceptScheme_751925ed;
  skos:prefLabel "precipitation"@en .

:c_774ecfdd a skos:Concept;
  dct:created "2020-10-16T17:09:21.752Z"^^xsd:dateTime;
  dct:modified "2020-10-16T17:10:04.522Z"^^xsd:dateTime;
  skos:broader :c_597ee1e5;
  skos:definition """Any part of the external envelope of a
building that is at an angle of less than 70° to
the horizontal."""@en;
  skos:inScheme :conceptScheme_751925ed;
  skos:prefLabel "roof"@en .

:c_040286d4 a skos:Concept;
  dct:created "2020-10-16T17:10:21.683Z"^^xsd:dateTime;
  dct:modified "2020-10-16T17:10:41.886Z"^^xsd:dateTime;
  skos:broader :c_597ee1e5;
  skos:definition """Water droplets driven by the wind from the
surface of the sea or other bodies of water adjacent
to buildings. Sea spray can be especially hazardous
to materials because of its salt content."""@en;
  skos:inScheme :conceptScheme_751925ed;
  skos:prefLabel "spray"@en .

:c_90ae9da8 a skos:Concept;
  dct:created "2020-10-16T17:10:59.392Z"^^xsd:dateTime;
  dct:modified "2020-10-16T17:11:23.669Z"^^xsd:dateTime;
  skos:broader :c_597ee1e5;
  skos:definition """Deposition of liquid
water from a vapour, occurring on visible
surfaces within the building."""@en;
  skos:inScheme :conceptScheme_751925ed;
  skos:prefLabel "surface condensation"@en .

:c_12c07b97 a skos:Concept;
  dct:created "2020-10-16T17:11:40.167Z"^^xsd:dateTime;
  dct:modified "2020-10-16T17:12:07.999Z"^^xsd:dateTime;
  skos:broader :c_597ee1e5;
  skos:definition """Material of construction,
usually a membrane, that substantially reduces
the water vapour transfer through any building in
which it is incorporated."""@en;
  skos:inScheme :conceptScheme_751925ed;
  skos:prefLabel "vapour control layer"@en .

:c_b7704238 a skos:Concept;
  dct:created "2020-10-16T17:12:23.157Z"^^xsd:dateTime;
  dct:modified "2020-10-16T17:12:41.379Z"^^xsd:dateTime;
  skos:broader :c_597ee1e5;
  skos:definition """Any opaque part of the external envelope
of a building that is at an angle of 70° or more to
the horizontal."""@en;
  skos:inScheme :conceptScheme_751925ed;
  skos:prefLabel "wall"@en .

:c_f6ff7c1c a skos:Concept;
  dct:created "2020-10-17T06:18:31.390Z"^^xsd:dateTime;
  skos:broader :c_8cba3c82;
  skos:inScheme :conceptScheme_751925ed;
  skos:prefLabel "toxic substances 1992 edition incorporating 2002, 2010 and 2013 amendments"@en .

:c_586b08a2 a skos:Concept;
  dct:created "2020-10-17T06:22:58.683Z"^^xsd:dateTime;
  dct:modified "2020-10-17T06:24:13.204Z"^^xsd:dateTime;
  skos:broader :c_1a6e1e92;
  skos:definition """* This Approved Document gives guidance for
compliance with the Building Regulations for
building work carried out in England. It also
applies to building work carried out on excepted
energy buildings in Wales as defined in the Welsh
Ministers (Transfer of Functions)(No 2) Order 2009."""@en;
  skos:inScheme :conceptScheme_751925ed;
  skos:prefLabel "resistance to the passage of sound 2003 edition incorporating 2004, 2010, 2013 and 2015 amendments"@en .

:c_f4cc0ec3 a skos:Concept;
  dct:created "2020-10-17T06:26:16.079Z"^^xsd:dateTime;
  skos:broader :c_586b08a2;
  skos:definition """The definitions given below are for the purposes of this document only, and are not intended to
be rigorous. Fuller definitions of the various
acoustical terms are to be found in the relevant British Standards listed in Annex D."""@en;
  skos:inScheme :conceptScheme_751925ed;
  skos:prefLabel "annex c: glossary"@en .

:c_4b4c9739 dct:modified "2020-10-24T20:01:47.685Z"^^xsd:dateTime .

:c_59a3ae21 skos:narrower :c_0319d3fa, :c_03fe243e, :c_2842eb4b, :c_3f23e147, :c_485cf2fc,
    :c_54dcd677, :c_62cc4d78, :c_76c8b363, :c_7cf13722, :c_7cf2b5eb, :c_a8de44e3, :c_c07e16c5,
    :c_dd64e423, :c_eb6a5187, :c_f3c590e2, :c_fc7ec0c8 .

:c_4d4c50dd skos:inScheme :conceptScheme_751925ed;
  skos:prefLabel "infiltration"@en .

:c_a8de44e3 dct:modified "2020-10-24T19:09:33.148Z"^^xsd:dateTime .

:c_1fa348f3 a skos:Concept;
  dct:created "2020-10-19T19:02:43.189Z"^^xsd:dateTime;
  skos:broader :c_58df2af5;
  skos:inScheme :conceptScheme_751925ed;
  skos:prefLabel "a1 loading"@en .

:c_34ab31dc a skos:Concept;
  dct:created "2020-10-19T19:02:59.575Z"^^xsd:dateTime;
  skos:broader :c_58df2af5;
  skos:inScheme :conceptScheme_751925ed;
  skos:prefLabel "a2 ground movement"@en .

:c_56aca7cf a skos:Concept;
  dct:created "2020-10-19T19:03:45.481Z"^^xsd:dateTime;
  skos:broader :c_58df2af5;
  skos:inScheme :conceptScheme_751925ed;
  skos:prefLabel "a3 disproportionate collapse"@en .

:c_bd26d581 a skos:Concept;
  dct:created "2020-10-19T19:04:13.948Z"^^xsd:dateTime;
  skos:broader :c_58df2af5;
  skos:inScheme :conceptScheme_751925ed;
  skos:prefLabel "b1 means of waring and escape"@en .

:c_926affad a skos:Concept;
  dct:created "2020-10-19T19:04:58.189Z"^^xsd:dateTime;
  skos:broader :c_58df2af5;
  skos:inScheme :conceptScheme_751925ed;
  skos:prefLabel "b2 internal fire spread linings"@en .

:c_d7714b03 a skos:Concept;
  dct:created "2020-10-19T19:05:20.709Z"^^xsd:dateTime;
  skos:broader :c_58df2af5;
  skos:inScheme :conceptScheme_751925ed;
  skos:prefLabel "b3 internal fire spread structure"@en .

:c_95a5e382 a skos:Concept;
  dct:created "2020-10-19T19:05:41.132Z"^^xsd:dateTime;
  skos:broader :c_58df2af5;
  skos:inScheme :conceptScheme_751925ed;
  skos:prefLabel "b4 external fire spread"@en .

:c_419da0ad a skos:Concept;
  dct:created "2020-10-19T19:06:06.820Z"^^xsd:dateTime;
  skos:broader :c_58df2af5;
  skos:inScheme :conceptScheme_751925ed;
  skos:prefLabel "b5 access and facilities for the fire service"@en .

:c_9d708081 a skos:Concept;
  dct:created "2020-10-19T19:07:46.203Z"^^xsd:dateTime;
  skos:broader :c_f9b32acf;
  skos:inScheme :conceptScheme_751925ed;
  skos:prefLabel "regulation 38 fire safety information"@en .

:c_58df2af5 dct:modified "2020-10-19T19:20:11.959Z"^^xsd:dateTime;
  skos:narrower :c_1fa348f3, :c_34ab31dc, :c_419da0ad, :c_926affad, :c_95a5e382, :c_bd26d581,
    :c_d7714b03 .

:c_86cfaae6 dct:modified "2020-10-23T16:52:59.669Z"^^xsd:dateTime;
  skos:narrower :c_58df2af5, :c_f232ec50 .

:c_f9b32acf dct:modified "2020-10-28T14:47:43.550Z"^^xsd:dateTime;
  skos:narrower :c_06f29df7, :c_37246cae, :c_9d708081 .

:c_feba40b2 a skos:Concept;
  skos:broader :c_37246cae;
  skos:definition """as a file appropriate to the characteristics of
the project, containing relevant health and safety information to be taken into
account during any subsequent project"""@en;
  skos:inScheme :conceptScheme_751925ed;
  skos:prefLabel "appendix 4 the health and safety file"@en .

:skosCollection_50d4bd2e a skos:Collection;
  dct:created "2020-10-23T17:24:32.699Z"^^xsd:dateTime;
  skos:member :c_040286d4, :c_04c52352, :c_054f5d4e, :c_056e5a0a, :c_0c23af6b, :c_10030a9a,
    :c_10ea4ecc, :c_12c07b97, :c_132d79ca, :c_13543964, :c_14b52896, :c_1a7ea9e5, :c_1f1f7725,
    :c_228ee3b0, :c_25dbe396, :c_2618c4b3, :c_28013078, :c_28e7c922, :c_33c0e1b5, :c_3454d214,
    :c_34f295d5, :c_35d3a535, :c_362390fa, :c_3736f311, :c_38ba0f99, :c_3afc08f0, :c_3cae7829,
    :c_3d59dac9, :c_3e5063e6, :c_40560ccd, :c_43d8f455, :c_46be855e, :c_47c790ae, :c_48a520f8,
    :c_49a5a923, :c_4a90e0e1, :c_4aee7770, :c_4cb80404, :c_56fef4b5, :c_5724a233, :c_586c25b3,
    :c_5ef03467, :c_5fea650b, :c_61f82d61, :c_6284471b, :c_706598d3, :c_727adfdb, :c_7400b440,
    :c_774ecfdd, :c_778ca063, :c_7804ad6c, :c_79a3679f, :c_7a2d826e, :c_7b85eda3, :c_7c12f560,
    :c_7d862abe, :c_7e4da283, :c_7fc5469b, :c_8258611b, :c_83464c52, :c_858351ef, :c_88af4873,
    :c_90ae9da8, :c_9a0f5e20, :c_9b7f9eb7, :c_9e4931f7, :c_9e8d26ab, :c_a4eaf123, :c_a965ecce,
    :c_ad9a7d0c, :c_b0f3b4fb, :c_b2cab8d9, :c_b304ed8a, :c_b3f65603, :c_b44f46e0, :c_b4ccd5f2,
    :c_b6083e42, :c_b67f0d40, :c_b7704238, :c_b975b2d2, :c_b980c88c, :c_b98dbf2a, :c_bed063fd,
    :c_c02d4d7d, :c_c8b52d92, :c_c916e597, :c_cb3d4c10, :c_cb86c2ff, :c_cc61a0f4, :c_cd2ba206,
    :c_cda2477f, :c_ce403f47, :c_d32d8045, :c_d44ed148, :c_d54c6174, :c_d5c15327, :c_d8e990c2,
    :c_da6168d8, :c_db47eea3, :c_dd03e186, :c_e7e6b110, :c_e943b612, :c_ee10273a, :c_f12e46ec,
    :c_f4139893, :c_f5536b7d, :c_f5ae3ea1, :c_f636fce4, :c_f70bb786;
  skos:prefLabel "building regulation key terms"@en .

:c_37246cae a skos:Concept;
  dct:created "2020-10-23T16:58:55.740Z"^^xsd:dateTime;
  skos:inScheme :conceptScheme_751925ed;
  skos:narrower :c_feba40b2;
  skos:prefLabel "construction (design and management) regulations 2015"@en .

:c_0109c085 skos:broader :c_502a871c .

:c_06f29df7 dct:modified "2020-10-19T19:27:13.760Z"^^xsd:dateTime;
  skos:broader :c_f9b32acf .

:c_f232ec50 a skos:Concept;
  dct:created "2020-10-23T16:52:46.611Z"^^xsd:dateTime;
  dct:modified "2020-10-23T16:54:33.453Z"^^xsd:dateTime;
  skos:broader :c_86cfaae6;
  skos:inScheme :conceptScheme_751925ed;
  skos:narrower :c_16a278c8;
  skos:prefLabel "part 8"@en .

:c_16a278c8 a skos:Concept;
  dct:created "2020-10-23T16:53:14.729Z"^^xsd:dateTime;
  skos:broader :c_f232ec50;
  skos:inScheme :conceptScheme_751925ed;
  skos:prefLabel "fire safety information"@en .

:c_502a871c skos:narrower :c_1a6e1e92, :c_1b060096, :c_2a34c0b8, :c_2ca1576c, :c_42d467db,
    :c_5ffbc967, :c_73c4361e, :c_8cba3c82, :c_a20cbb62, :c_b7bccf3d, :c_be604dfa, :c_d4480e31,
    :c_e186f594, :c_f68328a2, :c_fec1533e .

:c_63df1a7b a skos:Concept;
  skos:broader :c_59a3ae21;
  skos:definition " (general ventilation) is nominally continuous ventilation of rooms or spaces at a relatively low rate to dilute and remove pollutants and water vapour not removed by operation of extract ventilation, purge ventilation or infiltration, as well as supplying outdoor air into the building. For an individual dwelling this is referred to as ‘whole dwelling ventilation’."@en;
  skos:inScheme :conceptScheme_751925ed;
  skos:prefLabel "whole building ventilation"@en .

:c_eb6a5187 a skos:Concept;
  dct:modified "2020-10-26T07:32:32.754Z"^^xsd:dateTime;
  skos:broader :c_59a3ae21;
  skos:definition "is where a mechanical ventilator does not run all the time, usually running only when there is a particular need to remove pollutants or water vapour (e.g. during cooking or bathing). Intermittent operation may be under either manual control or automatic control."@en;
  skos:inScheme :conceptScheme_751925ed;
  skos:prefLabel "intermittent operation"@en .

:c_373d0f37 skos:broader :c_59a3ae21;
  skos:inScheme :conceptScheme_751925ed .

:c_8dc8a4f6 a skos:Concept;
  skos:broader :c_59a3ae21;
  skos:definition "is a room containing a bath or shower and, in addition, can also include sanitary accommodation."@en;
  skos:inScheme :conceptScheme_751925ed .

:c_dd64e423 a skos:Concept;
  skos:broader :c_59a3ae21;
  skos:definition "is a space where large numbers of people are expected to gather, such as a shopping mall or cinema/theatre foyer. For the purposes of this Approved Document, a space used solely or principally for circulation (e.g. a corridor or lift lobby in an office building or blocks of flats) is not a common space."@en .

:c_7cf2b5eb skos:inScheme :conceptScheme_751925ed;
  skos:prefLabel "purge ventilation"@en .

:c_eeea044b dct:modified "2020-10-26T07:31:36.088Z"^^xsd:dateTime;
  skos:broader :c_59a3ae21;
  skos:prefLabel "bcb or building control body"@en .

:c_54dcd677 a skos:Concept;
  skos:broader :c_59a3ae21;
  skos:definition "is a measure of the aerodynamic performance of a ventilator. It is the area of a sharp-edged circular orifice which air would pass through at the same volume flow rate, under an identical applied pressure difference, as the opening under consideration."@en;
  skos:inScheme :conceptScheme_751925ed;
  skos:prefLabel "cquivalent area"@en .

:c_62cc4d78 a skos:Concept;
  dct:modified "2020-10-26T07:28:48.195Z"^^xsd:dateTime;
  skos:definition "is a ventilation opening which may be opened and closed under either manual or automatic control."@en;
  skos:inScheme :conceptScheme_751925ed;
  skos:prefLabel "closable opening"@en .

:c_0319d3fa a skos:Concept;
  dct:modified "2020-10-26T07:23:20.238Z"^^xsd:dateTime;
  skos:definition "is where a ventilation device is opened and closed, or switched on and off, or its performance is adjusted by the occupants of a room or building (see automatic control)."@en;
  skos:inScheme :conceptScheme_751925ed;
  skos:prefLabel "manual control"@en .

:c_15104e5f skos:broader :c_59a3ae21;
  skos:inScheme :conceptScheme_751925ed;
  skos:prefLabel "stack effect"@en .

:c_fc7ec0c8 a skos:Concept;
  skos:broader :c_59a3ae21;
  skos:definition "is a general descriptive term for the resistance of the building envelope to infiltration with ventilators closed. The greater the airtightness at a given pressure difference across the envelope, the lower the infiltration."@en;
  skos:inScheme :conceptScheme_751925ed;
  skos:prefLabel "airtightness"@en .

:c_485cf2fc dct:modified "2020-10-24T19:07:17.093Z"^^xsd:dateTime;
  skos:broader :c_59a3ae21;
  skos:definition "(in relation to dwellings) is a dwelling, or a usable part of a dwelling (i.e. a habitable room), that is situated partly or entirely below ground level. Note that a cellar is distinct from a basement in that it is used only for storage, heating plant or purposes other than habitation."@en;
  skos:inScheme :conceptScheme_751925ed;
  skos:prefLabel "basement"@en .

:c_830012c2 a skos:Concept;
  dct:modified "2020-10-24T19:07:36.414Z"^^xsd:dateTime;
  skos:definition "is a part of a dwelling which is situated partly or entirely below ground level, and is distinct from a basement in that it is used only for storage, heating plant or purposes other than habitation."@en;
  skos:inScheme :conceptScheme_751925ed .

:c_3f23e147 skos:broader :c_59a3ae21;
  skos:definition "is a ventilation system using ducts from terminals in the ceiling of rooms to terminals on the roof that extract air to outside by a combination of the natural stack effect and the pressure effects of wind passing over the roof of the building."@en;
  skos:inScheme :conceptScheme_751925ed;
  skos:prefLabel "passive stack ventilation (psv)"@en .

:c_7cf13722 a skos:Concept;
  skos:broader :c_59a3ae21;
  skos:definition "is a room in a building other than a dwelling that is occupied by people, such as an office, workroom, classroom or hotel bedroom, but not a bathroom, sanitary accommodation, utility room or rooms or spaces used solely or principally for circulation, building services plant or storage purposes."@en;
  skos:inScheme :conceptScheme_751925ed;
  skos:prefLabel "occupiable room"@en .

:c_9b5f7333 a skos:Concept;
  skos:broader :c_59a3ae21;
  skos:definition "is any means of purpose- provided ventilation (whether it is permanent or closable) which opens directly to external air, such as the openable parts of a window, a louvre or a background ventilator. It also includes any door which opens directly to external air."@en;
  skos:inScheme :conceptScheme_751925ed;
  skos:prefLabel "ventilation opening"@en .

:c_ac856c1e a skos:Concept;
  skos:broader :c_59a3ae21;
  skos:definition "is the physical property used to measure the airtightness of the building fabric. It is defined as air leakage rate per hour per square metre of envelope area at a test reference pressure differential across the building envelope of 50 Pascal (50 N/m2). The design air permeability is the target value set at the design stage."@en;
  skos:inScheme :conceptScheme_751925ed;
  skos:prefLabel "air permeability"@en-GB .

:c_e7b31cc5 a skos:Concept;
  dct:modified "2020-10-26T07:36:15.983Z"^^xsd:dateTime;
  skos:broader :c_59a3ae21;
  skos:definition "is a room used for domestic activities (such as cooking, clothes washing and bathing) which give rise to significant production of airborne moisture, e.g. a kitchen, utility room or bathroom. For the purposes of Part F, sanitary accommodation is also regarded as a wet room."@en;
  skos:inScheme :conceptScheme_751925ed;
  skos:prefLabel "wet room"@en .

:c_59a3ae21 a skos:Concept;
  dct:created "2020-10-24T18:42:24.065Z"^^xsd:dateTime;
  skos:definition """The following are key terms used in this
document:"""@en;
  skos:inScheme :conceptScheme_751925ed;
  skos:narrower :c_15104e5f, :c_32d39119, :c_373d0f37, :c_4fe84b3b, :c_63df1a7b, :c_67f6207e,
    :c_8dc8a4f6, :c_92db7c07, :c_9b5f7333, :c_ac856c1e, :c_d10595f3, :c_e7b31cc5;
  skos:notation "3.1"@en;
  skos:prefLabel "key terms (adf)"@en .

:c_90aedbdc skos:narrower :c_e2afc611 .

:c_92db7c07 a skos:Concept;
  dct:modified "2020-10-26T07:20:25.585Z"^^xsd:dateTime;
  skos:broader :c_59a3ae21;
  skos:definition "is a measure of the availability of water to micro-organisms, and is determined from the ratio of the vapour pressure of the water in the substrate to that of pure water at the same temperature and pressure. This ratio is, in steady-state conditions, numerically equal to the equilibrium relative humidity of the air, except that the latter is commonly expressed as a percentage (from IEA Annex 14 source book, 1991)."@en;
  skos:inScheme :conceptScheme_751925ed;
  skos:prefLabel "surface water activity"@en .

:c_67f6207e a skos:Concept;
  dct:modified "2020-10-26T07:24:36.849Z"^^xsd:dateTime;
  skos:broader :c_59a3ae21;
  skos:definition "is a room containing a sink or other feature or equipment which may reasonably be expected to produce water vapour in significant quantities."@en;
  skos:inScheme :conceptScheme_751925ed;
  skos:prefLabel "utility room"@en .

:c_f3c590e2 a skos:Concept;
  dct:modified "2020-10-26T07:40:01.575Z"^^xsd:dateTime;
  skos:broader :c_59a3ae21;
  skos:definition "is a small ventilation opening designed to provide controllable whole building ventilation. See Diagram 1."@en;
  skos:inScheme :conceptScheme_751925ed;
  skos:prefLabel "background ventilator"@en .

:c_32d39119 a skos:Concept;
  dct:modified "2020-10-26T07:38:12.648Z"^^xsd:dateTime;
  skos:broader :c_59a3ae21;
  skos:definition "is that part of the ventilation of a building provided by ventilation devices designed into the building (e.g. via background ventilators, PSV, extract fans, mechanical ventilation or air-conditioning systems)."@en;
  skos:inScheme :conceptScheme_751925ed;
  skos:prefLabel "purpose-provided ventilation"@en .

:c_a8de44e3 a skos:Concept;
  skos:broader :c_59a3ae21;
  skos:definition "which is permanently fixed in the open position."@en;
  skos:inScheme :conceptScheme_751925ed;
  skos:prefLabel "permanent opening is a ventilation opening"@en .

:c_c07e16c5 a skos:Concept;
  dct:modified "2020-10-26T07:39:23.102Z"^^xsd:dateTime;
  skos:broader :c_59a3ae21;
  skos:definition "is the geometric open area of a ventilator."@en .

:c_4d4c50dd a skos:Concept;
  dct:modified "2020-10-26T07:44:14.675Z"^^xsd:dateTime;
  skos:broader :c_59a3ae21;
  skos:definition "is the uncontrolled exchange of air between inside a building and outside through cracks, porosity and other unintentional openings in a building, caused by pressure difference effects of the wind and/or stack effect."@en .

:c_f851b292 a skos:Concept;
  dct:modified "2020-10-26T07:37:24.648Z"^^xsd:dateTime;
  skos:broader :c_59a3ae21;
  skos:definition "is a room used for dwelling purposes but which is not solely a kitchen, utility room, bathroom, cellar or sanitary accommodation."@en;
  skos:inScheme :conceptScheme_751925ed .

:c_76c8b363 a skos:Concept;
  dct:modified "2020-10-26T07:33:24.590Z"^^xsd:dateTime;
  skos:broader :c_59a3ae21;
  skos:definition "is the removal of air directly from a space or spaces to outside. Extract ventilation may be by natural means (e.g. by passive stack ventilation) or by mechanical means (e.g. by an extract fan or central system)."@en .

:c_4fe84b3b a skos:Concept;
  dct:modified "2020-10-26T07:39:36.168Z"^^xsd:dateTime;
  skos:broader :c_59a3ae21;
  skos:definition "is the total internal volume of the heated space, including the volume of all furniture, internal walls, internal floors, etc."@en .

:c_2842eb4b a skos:Concept;
  dct:modified "2020-10-26T07:42:52.163Z"^^xsd:dateTime;
  skos:broader :c_59a3ae21;
  skos:definition "is where a mechanical ventilation device runs all the time, e.g. mechanical extract ventilation (MEV) and mechanical ventilation with heat recovery (MVHR). The air flow rate provided by the mechanical ventilation need not be constant but may be varied, under either manual or automatic control, in response to the demand for pollutant or water vapour removal."@en;
  skos:inScheme :conceptScheme_751925ed;
  skos:prefLabel "continuous operation"@en .

:c_03fe243e a skos:Concept;
  dct:modified "2020-10-26T07:41:29.432Z"^^xsd:dateTime;
  skos:broader :c_59a3ae21;
  skos:definition "is where a ventilation device is opened and closed or switched on and off or its performance is adjusted by a mechanical or electronic controller which responds to a relevant stimulus. That stimulus is usually related to the humidity of the air in a room, pollutant levels (e.g. carbon dioxide concentration in a room), occupancy of the space (e.g. using a passive infra-red motion detector) or pressure difference across the device (e.g. due to the wind outside)."@en;
  skos:inScheme :conceptScheme_751925ed;
  skos:prefLabel "automatic control"@en .

:c_d10595f3 a skos:Concept;
  skos:broader :c_59a3ae21;
  skos:definition "is the supply and removal of air (by natural and/or mechanical means) to and from a space or spaces in a building. It normally comprises a combination of purpose-provided ventilation and infiltration."@en;
  skos:prefLabel "ventilation"@en .

:c_6d6d73cd a skos:Concept;
  skos:inScheme :conceptScheme_751925ed;
  skos:prefLabel "sanitation, hot water safety and water efficiency 2015 edition with 2016 amendments"@en .

:c_373d0f37 a skos:Concept;
  dct:modified "2020-10-28T15:20:10.766Z"^^xsd:dateTime;
  skos:definition "is a space containing one or more water closets or urinals. Sanitary accommodation containing one or more cubicles counts as a single space if there is free circulation of air throughout the space."@en;
  skos:prefLabel "sanitary accommodation"@en-GB .

:c_7cf2b5eb a skos:Concept;
  dct:modified "2020-10-26T07:27:18.364Z"^^xsd:dateTime;
  skos:broader :c_59a3ae21;
  skos:definition "is manually controlled ventilation of rooms or spaces at a relatively high rate to rapidly dilute pollutants and/or water vapour. Purge ventilation may be provided by natural means (e.g. an openable window) or by mechanical means (e.g. a fan)."@en .

:c_dd64e423 dct:modified "2020-10-26T07:37:58.283Z"^^xsd:dateTime;
  skos:inScheme :conceptScheme_751925ed;
  skos:prefLabel "common space"@en .

:c_eeea044b a skos:Concept;
  skos:definition "is a local authority or an approved inspector."@en;
  skos:inScheme :conceptScheme_751925ed .

:c_0319d3fa skos:broader :c_59a3ae21 .

:c_fc7ec0c8 dct:modified "2020-10-24T19:06:57.628Z"^^xsd:dateTime .

:c_54dcd677 dct:modified "2020-10-26T07:29:31.653Z"^^xsd:dateTime .

:c_3f23e147 a skos:Concept;
  dct:modified "2020-10-26T07:36:30.614Z"^^xsd:dateTime .

:c_485cf2fc a skos:Concept .

:c_830012c2 skos:broader :c_59a3ae21;
  skos:prefLabel "cellar"@en .

:c_8dc8a4f6 dct:modified "2020-10-24T19:07:23.555Z"^^xsd:dateTime;
  skos:prefLabel "bathroom"@en .

:c_15104e5f a skos:Concept;
  dct:modified "2020-10-26T07:26:15.736Z"^^xsd:dateTime;
  skos:definition "is the pressure differential between inside and outside a building caused by differences in the density of the air due to an indoor/outdoor temperature difference."@en .

:c_ac856c1e dct:modified "2020-10-28T15:14:31.948Z"^^xsd:dateTime .

:c_63df1a7b dct:modified "2020-10-26T07:20:56.289Z"^^xsd:dateTime .

:c_9b5f7333 dct:modified "2020-10-26T07:22:06.343Z"^^xsd:dateTime .

:c_7cf13722 dct:modified "2020-10-26T07:27:46.498Z"^^xsd:dateTime .

:c_3b5778ee a skos:Concept;
  skos:broader :c_f4cc0ec3;
  skos:definition "Sound insulation that reduces transmission of airborne sound between buildings or parts of buildings."@en;
  skos:prefLabel "airborne sound insulation"@en .

:c_438bd78a a skos:Concept;
  skos:broader :c_f4cc0ec3;
  skos:definition "A direct or indirect air passage from one side of a structure to the other."@en;
  skos:prefLabel "air path"@en .

:c_8144317d a skos:Concept;
  skos:broader :c_f4cc0ec3;
  skos:definition "Process of sealing joints"@en;
  skos:prefLabel "caulking"@en .

:c_0c33e781 a skos:Concept;
  skos:broader :c_f4cc0ec3;
  skos:definition "A proprietary product or material such as mineral wool used to close the gap in a cavity wall."@en;
  skos:prefLabel "cavity stop"@en .

:c_f213d52c a skos:Concept;
  skos:broader :c_f4cc0ec3;
  skos:definition "The correction to a sound insulation quantity (such as DnT,w) to take account of a specific sound spectrum. See BS EN ISO 717-1:1997."@en;
  skos:prefLabel "ctr"@en .

:c_61aec10c a skos:Concept;
  skos:broader :c_f4cc0ec3;
  skos:definition "(See decibel)"@en;
  skos:prefLabel "db"@en .

:c_5bb42f0e a skos:Concept;
  skos:broader :c_f4cc0ec3;
  skos:definition "The unit used for many acoustic quantities to indicate the level with respect to a reference level."@en;
  skos:prefLabel "decibel (dB)"@en .

:c_1166f883 a skos:Concept;
  skos:broader :c_f4cc0ec3;
  skos:definition "Mass per unit volume, expressed in kilograms per cubic metre (kg/m3)."@en;
  skos:prefLabel "density"@en .

:c_e85e2d31 a skos:Concept;
  skos:broader :c_f4cc0ec3;
  skos:definition "The process in which sound that is incident on one side of a building element is radiated by the other side."@en;
  skos:prefLabel "direct transmission"@en .

:c_b3eb4d7b a skos:Concept;
  skos:broader :c_f4cc0ec3;
  skos:definition "The difference in sound level between a pair of rooms, in a stated frequency band, corrected for the reverberation time. See BS EN ISO 140-4:1998."@en;
  skos:prefLabel "dnt"@en .

:c_9a21f5a2 a skos:Concept;
  skos:broader :c_f4cc0ec3;
  skos:definition "A single-number quantity which characterises the airborne sound insulation between rooms. See BS EN ISO 717-1:1997"@en;
  skos:prefLabel "dnt,w"@en .

:c_c57961a6 a skos:Concept;
  skos:broader :c_f4cc0ec3;
  skos:definition "A single-number quantity which characterises the airborne sound insulation between rooms using noise spectrum no. 2 as defined in BS EN ISO 717-1:1997. See BS EN ISO 717-1:1997."@en;
  skos:prefLabel "dnt,w + ctr"@en .

:c_cbfc0947 a skos:Concept;
  skos:broader :c_f4cc0ec3;
  skos:definition "A parameter used to describe the ability of a resilient material or wall tie to transmit vibration. Specimens with high dynamic stiffness (dynamically ‘stiff’) transmit more vibration than specimens with low dynamic stiffness (dynamically ‘soft’). See BS EN 29052-1:1992 for resilient materials. See BRE Information Paper IP 3/01 for wall ties."@en;
  skos:prefLabel "dynamic stiffness"@en .

:c_4cb28fa4 a skos:Concept;
  skos:broader :c_f4cc0ec3;
  skos:definition "Any building element that contributes to sound transmission between rooms in a building that is not a separating floor or separating wall."@en;
  skos:prefLabel "flanking element"@en .

:c_345811e8 a skos:Concept;
  skos:broader :c_f4cc0ec3;
  skos:definition "Sound transmitted between rooms via flanking elements instead of directly through separating elements or along any path other than the direct path."@en;
  skos:prefLabel "flanking transmission"@en .

:c_3262a30a a skos:Concept;
  skos:broader :c_f4cc0ec3;
  skos:definition "A floating floor consists of a floating layer and resilient layer (see also resilient layer and floating layer)."@en;
  skos:prefLabel "floating floor"@en .

:c_4f47aeea a skos:Concept;
  skos:broader :c_f4cc0ec3;
  skos:definition "A surface layer that rests on a resilient layer and is therefore isolated from the base floor and the surrounding walls (see also resilient layer)."@en;
  skos:prefLabel "floating layer"@en .

:c_d68c8ade a skos:Concept;
  skos:broader :c_f4cc0ec3;
  skos:definition "A partition consisting of board or boards connected to both sides of a wood or metal frame."@en;
  skos:prefLabel "framed wall"@en .

:c_8abc2fd9 a skos:Concept;
  skos:broader :c_f4cc0ec3;
  skos:definition "The number of pressure variations (or cycles) per second that gives a sound its distinctive tone. The unit of frequency is the Hertz (Hz)."@en;
  skos:prefLabel "frequency"@en .

:c_f40ac57b a skos:Concept;
  skos:broader :c_f4cc0ec3;
  skos:definition "A continuous range of frequencies between stated upper and lower limits (see also octave band and one-third octave band)."@en;
  skos:prefLabel "frequency band"@en .

:c_aa316632 a skos:Concept;
  skos:broader :c_f4cc0ec3;
  skos:definition "The unit of the frequency of a sound (formerly called cycles per second)."@en;
  skos:prefLabel "hertz (hz)"@en .

:c_c2902dec a skos:Concept;
  skos:broader :c_f4cc0ec3;
  skos:definition "Sound resulting from direct impact on a building element."@en;
  skos:prefLabel "impact sound"@en .

:c_588bf28f a skos:Concept;
  skos:broader :c_f4cc0ec3;
  skos:definition "Sound insulation which reduces impact sound transmission from direct impacts such as footsteps on a building element."@en;
  skos:prefLabel "impact sound insulation"@en .

:c_895306c7 a skos:Concept;
  skos:broader :c_f4cc0ec3;
  skos:definition "A ceiling which is fixed independently of a separating floor or an internal floor (see separating floor and internal floor)."@en;
  skos:prefLabel "independent ceiling"@en .

:c_07abc5c2 a skos:Concept;
  skos:broader :c_f4cc0ec3;
  skos:definition "Any floor that is not a separating floor (see separating floor)."@en;
  skos:prefLabel "internal floor"@en .

:c_c8566bf0 a skos:Concept;
  skos:broader :c_f4cc0ec3;
  skos:definition "A landing between two floors (see also landing)."@en;
  skos:prefLabel "intermediate landing"@en .

:c_3d888dc1 a skos:Concept;
  skos:broader :c_f4cc0ec3;
  skos:definition "Any wall that does not have a separating function."@en;
  skos:prefLabel "internal wall"@en .

:c_70a0403c a skos:Concept;
  skos:broader :c_f4cc0ec3;
  skos:definition "The absence of rigid connections between two or more parts of a structure."@en;
  skos:prefLabel "isolation"@en .

:c_34c7d4e3 a skos:Concept;
  skos:broader :c_f4cc0ec3;
  skos:definition "A platform or part of floor structure at the end of a flight of stairs or ramp."@en;
  skos:prefLabel "landing"@en .

:c_81482951 a skos:Concept;
  dct:modified "2020-10-25T04:25:51.418Z"^^xsd:dateTime;
  skos:broader :c_f4cc0ec3;
  skos:definition "The impact sound pressure level in a stated frequency band, corrected for the reverberation time. See BS EN ISO 140-7:1998."@en;
  skos:inScheme :conceptScheme_751925ed;
  skos:prefLabel "l’nt"@en .

:c_d26ff5d2 a skos:Concept;
  skos:broader :c_f4cc0ec3;
  skos:definition "A single-number quantity used to characterise the impact sound insulation of floors. See BS EN ISO 717-2:1997."@en;
  skos:prefLabel "l’nt,w"@en .

:c_b4273037 a skos:Concept;
  skos:broader :c_f4cc0ec3;
  skos:definition "Mass per unit area is expressed in terms of kilograms per square metre (kg/m²)."@en;
  skos:prefLabel "mass per unit area"@en .

:c_93488b6d a skos:Concept;
  dct:modified "2020-10-25T04:26:50.620Z"^^xsd:dateTime;
  skos:broader :c_f4cc0ec3;
  skos:definition "Noise is unwanted sound."@en;
  skos:inScheme :conceptScheme_751925ed;
  skos:prefLabel "noise"@en .

:c_e6d846bf a skos:Concept;
  dct:modified "2020-10-25T04:27:00.327Z"^^xsd:dateTime;
  skos:broader :c_f4cc0ec3;
  skos:definition "A frequency band in which the upper limit of the band is twice the frequency of the lower limit."@en;
  skos:inScheme :conceptScheme_751925ed;
  skos:prefLabel "octave band"@en .

:c_c13a7c46 a skos:Concept;
  skos:broader :c_f4cc0ec3;
  skos:definition "A frequency band in which the upper limit of the band is 21/3 times the frequency of the lower limit."@en;
  skos:prefLabel "one-third octave band"@en .

:c_2a1002d3 a skos:Concept;
  dct:modified "2020-10-25T04:27:58.892Z"^^xsd:dateTime;
  skos:broader :c_f4cc0ec3;
  skos:definition "A single-number quantity which characterises the airborne sound insulation of a material or building element in the laboratory. See BS EN ISO 717-1:1997."@en;
  skos:inScheme :conceptScheme_751925ed;
  skos:prefLabel "rw"@en .

:c_3fc6a13d a skos:Concept;
  dct:modified "2020-10-25T04:27:25.919Z"^^xsd:dateTime;
  skos:broader :c_f4cc0ec3;
  skos:definition "A layer that isolates a floating layer from a base floor and surrounding walls."@en;
  skos:inScheme :conceptScheme_751925ed;
  skos:prefLabel "resilient layer"@en .

:c_8f476b03 a skos:Concept;
  dct:modified "2020-10-25T04:27:37.381Z"^^xsd:dateTime;
  skos:broader :c_f4cc0ec3;
  skos:definition "The persistence of sound in a space after a sound source has been stopped."@en;
  skos:inScheme :conceptScheme_751925ed;
  skos:prefLabel "reverberation"@en .

:c_6ed11205 a skos:Concept;
  dct:modified "2020-10-25T04:27:48.773Z"^^xsd:dateTime;
  skos:broader :c_f4cc0ec3;
  skos:definition "The time, in seconds, taken for the sound to decay by 60dB after a sound source has been stopped."@en;
  skos:inScheme :conceptScheme_751925ed;
  skos:prefLabel "reverberation time"@en .

:c_fa726c7b a skos:Concept;
  dct:modified "2020-10-25T04:28:10.553Z"^^xsd:dateTime;
  skos:broader :c_f4cc0ec3;
  skos:definition "Floor that separates flats or rooms for residential purposes."@en;
  skos:inScheme :conceptScheme_751925ed;
  skos:prefLabel "separating floor"@en .

:c_e43f1fcb a skos:Concept;
  dct:modified "2020-10-28T15:17:24.773Z"^^xsd:dateTime;
  skos:broader :c_f4cc0ec3;
  skos:definition "Wall that separates adjoining dwelling-houses, flats or rooms for residential purposes."@en;
  skos:inScheme :conceptScheme_751925ed;
  skos:prefLabel "separating wall"@en-GB .

:c_da4b364b a skos:Concept;
  dct:modified "2020-10-25T04:28:31.298Z"^^xsd:dateTime;
  skos:broader :c_f4cc0ec3;
  skos:definition "A quantity related to the physical intensity of a sound."@en;
  skos:inScheme :conceptScheme_751925ed;
  skos:prefLabel "sound pressure level"@en .

:c_95d3756f a skos:Concept;
  dct:modified "2020-10-25T04:28:53.490Z"^^xsd:dateTime;
  skos:broader :c_f4cc0ec3;
  skos:definition "A quantity, measured in a laboratory, which characterises the sound insulating properties of a material or building element in a stated frequency band. See BS EN ISO 140-3:1995."@en;
  skos:inScheme :conceptScheme_751925ed;
  skos:prefLabel "sound reduction index (r)"@en .

:c_8c6a9923 a skos:Concept;
  dct:modified "2020-10-25T04:29:06.143Z"^^xsd:dateTime;
  skos:broader :c_f4cc0ec3;
  skos:definition "The composition of a particular sound in terms of separate frequency bands."@en;
  skos:inScheme :conceptScheme_751925ed;
  skos:prefLabel "spectrum"@en .

:c_3b310e19 a skos:Concept;
  dct:modified "2020-10-25T04:29:20.043Z"^^xsd:dateTime;
  skos:broader :c_f4cc0ec3;
  skos:definition "Sound which is carried via the structure of a building."@en;
  skos:inScheme :conceptScheme_751925ed;
  skos:prefLabel "structure-borne sound"@en .

:c_5aa42901 a skos:Concept;
  dct:modified "2020-10-25T04:29:34.851Z"^^xsd:dateTime;
  skos:broader :c_f4cc0ec3;
  skos:definition "United Kingdom Accreditation Service."@en;
  skos:inScheme :conceptScheme_751925ed;
  skos:prefLabel "ukas"@en .

:c_ac95ba41 a skos:Concept;
  dct:modified "2020-10-24T20:19:52.881Z"^^xsd:dateTime;
  skos:broader :c_f4cc0ec3;
  skos:definition "The measured improvement of impact sound insulation resulting from the installation of a floor covering or floating floor on a test floor in a laboratory. See BS EN ISO 717-2:1997."@en;
  skos:inScheme :conceptScheme_751925ed;
  skos:prefLabel "dlw"@en .

:c_f40ac57b dct:modified "2020-10-24T20:24:01.793Z"^^xsd:dateTime;
  skos:inScheme :conceptScheme_751925ed .

:c_1166f883 dct:modified "2020-10-24T20:19:10.331Z"^^xsd:dateTime;
  skos:inScheme :conceptScheme_751925ed .

:c_438bd78a dct:modified "2020-10-24T20:10:42.096Z"^^xsd:dateTime;
  skos:inScheme :conceptScheme_751925ed .

:c_aa316632 dct:modified "2020-10-24T20:24:34.204Z"^^xsd:dateTime;
  skos:inScheme :conceptScheme_751925ed .

:c_4cb28fa4 dct:modified "2020-10-24T20:22:03.002Z"^^xsd:dateTime;
  skos:inScheme :conceptScheme_751925ed .

:c_07abc5c2 dct:modified "2020-10-25T04:25:09.858Z"^^xsd:dateTime;
  skos:inScheme :conceptScheme_751925ed .

:c_8abc2fd9 dct:modified "2020-10-24T20:23:35.208Z"^^xsd:dateTime;
  skos:inScheme :conceptScheme_751925ed .

:c_0c33e781 dct:modified "2020-10-24T20:11:55.304Z"^^xsd:dateTime;
  skos:inScheme :conceptScheme_751925ed .

:c_c57961a6 dct:modified "2020-10-24T20:21:01.089Z"^^xsd:dateTime;
  skos:inScheme :conceptScheme_751925ed .

:c_c2902dec dct:modified "2020-10-24T20:25:01.285Z"^^xsd:dateTime;
  skos:inScheme :conceptScheme_751925ed .

:c_3262a30a dct:modified "2020-10-24T20:22:24.209Z"^^xsd:dateTime;
  skos:inScheme :conceptScheme_751925ed .

:c_cbfc0947 dct:modified "2020-10-24T20:21:20.858Z"^^xsd:dateTime;
  skos:inScheme :conceptScheme_751925ed .

:c_5bb42f0e dct:modified "2020-10-24T20:18:46.501Z"^^xsd:dateTime;
  skos:inScheme :conceptScheme_751925ed .

:c_61aec10c dct:modified "2020-10-24T20:18:25.333Z"^^xsd:dateTime;
  skos:inScheme :conceptScheme_751925ed .

:c_3d888dc1 dct:modified "2020-10-25T04:25:22.708Z"^^xsd:dateTime;
  skos:inScheme :conceptScheme_751925ed .

:c_d68c8ade dct:modified "2020-10-24T20:23:10.718Z"^^xsd:dateTime;
  skos:inScheme :conceptScheme_751925ed .

:c_b4273037 dct:modified "2020-10-25T04:26:38.681Z"^^xsd:dateTime;
  skos:inScheme :conceptScheme_751925ed .

:c_34c7d4e3 dct:modified "2020-10-25T04:26:24.011Z"^^xsd:dateTime;
  skos:inScheme :conceptScheme_751925ed .

:c_4f47aeea dct:modified "2020-10-24T20:22:46.510Z"^^xsd:dateTime;
  skos:inScheme :conceptScheme_751925ed .

:c_9a21f5a2 dct:modified "2020-10-24T20:20:33.912Z"^^xsd:dateTime;
  skos:inScheme :conceptScheme_751925ed .

:c_588bf28f dct:modified "2020-10-25T04:24:24.550Z"^^xsd:dateTime;
  skos:inScheme :conceptScheme_751925ed .

:c_f213d52c dct:modified "2020-10-24T20:17:54.891Z"^^xsd:dateTime;
  skos:inScheme :conceptScheme_751925ed .

:c_70a0403c dct:modified "2020-10-25T04:25:34.953Z"^^xsd:dateTime;
  skos:inScheme :conceptScheme_751925ed .

:c_c8566bf0 dct:modified "2020-10-25T04:24:52.842Z"^^xsd:dateTime;
  skos:inScheme :conceptScheme_751925ed .

:c_3b5778ee dct:modified "2020-10-24T20:10:58.711Z"^^xsd:dateTime;
  skos:inScheme :conceptScheme_751925ed .

:c_895306c7 dct:modified "2020-10-25T04:24:39.232Z"^^xsd:dateTime;
  skos:inScheme :conceptScheme_751925ed .

:c_e85e2d31 dct:modified "2020-10-24T20:19:31.526Z"^^xsd:dateTime;
  skos:inScheme :conceptScheme_751925ed .

:c_345811e8 dct:modified "2020-10-26T07:19:47.127Z"^^xsd:dateTime;
  skos:inScheme :conceptScheme_751925ed .

:c_d26ff5d2 dct:modified "2020-10-25T04:26:09.753Z"^^xsd:dateTime;
  skos:inScheme :conceptScheme_751925ed .

:c_b3eb4d7b dct:modified "2020-10-24T20:20:13.014Z"^^xsd:dateTime;
  skos:inScheme :conceptScheme_751925ed .

:c_c13a7c46 dct:modified "2020-10-25T04:27:14.383Z"^^xsd:dateTime;
  skos:inScheme :conceptScheme_751925ed .

:c_8144317d dct:modified "2020-10-24T20:11:37.568Z"^^xsd:dateTime;
  skos:inScheme :conceptScheme_751925ed .

:c_f4cc0ec3 dct:modified "2020-10-24T20:07:15.383Z"^^xsd:dateTime;
  skos:narrower :c_07abc5c2, :c_0c33e781, :c_0db511ab, :c_1166f883, :c_2a1002d3, :c_3262a30a,
    :c_345811e8, :c_34c7d4e3, :c_3b310e19, :c_3b5778ee, :c_3d888dc1, :c_3fc6a13d, :c_438bd78a,
    :c_4b4c9739, :c_4cb28fa4, :c_4f47aeea, :c_588bf28f, :c_5aa42901, :c_5bb42f0e, :c_61aec10c,
    :c_6ed11205, :c_70a0403c, :c_8144317d, :c_81482951, :c_895306c7, :c_8abc2fd9, :c_8c6a9923,
    :c_8f476b03, :c_93488b6d, :c_95d3756f, :c_9a21f5a2, :c_aa316632, :c_ac95ba41, :c_b3eb4d7b,
    :c_b4273037, :c_c13a7c46, :c_c2902dec, :c_c57961a6, :c_c8566bf0, :c_c878dbda, :c_cbfc0947,
    :c_d26ff5d2, :c_d68c8ade, :c_da4b364b, :c_e43f1fcb, :c_e6d846bf, :c_e85e2d31, :c_f213d52c,
    :c_f3cee240, :c_f40ac57b, :c_fa726c7b .

:c_0db511ab a skos:Concept;
  dct:modified "2020-10-24T20:01:38.708Z"^^xsd:dateTime;
  skos:broader :c_f4cc0ec3;
  skos:definition "Conversion of sound energy to heat, often by the use of a porous material."@en;
  skos:inScheme :conceptScheme_751925ed;
  skos:prefLabel "absorption"@en .

:c_4b4c9739 a skos:Concept;
  skos:broader :c_f4cc0ec3;
  skos:definition "A quantity characterising the effectiveness of a sound absorbing surface. The proportion of sound energy absorbed is given as a number between zero (for a fully reflective surface) and one (for a fully absorptive surface). Note that sound absorption coefficients determined from laboratory measurements may have values slightly larger than one. See BS EN 20354:1993."@en;
  skos:inScheme :conceptScheme_751925ed;
  skos:prefLabel "absorption coefficient"@en .

:c_c878dbda a skos:Concept;
  dct:modified "2020-10-24T20:01:44.488Z"^^xsd:dateTime;
  skos:broader :c_f4cc0ec3;
  skos:definition "Material that absorbs sound energy."@en;
  skos:inScheme :conceptScheme_751925ed;
  skos:prefLabel "absorptive material"@en .

:c_f3cee240 a skos:Concept;
  dct:modified "2020-10-24T20:01:41.621Z"^^xsd:dateTime;
  skos:broader :c_f4cc0ec3;
  skos:definition "Sound propagating through the air."@en;
  skos:inScheme :conceptScheme_751925ed;
  skos:prefLabel "airborne sound"@en .

:c_44c61ce8 a skos:Concept;
  dct:created "2020-10-25T04:32:22.323Z"^^xsd:dateTime;
  skos:broader :c_2ca1576c;
  skos:inScheme :conceptScheme_751925ed;
  skos:narrower :c_59a3ae21 .

:c_6d6d73cd dct:created "2020-10-25T04:38:31.854Z"^^xsd:dateTime;
  skos:broader :c_73c4361e;
  skos:narrower :c_90aedbdc .

:c_d10595f3 dct:modified "2020-10-25T04:37:04.887Z"^^xsd:dateTime .

:c_73c4361e skos:narrower :c_6d6d73cd .

:c_59a3ae21 dct:modified "2020-10-25T04:34:27.571Z"^^xsd:dateTime;
  skos:broader :c_44c61ce8 .

:c_2ca1576c dct:modified "2020-10-25T04:35:01.892Z"^^xsd:dateTime;
  skos:narrower :c_44c61ce8 .

:c_90aedbdc a skos:Concept;
  dct:created "2020-10-25T04:45:46.524Z"^^xsd:dateTime;
  skos:broader :c_6d6d73cd;
  skos:inScheme :conceptScheme_751925ed;
  skos:narrower :c_316d73a9;
  skos:prefLabel "key terms (adg)"@en .

:c_679215e0 skos:definition """This document is one of a series that has been
approved and issued by the Secretary of State
for the purpose of providing practical guidance
with respect to the requirements of Schedule 1
to and Regulation 7 of the Building Regulations
2010 (SI 2010/2214) for England and Wales."""@en .

:c_0822f77e a skos:Concept;
  skos:broader :c_90aedbdc;
  skos:definition "includes the erection or extension of a building, the provision or extension of a controlled service or ﬁtting in or in connection with a building, and the material alteration of a building, or a controlled service or ﬁtting."@en;
  skos:prefLabel "building work"@en-GB .

:c_39f68990 a skos:Concept;
  skos:broader :c_90aedbdc;
  skos:definition "means a mechanically operated valve that opens to discharge water when a ﬁxed (factory set) temperature or ﬁxed (factory set) pressure  is exceeded."@en;
  skos:prefLabel "combined temperature and pressure relief valve"@en .

:c_a1430501 a skos:Concept;
  skos:broader :c_90aedbdc;
  skos:definition "includes a service or ﬁtting subject to Schedule 1 requirements in respect of sanitation, hot water safety, water efﬁciency, drainage and waste disposal, combustion appliances and fuel storage, conservation of fuel or power, and electrical safety."@en .

:c_70908a07 skos:narrower :c_ab063a87 .

:c_62dfaa11 a skos:Concept;
  skos:broader :c_90aedbdc;
  skos:definition "means a method of heating in which the heat source is integral with the hot water vessel. Examples are an electrical immersion heater, or a gas burner with a ﬂue arrangement that passes through the vessel so that the ﬂue transfers heat to the stored water, or the circulation of water from a vessel situated near a burner with a ﬂue arrangement so that the ﬂue transfers heat to the circulating water."@en;
  skos:prefLabel "direct heating"@en .

:c_252b3da8 a skos:Concept;
  skos:broader :c_90aedbdc;
  skos:definition "means water that has been heated for cooking, food preparation, personal washing or cleaning purposes. The term is used irrespective of the type of building in which the hot water system is installed."@en;
  skos:prefLabel "domestic hot water"@en .

:c_36ceda7d a skos:Concept;
  skos:broader :c_90aedbdc;
  skos:definition "means a closet having a movable receptacle for the reception of faecal matter and its deodorisation by the use of earth, ashes or chemicals, or by other methods. This will therefore include chemical and composting toilets."@en .

:skosCollection_50d4bd2e skos:member :c_45847832, :c_4bcbd7aa, :c_e31d69a7 .

:c_8caf9cc1 a skos:Concept;
  skos:broader :c_90aedbdc;
  skos:definition "means the erection of any building or extension of a kind described in regulation 9 of and Schedule 2 to the Building Regulations 2010; or the carrying out of any work to or in connection with such a building or extension, if after the carrying out of that work it is still a building or extension of a kind described in that Schedule."@en;
  skos:prefLabel "exempt buildings and work"@en .

:c_66727700 a skos:Concept;
  skos:broader :c_90aedbdc;
  skos:definition "means a vessel to temporarily accommodate the expansion of water from the unvented hot water storage vessel as it is heated."@en;
  skos:prefLabel "expansion vessel"@en .

:c_e4d9fbd5 a skos:Concept;
  skos:broader :c_90aedbdc;
  skos:definition "is domestic wastewater excluding faecal matter and urine. When appropriately treated this may replace the use of wholesome water in WCs, urinals, irrigation or washing machines."@en;
  skos:prefLabel "greywater"@en .

:c_b1f8943d a skos:Concept;
  skos:broader :c_90aedbdc;
  skos:definition "means rainwater harvested from roofs or other suitable surfaces and collected and stored. When appropriately treated, this may replace the use of wholesome water in WCs, urinals, irrigation or washing machines."@en;
  skos:prefLabel "harvested rainwater"@en .

:c_cb024dd1 a skos:Concept;
  skos:broader :c_90aedbdc;
  skos:definition "means water that, when cold, was wholesome in accordance with the deﬁnition below and has been subjected to a heat source to increase its temperature."@en;
  skos:prefLabel "heated wholesome water"@en .

:c_3f5a9958 a skos:Concept;
  skos:broader :c_90aedbdc;
  skos:definition "means a vessel for storing: a. heated wholesome hot water or softened wholesome hot water for subsequent use b. water that is used to heat other water together with any ancillary safety devices described in paragraphs 3.10 and 3.11 of this Approved Document and all other applicable operating devices."@en;
  skos:prefLabel "hot water storage system"@en .

:c_ced9eb5e a skos:Concept;
  dct:modified "2020-10-26T07:29:02.985Z"^^xsd:dateTime;
  skos:broader :c_90aedbdc;
  skos:definition "means a hot water storage system having the safety devices described in 3.10 and 3.17 of this Approved Document factory-ﬁtted by the manufacturer, together with a kit containing other applicable devices supplied by the manufacturer to be ﬁtted by the installer."@en;
  skos:inScheme :conceptScheme_751925ed;
  skos:prefLabel "hot water storage system package"@en .

:c_86cbd31f a skos:Concept;
  skos:broader :c_90aedbdc;
  skos:definition "means a hot water storage system having the safety devices described in 3.10 and 3.17 of this Approved Document and all other applicable operating devices factory-ﬁtted by the manufacturer."@en;
  skos:prefLabel "hot water storage system unit"@en .

:c_f7036f54 a skos:Concept;
  skos:broader :c_90aedbdc;
  skos:definition "means a method of heating stored water through a heat exchanger."@en;
  skos:prefLabel "indirect heating"@en .

:c_4a4a5b61 a skos:Concept;
  skos:broader :c_90aedbdc;
  skos:definition "means a room or part of a room which contains a sink and food preparation facilities"@en;
  skos:prefLabel "kitchen"@en .

:c_47b084b0 a skos:Concept;
  dct:modified "2020-10-28T14:49:24.169Z"^^xsd:dateTime;
  skos:broader :c_90aedbdc;
  skos:definition "means an alteration which results in a building or a controlled service or ﬁtting not complying with, or being more, means of warning and escape, internal and external ﬁre spread, ﬁre service access and facilities, and access and use."@en;
  skos:inScheme :conceptScheme_751925ed;
  skos:prefLabel "material alteration (adg)"@en .

:c_ee888332 a skos:Concept;
  skos:broader :c_90aedbdc;
  skos:definition "means a device that will interrupt the supply of heat to a hot water storage vessel when a ﬁxed (factory set) temperature is exceeded. If this protective device is actuated it should only be possible to reset it manually."@en;
  skos:prefLabel "non-self-resetting energy cut-out"@en .

:c_e47ea7fb a skos:Concept;
  dct:modified "2020-10-26T07:35:00.935Z"^^xsd:dateTime;
  skos:broader :c_90aedbdc;
  skos:definition "means handling, making and cooking of food."@en;
  skos:inScheme :conceptScheme_751925ed;
  skos:prefLabel "preparation of food"@en .

:c_1aa022f8 a skos:Concept;
  dct:modified "2020-10-26T07:28:29.370Z"^^xsd:dateTime;
  skos:broader :c_90aedbdc;
  skos:definition "means a mechanically operated valve that opens to discharge water when a ﬁxed (factory set) pressure is exceeded."@en;
  skos:inScheme :conceptScheme_751925ed;
  skos:prefLabel "pressure relief valve"@en .

:c_0cdb0b97 a skos:Concept;
  dct:modified "2020-10-26T07:35:13.859Z"^^xsd:dateTime;
  skos:broader :c_90aedbdc;
  skos:definition "means a store of heat energy that can be used to heat domestic hot water by means of a heat exchanger. The thermal store can be heated by a variety of heat sources. Primary hot water thermal stores can be either vented or unvented."@en;
  skos:inScheme :conceptScheme_751925ed;
  skos:prefLabel "primary thermal store"@en .

:c_e2afc611 a skos:Concept;
  dct:modified "2020-10-26T07:32:20.075Z"^^xsd:dateTime;
  skos:broader :c_90aedbdc;
  skos:definition "for the purposes of this document means the identiﬁcation of the hazards associated with a process or activity combined with an assessment of the probability and consequences of each hazard."@en;
  skos:inScheme :conceptScheme_751925ed;
  skos:prefLabel "risk assessment"@en .

:c_fec9943e a skos:Concept;
  skos:broader :c_90aedbdc;
  skos:definition "means a room, or a suite of rooms, which is not a dwelling- house or a ﬂat and which is used by one or more persons to live and sleep in, and includes a room in a hostel, a hotel, a boarding house, a hall of residence or a residential home, but does not include a room in a hospital, or other similar establishment, used for patient accommodation.        "@en;
  skos:inScheme :conceptScheme_751925ed .

:c_316d73a9 a skos:Concept;
  dct:modified "2020-10-26T07:39:49.038Z"^^xsd:dateTime;
  skos:broader :c_90aedbdc;
  skos:definition "means a room containing a WC or urinal, whether or not it also contains other sanitary appliances. Sanitary accommodation containing one or more cubicles counts as a single space if there is free circulation of air throughout the space."@en;
  skos:inScheme :conceptScheme_751925ed;
  skos:prefLabel "sanitary accommodation"@en .

:c_f8b75f3a a skos:Concept;
  dct:modified "2020-10-26T07:36:00.668Z"^^xsd:dateTime;
  skos:broader :c_90aedbdc;
  skos:definition "means WC, urinal, bath, shower, washbasin, sink, bidet and drinking fountain. It also includes appliances that are not connected to a water supply (e.g. composting toilet) or drain (e.g. waterless urinal)."@en;
  skos:inScheme :conceptScheme_751925ed;
  skos:prefLabel "sanitary appliance"@en .

:c_1b2db6bc a skos:Concept;
  skos:broader :c_90aedbdc;
  skos:definition "means closets and urinals."@en;
  skos:inScheme :conceptScheme_751925ed .

:c_00af1bc5 a skos:Concept;
  dct:modified "2020-10-25T05:13:52.276Z"^^xsd:dateTime;
  skos:broader :c_90aedbdc;
  skos:definition "means a receptacle used for holding water (for preparation of food or washing up) supplied through a tap and having a wastepipe."@en;
  skos:inScheme :conceptScheme_751925ed;
  skos:prefLabel "sink"@en .

:c_3d59dac9 a skos:Concept;
  skos:broader :c_90aedbdc;
  skos:definition "means water which would be regarded as wholesome for the purposes of regulations made under section 67 of the Water Industry Act 1991 (standards of wholesomeness) as they apply for the purposes of Part G of Schedule 1 in accordance with paragraph (2c) but for the presence of sodium in excess of the level speciﬁed in those regulations if it is caused by a water softener or water softening process which reduces the concentrations of calcium and magnesium."@en;
  skos:inScheme :conceptScheme_751925ed .

:c_e146ab76 skos:definition "is the maximum declared energy output rate (kW) as declared on the appliance data plate."@en .

:c_e31d69a7 a skos:Concept;
  dct:modified "2020-10-25T05:14:01.936Z"^^xsd:dateTime;
  skos:broader :c_90aedbdc;
  skos:definition "means a device, installed in the discharge pipe from a valve, that provides an air break allowing discharge to be conducted safely to a place of termination. The tundish also provides a visible indication of a discharge and functions as backﬂow prevention device."@en;
  skos:inScheme :conceptScheme_751925ed;
  skos:prefLabel "tundish"@en .

:c_4bcbd7aa a skos:Concept;
  dct:modified "2020-10-26T07:40:29.959Z"^^xsd:dateTime;
  skos:broader :c_90aedbdc;
  skos:definition "means a mechanically operated valve that opens to discharge water when a ﬁxed (factory set) temperature is exceeded."@en;
  skos:inScheme :conceptScheme_751925ed;
  skos:prefLabel "temperature relief valve"@en .

:c_fbe47c16 a skos:Concept;
  dct:modified "2020-10-26T07:20:41.669Z"^^xsd:dateTime;
  skos:broader :c_90aedbdc;
  skos:definition "means a vessel fed with cold water from a supply pipe or dedicated storage cistern (without a vent pipe) and in which water is heated directly or indirectly. Expansion of the water when it is heated is accommodated either internally or externally and the system is ﬁtted with safety devices to prevent water temperatures exceeding 100˚C, and other applicable operating devices to control primary ﬂow, prevent backﬂow, control working pressure and accommodate expansion."@en;
  skos:inScheme :conceptScheme_751925ed;
  skos:prefLabel "unvented (closed) hot water storage system"@en .

:c_885de476 a skos:Concept;
  dct:modified "2020-10-25T05:14:32.439Z"^^xsd:dateTime;
  skos:broader :c_90aedbdc;
  skos:definition "means an appliance used for reception and disposal of urine."@en;
  skos:inScheme :conceptScheme_751925ed;
  skos:prefLabel "urinal"@en .

:c_a0d96205 a skos:Concept;
  dct:modified "2020-10-26T07:28:00.179Z"^^xsd:dateTime;
  skos:broader :c_90aedbdc;
  skos:definition "means a vessel fed with cold water from a dedicated storage cistern. Expansion of the water when it is heated is accommodated through the cold feed pipe. A vent pipe connecting the top of the vessel to a point open to the atmosphere above the cold water storage cistern is provided as a safety device."@en;
  skos:inScheme :conceptScheme_751925ed;
  skos:prefLabel "vented (open) hot water storage system"@en .

:c_9d5baa50 a skos:Concept;
  skos:broader :c_90aedbdc;
  skos:definition "means a closet that has a separate ﬁxed receptacle connected to a drainage system and separate provision for ﬂushing from a supply of clean water either by the operation of a mechanism or by automatic action. Water-closets are also referred to as WCs."@en;
  skos:inScheme :conceptScheme_751925ed .

:skosCollection_50d4bd2e skos:member :c_12b20158, :c_7f8af2c2, :c_885de476, :c_a0d96205,
    :c_d39bf581, :c_fbe47c16 .

:c_99150200 a skos:Concept;
  dct:modified "2020-10-26T07:30:33.748Z"^^xsd:dateTime;
  skos:broader :c_90aedbdc;
  skos:definition "means water complying  with the requirements of regulations made under Section 67 (Standards of wholesomeness) of the Water Industry Act 1991. The regulations made under this Section at the time of publication Regulations 2000 (SI 2000/3184 as amended),and, for Wales, the Water Supply (Water Quality) Regulations 2001 (SI 2001/3911 as amended)."@en;
  skos:inScheme :conceptScheme_751925ed;
  skos:prefLabel "wholesome water"@en .

:c_a1430501 skos:inScheme :conceptScheme_751925ed .

:c_70908a07 dct:modified "2020-10-26T06:59:49.089Z"^^xsd:dateTime .

:c_39f68990 dct:modified "2020-10-26T07:43:22.855Z"^^xsd:dateTime;
  skos:inScheme :conceptScheme_751925ed .

:c_8caf9cc1 dct:modified "2020-10-26T07:29:45.865Z"^^xsd:dateTime;
  skos:inScheme :conceptScheme_751925ed .

:c_3f5a9958 dct:modified "2020-10-26T07:30:48.875Z"^^xsd:dateTime;
  skos:inScheme :conceptScheme_751925ed .

:c_b1f8943d dct:modified "2020-10-26T07:27:31.748Z"^^xsd:dateTime;
  skos:inScheme :conceptScheme_751925ed .

:c_e4d9fbd5 dct:modified "2020-10-26T07:40:45.571Z"^^xsd:dateTime;
  skos:inScheme :conceptScheme_751925ed .

:c_252b3da8 dct:modified "2020-10-26T07:33:40.695Z"^^xsd:dateTime;
  skos:inScheme :conceptScheme_751925ed .

:c_62dfaa11 dct:modified "2020-10-26T07:42:24.653Z"^^xsd:dateTime;
  skos:inScheme :conceptScheme_751925ed .

:c_0822f77e skos:inScheme :conceptScheme_751925ed .

:c_152c4bbc a skos:Concept;
  dct:created "2020-10-25T05:44:27.690Z"^^xsd:dateTime;
  dct:modified "2020-10-25T06:30:47.310Z"^^xsd:dateTime;
  skos:broader :c_710680da;
  skos:definition "The following definitions have been adopted solely for the purposes of providing clarity in this Approved Document."@en;
  skos:inScheme :conceptScheme_751925ed;
  skos:narrower :c_e146ab76;
  skos:notation "1.4"@en;
  skos:prefLabel "explanation of terms used"@en .

:c_36ceda7d skos:inScheme :conceptScheme_751925ed .

:c_f7036f54 dct:modified "2020-10-26T07:26:46.645Z"^^xsd:dateTime;
  skos:inScheme :conceptScheme_751925ed .

:c_cb024dd1 dct:modified "2020-10-26T07:19:05.888Z"^^xsd:dateTime;
  skos:inScheme :conceptScheme_751925ed .

:c_4a4a5b61 dct:modified "2020-10-25T05:15:00.041Z"^^xsd:dateTime;
  skos:inScheme :conceptScheme_751925ed .

:c_66727700 dct:modified "2020-10-26T07:40:15.158Z"^^xsd:dateTime;
  skos:inScheme :conceptScheme_751925ed .

:c_86cbd31f dct:modified "2020-10-26T07:26:00.678Z"^^xsd:dateTime;
  skos:inScheme :conceptScheme_751925ed .

:c_ee888332 dct:modified "2020-10-26T07:21:33.767Z"^^xsd:dateTime;
  skos:inScheme :conceptScheme_751925ed .

:c_90aedbdc dct:modified "2020-10-25T05:16:53.211Z"^^xsd:dateTime;
  skos:narrower :c_00af1bc5, :c_0822f77e, :c_1b2db6bc, :c_252b3da8, :c_36ceda7d, :c_39f68990,
    :c_3d59dac9, :c_3f5a9958, :c_47b084b0, :c_4a4a5b61, :c_4bcbd7aa, :c_62dfaa11, :c_66727700,
    :c_86cbd31f, :c_885de476, :c_8caf9cc1, :c_99150200, :c_9d5baa50, :c_a0d96205, :c_a1430501,
    :c_b1f8943d, :c_cb024dd1, :c_ced9eb5e, :c_e31d69a7, :c_e4d9fbd5, :c_ee888332, :c_f7036f54,
    :c_f8b75f3a, :c_fbe47c16, :c_fec9943e .

:c_f6ff7c1c dct:modified "2020-10-25T05:28:02.128Z"^^xsd:dateTime;
  skos:definition """The Building Regulations 2010 (SI 2010/2214),
which came into operation on 1 October 2010,
replace the Building Regulations 2000 (SI 2000/2531)
and consolidate all subsequent revisions to those
regulations. This document is one of a series that
has been approved and issued by the Secretary
of State for the purpose of providing practical
guidance with respect to the requirements of
Schedule 1 to and Regulation 7 of the Building
Regulations 2010 for England and Wales."""@en .

:c_679215e0 a skos:Concept;
  dct:modified "2020-10-25T05:21:08.543Z"^^xsd:dateTime;
  skos:broader :c_42d467db;
  skos:inScheme :conceptScheme_751925ed;
  skos:prefLabel "drainage and waste disposal 2015 edition"@en .

:c_44c61ce8 dct:modified "2020-10-25T05:26:12.088Z"^^xsd:dateTime;
  skos:definition """This document has been approved by the
Secretary of State to provide practical guidance
on ways of complying with the requirements in
Part F of Schedule 1 to, and regulations 39, 42
and 44 (in so far as it relates to fixed systems
for mechanical ventilation) of, the Building
Regulations 2010 (SI 2010/2214) for England
and Wales, and regulations 20(1) and 20(6) (in so
far as it relates to fixed systems for mechanical
ventilation) of the Building (Approved Inspectors
etc) Regulations 2010 (SI 2010/2215) for England
and Wales. The Building Regulations 2010
and the Building (Approved Inspectors etc)
Regulations 2010 are referred to throughout
the remainder of this document as ‘the Building
Regulations’ and ‘the Approved Inspectors
Regulations’ respectively."""@en .

:c_73c4361e dct:modified "2020-10-25T05:23:12.369Z"^^xsd:dateTime .

:c_4e975ede dct:modified "2020-10-25T05:31:08.927Z"^^xsd:dateTime .

:c_6d6d73cd dct:modified "2020-10-25T05:25:19.058Z"^^xsd:dateTime;
  skos:definition """This document has been approved and issued
by the Secretary of State to provide practical
guidance on ways of complying with Requirements G1 to G6 and regulations 7 and 36 of the Building
Regulations 2010 (SI 2010/2214) for England and
Wales, as amended. The Building Regulations
2010 are referred to throughout the remainder
of this Document as ‘the Building Regulations’.
Where appropriate the Approved Document also
gives guidance on relevant requirements in the
Building (Approved Inspectors etc.) Regulations
2010 (SI 2010/2215)."""@en .

:c_12c47f28 skos:definition """This document is one of a series that has been
approved by the First Secretary of State for the
purpose of providing practical guidance with
respect to the requirements of Schedule 1 to and
Regulation 7 of the Building Regulations 2010
(SI 2010/2214) for England and Wales."""@en .

:c_710680da a skos:Concept;
  dct:created "2020-10-25T05:35:17.135Z"^^xsd:dateTime;
  dct:modified "2020-10-25T05:45:02.801Z"^^xsd:dateTime;
  skos:broader :c_fec1533e;
  skos:definition """This document has been approved and issued
by the Secretary of State to provide practical
guidance on ways of complying with Requirements
J1 to J7 and regulations 7 of the Building
Regulations 2010 (SI 2010/2214) for England
and Wales. The Building Regulations 2010 are
referred to throughout the remainder of this
Document as ‘the Building Regulations’. Where
appropriate the Approved Document also gives
guidance on relevant requirements in the Building
(Approved Inspectors etc) Regulations 2010
(SI 2010/2215)."""@en;
  skos:inScheme :conceptScheme_751925ed;
  skos:narrower :c_152c4bbc;
  skos:prefLabel "combustion appliances and fuel storage systems 2010 edition incorporating 2010 and 2013 amendments"@en .

:c_fec1533e dct:modified "2020-10-25T05:36:43.835Z"^^xsd:dateTime;
  skos:narrower :c_710680da .

:c_3b6a6b21 dct:modified "2020-10-26T07:26:32.046Z"^^xsd:dateTime;
  skos:prefLabel "solid biofuel"@en .

:c_be620037 a skos:Concept;
  skos:broader :c_152c4bbc;
  skos:definition "is an enclosure specifically constructed or adapted to accommodate one or more combustion appliances."@en;
  skos:prefLabel "appliance compartment"@en .

:c_3fa58f37 a skos:Concept;
  skos:broader :c_152c4bbc;
  skos:definition "is a method of installing an open-flued appliance into a compartment which is sealed from the remainder of the building and whose ventilation is so arranged in conjunction with the appliance flue as to achieve a balanced flue effect."@en;
  skos:prefLabel "balanced compartment"@en .

:c_2ea90bc3 a skos:Concept;
  skos:broader :c_152c4bbc;
  skos:definition "appliance is a type of room- sealed appliance which draws its combustion air from a point outside the building adjacent to the point at which the combustion products are discharged, the inlet and outlet being so disposed that wind effects are substantially balanced. Balanced flues may run vertically, but in the most common configuration they discharge horizontally through the external wall against which the appliance is situated."@en;
  skos:prefLabel "balanced flue"@en .

:c_0de6ed98 a skos:Concept;
  skos:broader :c_152c4bbc;
  skos:definition "is the boundary of the land or buildings belonging to and under the control of the building owner. Depending upon the paragraphs of this Approved Document to which it applies, it may be drawn only around the perimeter of the land in question or extended to the centreline of adjacent routes or waterways as shown in Diagram 1."@en;
  skos:prefLabel "boundary"@en .

:c_3e30efaf a skos:Concept;
  skos:broader :c_152c4bbc;
  skos:definition "is a body that carries out checks for compliance with the Building Regulations on plans of building work and on the building work itself. The Building Control Body may be either the local authority or an Approved Inspector. For further details, see the manual to the Building Regulations."@en;
  skos:prefLabel "building control body"@en-GB .

:c_8c3e4b6f a skos:Concept;
  skos:broader :c_152c4bbc;
  skos:definition "The of an oil tank is its nominal capacity as stated by the manufacturer. It is usually 95 per cent of the volume of liquid required to fill it to the brim."@en;
  skos:prefLabel "capacity"@en .

:c_4a83bd38 a skos:Concept;
  skos:broader :c_152c4bbc;
  skos:definition " is a structure consisting of a wall or walls enclosing one or more flues (see Diagram 2). In the gas industry, the chimney for a gas appliance is commonly called the flue."@en;
  skos:prefLabel "chimney"@en .

:c_cf1e8e52 a skos:Concept;
  skos:broader :c_152c4bbc;
  skos:definition " is an apparatus where fuel is burned to generate heat for space heating, water heating, cooking or other similar purpose. The appliance does not include systems to deliver fuel to it or for the distribution of heat. Typical combustion appliances are boilers, warm air heaters, water heaters, fires, stoves and cookers."@en;
  skos:prefLabel "combustion appliance (or appliance)"@en .

:c_7390c895 a skos:Concept;
  skos:broader :c_152c4bbc;
  skos:definition "in BS EN 1443:2003 expresses the performance characteristics of a chimney or its components, as assessed in accordance with an appropriate European product standard, by means of a code such as EN 1234 – T400 N1 D1 Gxx. Further information is given in Appendix G."@en;
  skos:prefLabel "designation system"@en .

:c_ee1dbf01 a skos:Concept;
  skos:broader :c_152c4bbc;
  skos:definition "is an opening formed by a factory-made component into any part of the flue serving an open-flued appliance. Such openings may be provided to allow dilution air to be drawn into a flue or to lessen the effects of down-draught on combustion in the appliance"@en;
  skos:prefLabel "draught break"@en .

:c_119d7903 a skos:Concept;
  skos:broader :c_152c4bbc;
  skos:definition "is a form of draught break intended to prevent conditions in the main length of flue from interfering with the combustion performance of an open-flued appliance (see Diagram 3(a)). It allows the appliance to operate without interference from down- draughts that may occur in adverse wind conditions and excessive draught."@en;
  skos:prefLabel "draught diverter"@en .

:c_bfc3ac08 a skos:Concept;
  skos:broader :c_152c4bbc;
  skos:definition "is a factory-made counter-balanced flap device admitting air to the flue, from the same space as the combustion air, to prevent excessive variations in the draught (see Diagram 3(b)). It is usual for these to be in the fluepipe or chimney, but they may be located on the appliance."@en;
  skos:prefLabel "draught stabiliser"@en .

:c_d55b06b8 a skos:Concept;
  skos:broader :c_152c4bbc;
  skos:definition "is defined in BS EN 13141 -1:2004 as the area of a sharp-edged circular orifice which would pass the same air flow rate at the same applied pressure difference as the product or device being tested. The equivalent area of a simple ventilator will be less than the geometrical free area and for complex products may be significantly less."@en;
  skos:prefLabel "equivalent area"@en .

:c_0ef5294b a skos:Concept;
  skos:broader :c_152c4bbc;
  skos:definition "are prefabricated chimneys that are commonly manufactured as sets of components for assembly on site (although they can be supplied as one unit), having the performance appropriate for the intended appliance. They are available in various materials and types ranging from single-walled metal chimneys suitable for some gas appliances to twin-walled chimneys with insulation sandwiched between an inner liner and an outer metal wall which are designed for oil or solid fuel use."@en;
  skos:prefLabel "factory-made metal chimneys (also known as system chimneys)"@en .

:c_17d58c6d a skos:Concept;
  skos:broader :c_152c4bbc;
  skos:definition "the proper discharge of the flue gases depends upon the operation of a fan, which may be separately installed in the flue or may be an integral part of the combustion appliance. Fans in combustion appliances either may extract flue gases from the combustion chamber or may cause the flue gases to be displaced from the combustion chamber if the fan is supplying it with air for combustion. Appliances with fans providing the combustion air (including most oil-fired and many gas- fired boilers) are also commonly referred to as forced draught appliances (see Diagram 4). Flues in fanned draught installations run horizontally or vertically and can be at higher or lower pressures than their surroundings, dependent upon the location of the fan."@en;
  skos:prefLabel "fanned draught installation"@en .

:c_ed23b7cc a skos:Concept;
  skos:broader :c_152c4bbc;
  skos:definition "is a building or part of a building comprising one or more rooms, spaces or storeys constructed to prevent the spread of fire to or from another part of the same building or an adjoining building. (A roof-10. space above the top storey of a fire compartment is included in that fire compartment.) "@en;
  skos:prefLabel "fire compartment"@en .

:c_870f938c a skos:Concept;
  dct:modified "2020-10-26T07:21:50.256Z"^^xsd:dateTime;
  skos:broader :c_152c4bbc;
  skos:definition "of a building is a form of compartmentation in which part of a building is separated from another part of the same building by a compartment wall. Such walls run the full height of the part and are in one vertical plane. Further information on this is given in Approved Document B Vol 2 (see Section 8 Compartmentation and Appendix C Methods of Measurement)."@en;
  skos:inScheme :conceptScheme_751925ed;
  skos:prefLabel "separated part"@en .

:c_45847832 a skos:Concept;
  dct:modified "2020-10-26T07:45:06.786Z"^^xsd:dateTime;
  skos:broader :c_152c4bbc;
  skos:definition "is a structural opening (sometimes called a builder’s opening) formed in a wall or in a chimney breast, from which a chimney leads and which has a hearth at its base. Simple structural openings (Diagram 5(a)) are suitable for closed appliances such as stoves, cookers or boilers, but gathers (Diagram 5(b)) are necessary for accommodating open fires. Fireplace recesses are often lined with firebacks to accommodate inset open fires (Diagram 5(c)). Lining components and decorative treatments fitted around openings reduce the opening area. It is the finished fireplace opening area which determines the size of flue required for an open fire in such a recess."@en;
  skos:inScheme :conceptScheme_751925ed;
  skos:prefLabel "fireplace recess"@en .

:c_9ab3dc4c a skos:Concept;
  skos:broader :c_152c4bbc;
  skos:definition "of a component or construction is a measure of its ability to withstand the effects of fire in one or more ways for a stated period of time. Guidance on determination of performance in terms of fire resistance is given in Approved Document B (Fire Safety)."@en;
  skos:prefLabel "fire resistance"@en .

:c_3a3a6363 a skos:Concept;
  skos:broader :c_152c4bbc;
  skos:definition "is a means of shielding a fuel tank from the thermal radiation from a fire. For  LPG tanks, it also ensures that gas accidentally leaking from the tank or fittings must travel by a longer path and therefore disperse safely, before reaching a hazard such as an opening in a building, a boundary or other potential ignition source."@en;
  skos:prefLabel "fire wall"@en .

:c_12b20158 a skos:Concept;
  dct:modified "2020-10-25T06:27:16.350Z"^^xsd:dateTime;
  skos:broader :c_152c4bbc;
  skos:definition "is a passage that conveys the products of combustion from an appliance to the outside air (see Diagram 2)."@en;
  skos:inScheme :conceptScheme_751925ed;
  skos:prefLabel "flue"@en .

:c_3a623af3 a skos:Concept;
  skos:broader :c_152c4bbc;
  skos:definition "systems consist of a set of factory-made components, made from precast concrete, clay or other masonry units, that are designed for assembly on site to provide a complete chimney having the performance appropriate for the intended appliance. There are two types of common systems, one being solely for use with gas- burning appliances and the other, often called chimney block systems, being primarily designed for solid fuel-burning appliances."@en;
  skos:prefLabel "flueblock chimney"@en .

:c_7f8af2c2 a skos:Concept;
  skos:broader :c_152c4bbc;
  skos:definition "is a factory made unit, usually made of metal, which is similar to a prefabricated appliance chamber except that it is designed to accommodate a gas burning appliance in conjunction with a factory-made chimney."@en;
  skos:prefLabel "flue box"@en .

:c_9e940521 a skos:Concept;
  dct:modified "2020-10-26T07:41:44.182Z"^^xsd:dateTime;
  skos:broader :c_152c4bbc;
  skos:definition "is one which is designed to be used without connection to a flue. Its products of combustion mix with the surrounding room air and are eventually transported to the outside as stale air leaves the room (see Diagram 4(g))."@en;
  skos:inScheme :conceptScheme_751925ed;
  skos:prefLabel "flueless appliance"@en .

:c_e9c0c7da a skos:Concept;
  dct:modified "2020-10-26T07:31:18.401Z"^^xsd:dateTime;
  skos:broader :c_152c4bbc;
  skos:definition "is the wall of the chimney that is in contact with the products of combustion (see Diagram 2), such as a concrete flue liner, the inner liner of a factory-made chimney system or a flexible liner fitted into an existing chimney."@en;
  skos:inScheme :conceptScheme_751925ed;
  skos:prefLabel "flue liner"@en .

:c_873f1974 a skos:Concept;
  dct:modified "2020-10-26T07:43:06.458Z"^^xsd:dateTime;
  skos:broader :c_152c4bbc;
  skos:definition "is the point at which the products of combustion are discharged from the flue to the outside atmosphere, such as the top of a chimney pot or flue terminal."@en;
  skos:inScheme :conceptScheme_751925ed;
  skos:prefLabel "flue outlet"@en .

:c_dcbadafe a skos:Concept;
  dct:modified "2020-10-25T06:28:21.890Z"^^xsd:dateTime;
  skos:broader :c_152c4bbc;
  skos:definition "is a pipe, either single walled (bare or insulated) or double walled, which connects a combustion appliance to a flue in a chimney. For clarity, when used in this way, it may be called a connecting fluepipe. (Fluepipe is also used to describe the tubular components from which some factory made chimneys for gas and oil appliances are made or from which plastic flue systems are made)."@en;
  skos:inScheme :conceptScheme_751925ed;
  skos:prefLabel "fluepipe"@en .

:c_229f83e8 a skos:Concept;
  dct:modified "2020-10-26T07:24:13.103Z"^^xsd:dateTime;
  skos:broader :c_152c4bbc;
  skos:definition "is a base intended to safely isolate a combustion appliance from people, combustible parts of the building fabric and soft furnishings. The exposed surface of the hearth provides a region around the appliance which can be kept clear of anything at risk of fire. The body of the hearth may be thin insulating board, a substantial thickness of material such as concrete or some intermediate provision dependent upon the weight and downward heat emission characteristics of the appliance(s) upon it (see Diagram 6)."@en;
  skos:inScheme :conceptScheme_751925ed;
  skos:prefLabel "hearth"@en .

:c_22c38d73 a skos:Concept;
  dct:modified "2020-10-26T07:22:24.968Z"^^xsd:dateTime;
  skos:broader :c_152c4bbc;
  skos:definition "is the maximum rate of energy flow into an appliance. It is calculated as the rate of fuel flow to the appliance multiplied by either the fuel’s gross or net calorific value."@en;
  skos:inScheme :conceptScheme_751925ed;
  skos:prefLabel "heat input rate"@en .

:c_53d35017 a skos:Concept;
  dct:modified "2020-10-26T07:35:44.265Z"^^xsd:dateTime;
  skos:broader :c_152c4bbc;
  skos:definition "are those instructions produced by manufacturers to enable installers to correctly install and test appliances and flues and to commission them into service."@en;
  skos:inScheme :conceptScheme_751925ed;
  skos:prefLabel "installation instructions"@en .

:c_41ebf78a a skos:Concept;
  dct:modified "2020-10-25T06:28:31.179Z"^^xsd:dateTime;
  skos:broader :c_152c4bbc;
  skos:definition "the combustion products flow into the flue as a result of the draught produced due to the difference between the temperature of the gases within the flue and the temperature of the ambient air. Taller flues produce a greater draught at their base. Except for those balanced flue appliances which are designed to discharge directly through the wall adjacent to the appliance, a satisfactory natural draught requires an essentially vertical run of flue (see Diagram 4 (a) and (b))."@en;
  skos:inScheme :conceptScheme_751925ed;
  skos:prefLabel "natural draught flue"@en .

:c_ad9a7d0c a skos:Concept;
  dct:modified "2020-10-25T06:28:05.847Z"^^xsd:dateTime;
  skos:broader :c_152c4bbc;
  skos:definition "This is the highest level of reaction to fire performance. Non-combustible materials include: a. any material which when tested to BS 476-11:1982 (2007) does not flame nor cause any rise in temperature on either the centre (specimen) or furnace thermocouples; and b. products classified as non-combustible in tests following the procedures in BS 476-4:1970 (2007); c. any material classified as class A1 in accordance with BS EN 13501-1:2002 Fire classification of construction products and building elements. Classification using data from reaction to fire tests. Typical examples of such materials to be found in buildings include totally inorganic materials such as concrete, fired clay, ceramics, metals, plaster and masonry containing not more than 1 per cent by weight or volume of organic material. (Use in buildings of combustible metals such as magnesium–aluminium alloys should be assessed in each individual case.) More detailed information is given in Approved Document B (Fire Safety)."@en;
  skos:inScheme :conceptScheme_751925ed;
  skos:prefLabel "non-combustible material"@en .

:c_d39bf581 a skos:Concept;
  dct:modified "2020-10-25T06:27:28.765Z"^^xsd:dateTime;
  skos:broader :c_152c4bbc;
  skos:definition "for the purposes of the Gas Appliances (Safety) Regulations (1995), means: a. a. a body which is approved by the Secretary of State for Trade and Industry as being competent to carry out the required Attestation procedures for gas appliances and whose name and identification number has been notified by him/her to the Commission of the European Community and to other member States in accordance with the Gas Appliances (Safety) Regulations (1995); b. b. a body which has been similarly approved for the purposes of the Gas Appliances Directive by another member State and whose name and identification number has been notified to the Commission and to other member States pursuant to the Gas Appliances Directive."@en;
  skos:inScheme :conceptScheme_751925ed;
  skos:prefLabel "notified body"@en .

:c_22764bab a skos:Concept;
  dct:modified "2020-10-26T07:24:24.540Z"^^xsd:dateTime;
  skos:broader :c_152c4bbc;
  skos:definition "is one which draws its combustion air from the room or space within which it is installed and which requires a flue to discharge its products of combustion to the outside air (see Diagram 4 (a), (c) and (e))."@en;
  skos:inScheme :conceptScheme_751925ed;
  skos:prefLabel "open-flued appliance"@en .

:c_d67339c2 a skos:Concept;
  dct:modified "2020-10-26T07:34:19.568Z"^^xsd:dateTime;
  skos:broader :c_152c4bbc;
  skos:definition "is a set of factory-made precast concrete components designed to provide a fireplace recess to accommodate an appliance such as a stove, and incorporates a gather when used with an open fire. The chamber is normally positioned against a wall and may be designed to support a chimney. The chamber and chimney are often enclosed to create a false chimney breast (see also ‘flue box’)."@en;
  skos:inScheme :conceptScheme_751925ed;
  skos:prefLabel "prefabricated appliance chamber"@en .

:c_a794f4c0 a skos:Concept;
  dct:modified "2020-10-26T07:21:19.736Z"^^xsd:dateTime;
  skos:broader :c_152c4bbc;
  skos:definition "(sometimes shortened to rated input) for a gas appliance is the maximum heat input rate at which it can be operated, as declared on the appliance data plate. (See also heat input rate.)"@en;
  skos:inScheme :conceptScheme_751925ed;
  skos:prefLabel "rated heat input"@en .

:c_e146ab76 a skos:Concept;
  skos:broader :c_152c4bbc;
  skos:inScheme :conceptScheme_751925ed;
  skos:prefLabel "rated heat output for an oil appliance"@en .

:skosCollection_50d4bd2e skos:member :c_0ab83009, :c_2d35a0e4, :c_9d5baa50 .

:c_75f221c0 a skos:Concept;
  dct:modified "2020-10-26T07:32:58.549Z"^^xsd:dateTime;
  skos:broader :c_152c4bbc;
  skos:definition "for a solid fuel appliance is the manufacturer’s declared nominal energy output rate (kW) for the appliance. This may be different for different fuels."@en;
  skos:inScheme :conceptScheme_751925ed;
  skos:prefLabel "rated heat output for a solid fuel appliance"@en .

:c_0ab83009 a skos:Concept;
  dct:modified "2020-10-26T07:19:27.005Z"^^xsd:dateTime;
  skos:broader :c_152c4bbc;
  skos:definition "means an appliance whose combustion system is sealed from the room in which the appliance is located and which obtains air for combustion from a ventilated uninhabited space within the building or directly from the open air outside the building and which vents the products of combustion directly to open air outside the building (see Diagram 4 (b), (d) and (f))."@en;
  skos:inScheme :conceptScheme_751925ed;
  skos:prefLabel "room-sealed appliance"@en .

:c_3b6a6b21 a skos:Concept;
  skos:broader :c_152c4bbc;
  skos:definition "means, for the purpose of this Approved Document, a solid fuel derived from plants and trees. It can include logs, wood chips, wood pellets and other processed plant material."@en;
  skos:inScheme :conceptScheme_751925ed .

:c_152c4bbc skos:narrower :c_0ab83009, :c_0de6ed98, :c_0ef5294b, :c_119d7903, :c_12b20158,
    :c_17d58c6d, :c_22764bab, :c_229f83e8, :c_22c38d73, :c_2ea90bc3, :c_3a3a6363, :c_3a623af3,
    :c_3b6a6b21, :c_3e30efaf, :c_3fa58f37, :c_41ebf78a, :c_45847832, :c_4a83bd38, :c_53d35017,
    :c_7390c895, :c_75f221c0, :c_7f8af2c2, :c_870f938c, :c_873f1974, :c_8c3e4b6f, :c_9ab3dc4c,
    :c_9e940521, :c_a794f4c0, :c_ad9a7d0c, :c_be620037, :c_bfc3ac08, :c_cf1e8e52, :c_d39bf581,
    :c_d55b06b8, :c_d67339c2, :c_dcbadafe, :c_e9c0c7da, :c_ed23b7cc, :c_ee1dbf01 .

:c_01839084 a skos:Concept;
  dct:modified "2020-10-25T06:27:56.486Z"^^xsd:dateTime;
  skos:broader :c_152c4bbc;
  skos:definition "is a contracted part of the flue between a fireplace recess and its chimney (see Diagram 22). Throats are usually formed from prefabricated components as shown in Diagram 29."@en;
  skos:inScheme :conceptScheme_751925ed;
  skos:prefLabel "throat"@en .

:c_cf1e8e52 dct:modified "2020-10-26T07:43:35.566Z"^^xsd:dateTime;
  skos:inScheme :conceptScheme_751925ed .

:c_bfc3ac08 dct:modified "2020-10-26T07:33:53.775Z"^^xsd:dateTime;
  skos:inScheme :conceptScheme_751925ed .

:c_0de6ed98 dct:modified "2020-10-25T06:27:22.230Z"^^xsd:dateTime;
  skos:inScheme :conceptScheme_751925ed .

:c_2ea90bc3 dct:modified "2020-10-26T07:18:32.123Z"^^xsd:dateTime;
  skos:inScheme :conceptScheme_751925ed .

:c_17d58c6d dct:modified "2020-10-25T06:27:31.963Z"^^xsd:dateTime;
  skos:inScheme :conceptScheme_751925ed .

:c_0ef5294b dct:modified "2020-10-26T07:39:08.805Z"^^xsd:dateTime;
  skos:inScheme :conceptScheme_751925ed .

:c_3a3a6363 dct:modified "2020-10-26T07:30:00.294Z"^^xsd:dateTime;
  skos:inScheme :conceptScheme_751925ed .

:c_3fa58f37 dct:modified "2020-10-26T07:32:06.808Z"^^xsd:dateTime;
  skos:inScheme :conceptScheme_751925ed .

:c_ee1dbf01 dct:modified "2020-10-26T07:38:24.827Z"^^xsd:dateTime;
  skos:inScheme :conceptScheme_751925ed .

:c_119d7903 dct:modified "2020-10-26T07:37:41.839Z"^^xsd:dateTime;
  skos:inScheme :conceptScheme_751925ed .

:c_9ab3dc4c dct:modified "2020-10-26T07:29:18.306Z"^^xsd:dateTime;
  skos:inScheme :conceptScheme_751925ed .

:c_d55b06b8 dct:modified "2020-10-26T07:34:33.284Z"^^xsd:dateTime;
  skos:inScheme :conceptScheme_751925ed .

:c_be620037 dct:modified "2020-10-26T07:42:11.041Z"^^xsd:dateTime;
  skos:inScheme :conceptScheme_751925ed .

:c_8c3e4b6f dct:modified "2020-10-25T06:28:38.650Z"^^xsd:dateTime;
  skos:inScheme :conceptScheme_751925ed .

:c_4a83bd38 dct:modified "2020-10-26T07:42:36.954Z"^^xsd:dateTime;
  skos:inScheme :conceptScheme_751925ed .

:c_7390c895 dct:modified "2020-10-26T07:23:55.969Z"^^xsd:dateTime;
  skos:inScheme :conceptScheme_751925ed .

:c_3a623af3 dct:modified "2020-10-26T07:34:07.183Z"^^xsd:dateTime;
  skos:inScheme :conceptScheme_751925ed .

:c_7f8af2c2 dct:modified "2020-10-26T07:41:01.784Z"^^xsd:dateTime;
  skos:inScheme :conceptScheme_751925ed .

:c_3e30efaf dct:modified "2020-10-28T15:17:13.392Z"^^xsd:dateTime;
  skos:inScheme :conceptScheme_751925ed .

:c_ed23b7cc dct:modified "2020-10-26T07:43:47.723Z"^^xsd:dateTime;
  skos:inScheme :conceptScheme_751925ed .

:c_0822f77e dct:modified "2020-10-28T15:15:03.177Z"^^xsd:dateTime;
  skos:editorialNote """Note: Terms shown with * are defined in
legislation, either in the Building Act 1984 or the
Building Regulations 2010, where the definition
may be fuller than the definition given here."""@en;
  skos:notation "*"@en .

:c_36ceda7d dct:modified "2020-10-26T07:44:45.155Z"^^xsd:dateTime;
  skos:editorialNote """Note: Terms shown with * are defined in
legislation, either in the Building Act 1984 or the
Building Regulations 2010, where the definition
may be fuller than the definition given here."""@en;
  skos:notation "*"@en;
  skos:prefLabel "earth-closet"@en .

:skosCollection_50d4bd2e skos:member :c_00af1bc5, :c_01839084, :c_0822f77e, :c_0cdb0b97,
    :c_0de6ed98, :c_0ef5294b, :c_119d7903, :c_17d58c6d, :c_1aa022f8, :c_1b2db6bc, :c_22764bab,
    :c_229f83e8, :c_22c38d73, :c_252b3da8, :c_2ea90bc3, :c_316d73a9, :c_36ceda7d, :c_39f68990,
    :c_3a3a6363, :c_3a623af3, :c_3b6a6b21, :c_3e30efaf, :c_3f5a9958, :c_3fa58f37, :c_41ebf78a,
    :c_47b084b0, :c_4a4a5b61, :c_4a83bd38, :c_53d35017, :c_62dfaa11, :c_66727700, :c_7390c895,
    :c_75f221c0, :c_86cbd31f, :c_870f938c, :c_873f1974, :c_8c3e4b6f, :c_8caf9cc1, :c_99150200,
    :c_9ab3dc4c, :c_9e940521, :c_a1430501, :c_a5feab63, :c_a794f4c0, :c_b1f8943d, :c_be620037,
    :c_bfc3ac08, :c_cb024dd1, :c_ced9eb5e, :c_cf1e8e52, :c_d55b06b8, :c_d67339c2, :c_dcbadafe,
    :c_e146ab76, :c_e2afc611, :c_e47ea7fb, :c_e4d9fbd5, :c_e9c0c7da, :c_ed23b7cc, :c_ee1dbf01,
    :c_ee888332, :c_f7036f54, :c_f8b75f3a, :c_fec9943e .

:c_fec9943e dct:modified "2020-10-26T07:24:49.568Z"^^xsd:dateTime;
  skos:editorialNote """Note: Terms shown with * are defined in
legislation, either in the Building Act 1984 or the
Building Regulations 2010, where the definition
may be fuller than the definition given here."""@en;
  skos:notation "*"@en;
  skos:prefLabel "room for residential purposes"@en .

:c_1b2db6bc dct:modified "2020-10-26T07:28:14.032Z"^^xsd:dateTime;
  skos:editorialNote """Note: Terms shown with * are defined in
legislation, either in the Building Act 1984 or the
Building Regulations 2010, where the definition
may be fuller than the definition given here."""@en;
  skos:notation "*"@en;
  skos:prefLabel "sanitary convenience"@en .

:c_3d59dac9 dct:modified "2020-10-26T07:41:15.460Z"^^xsd:dateTime;
  skos:editorialNote """Note: Terms shown with * are defined in
legislation, either in the Building Act 1984 or the
Building Regulations 2010, where the definition
may be fuller than the definition given here."""@en;
  skos:notation "*"@en;
  skos:prefLabel "softened wholesome water"@en .

:c_9d5baa50 dct:modified "2020-10-26T07:37:00.801Z"^^xsd:dateTime;
  skos:editorialNote """Note: Terms shown with * are defined in
legislation, either in the Building Act 1984 or the
Building Regulations 2010, where the definition
may be fuller than the definition given here."""@en;
  skos:notation "*"@en;
  skos:prefLabel "water-closet (wc)"@en .

:c_e146ab76 dct:modified "2020-10-25T07:03:16.838Z"^^xsd:dateTime .

:c_16ea33d2 a skos:Concept;
  dct:created "2020-10-25T08:38:05.473Z"^^xsd:dateTime;
  dct:modified "2020-10-25T08:41:26.894Z"^^xsd:dateTime;
  skos:broader :c_be604dfa;
  skos:definition """* This approved document gives guidance for compliance with the Building Regulations for building
work carried out in England. It also applies to building work carried out on excepted energy
buildings in Wales as defined in the Welsh Ministers (Transfer of Functions) (No. 2) Order 2009."""@en;
  skos:inScheme :conceptScheme_751925ed;
  skos:narrower :c_b7d8c7ee;
  skos:prefLabel "protection from falling, collision and impact 2013 edition – for use in England*"@en .

:c_be604dfa dct:modified "2020-10-25T08:38:34.390Z"^^xsd:dateTime;
  skos:narrower :c_16ea33d2 .

:c_b7d8c7ee a skos:Concept;
  dct:created "2020-10-25T08:40:53.062Z"^^xsd:dateTime;
  skos:broader :c_16ea33d2;
  skos:definition "The following are key terms used in this document:"@en;
  skos:inScheme :conceptScheme_751925ed;
  skos:prefLabel "appendix a: key terms (adk)"@en .

:c_2d35a0e4 a skos:Concept;
  skos:broader :c_b7d8c7ee;
  skos:definition "An entrance which is accessible to people regardless of disability, age or gender."@en;
  skos:prefLabel "accessible entrance"@en .

:c_d3c63474 a skos:Concept;
  skos:broader :c_b7d8c7ee;
  skos:definition "A stair with paddle-shaped treads where the wide portion is on alternate sides on consecutive treads (see paragraphs 1.29 and 1.30)."@en;
  skos:prefLabel "alternating tread stair"@en .

:c_c9535965 a skos:Concept;
  skos:broader :c_b7d8c7ee;
  skos:definition "A structure – either a raised rail or a solid wall – that denies access to another area."@en;
  skos:prefLabel "barrier"@en .

:c_bf5868a2 a skos:Concept;
  skos:broader :c_b7d8c7ee;
  skos:definition "Serving more than one dwelling. "@en;
  skos:prefLabel "common stair (adk)"@en .

:c_22ca257a a skos:Concept;
  skos:broader :c_b7d8c7ee;
  skos:definition "The perception of a visual difference between two elements of the building, or fittings within the building, so that the difference in light reflectance value is of sufficient points to distinguish between the two elements."@en;
  skos:prefLabel "contrast visually"@en .

:c_b93c6e7e a skos:Concept;
  skos:broader :c_b7d8c7ee;
  skos:definition "A continuous series of steps or a continuous slope (ramp) between landings. (For the widths and lengths of flights see paragraphs 1.14–1.24.)"@en;
  skos:prefLabel "flight"@en .

:c_a9d47a76 a skos:Concept;
  dct:modified "2020-10-25T09:02:18.402Z"^^xsd:dateTime;
  skos:broader :c_b7d8c7ee;
  skos:definition "A stair intended for all users of a building on a day-to-day basis, as a normal route between levels."@en;
  skos:inScheme :conceptScheme_751925ed;
  skos:prefLabel "general access stair"@en .

:c_28dbd28f a skos:Concept;
  dct:modified "2020-10-25T09:02:27.555Z"^^xsd:dateTime;
  skos:broader :c_b7d8c7ee;
  skos:definition "For stairs: the depth from front to back of a tread, less any overlap with the next tread above (see paragraphs 1.2 and 1.3). (For the measurement of the going on tapered treads see paragraphs 1.25– 1.27.) For ramps: the length of the ramp between landings."@en;
  skos:inScheme :conceptScheme_751925ed;
  skos:prefLabel "going"@en .

:c_5d93d9fd a skos:Concept;
  skos:broader :c_b7d8c7ee;
  skos:definition "A barrier that denies pedestrians or vehicles access to another area, for example the floor below (see Diagrams 3.1 and 3.2)."@en;
  skos:prefLabel "guarding"@en .

:c_f902cb9b a skos:Concept;
  dct:modified "2020-10-25T09:02:12.811Z"^^xsd:dateTime;
  skos:broader :c_b7d8c7ee;
  skos:definition "A rail, at hand height or a little higher, for people to hold for support. (For handrails for stairs, see paragraphs 1.34–1.37; for handrails for ramps, see paragraphs 2.11–2.12.)"@en;
  skos:inScheme :conceptScheme_751925ed;
  skos:prefLabel "handrail"@en .

:c_c412c788 a skos:Concept;
  dct:modified "2020-10-25T09:02:56.193Z"^^xsd:dateTime;
  skos:broader :c_b7d8c7ee;
  skos:definition "A stair in a helix around a central void (see paragraph 1.28)."@en;
  skos:inScheme :conceptScheme_751925ed;
  skos:prefLabel "helical stair"@en .

:c_4bf44d19 a skos:Concept;
  dct:modified "2020-10-25T09:02:30.316Z"^^xsd:dateTime;
  skos:broader :c_b7d8c7ee;
  skos:definition "A means of access to another level, formed by a series of rungs or narrow treads. People normally ascend or descend facing the ladder. (See paragraphs 1.31–1.33.)"@en;
  skos:inScheme :conceptScheme_751925ed;
  skos:prefLabel "ladder"@en .

:c_3c4ca936 a skos:Concept;
  dct:modified "2020-10-25T09:03:18.170Z"^^xsd:dateTime;
  skos:broader :c_b7d8c7ee;
  skos:definition "The total quantity of visible light reflected by a surface at all wavelengths and directions when illuminated by a light source."@en;
  skos:inScheme :conceptScheme_751925ed;
  skos:prefLabel "light reflectance value (lrv)"@en .

:c_b21555ba a skos:Concept;
  dct:modified "2020-10-25T09:02:45.116Z"^^xsd:dateTime;
  skos:broader :c_b7d8c7ee;
  skos:definition "The leading edge of a stair tread. "@en;
  skos:inScheme :conceptScheme_751925ed;
  skos:prefLabel "nosing"@en .

:c_d287c321 a skos:Concept;
  dct:modified "2020-10-25T09:03:02.179Z"^^xsd:dateTime;
  skos:broader :c_b7d8c7ee;
  skos:definition "The angle of inclination (slope) between the horizontal and a line connecting the nosings of a stair."@en;
  skos:inScheme :conceptScheme_751925ed;
  skos:prefLabel "pitch"@en .

:c_c67b07d9 a skos:Concept;
  dct:modified "2020-10-25T09:02:09.354Z"^^xsd:dateTime;
  skos:broader :c_b7d8c7ee;
  skos:definition "A stair intended to be used for only one dwelling. "@en;
  skos:inScheme :conceptScheme_751925ed;
  skos:prefLabel "private stair"@en .

:c_4c4cb482 a skos:Concept;
  dct:modified "2020-10-25T09:02:36.919Z"^^xsd:dateTime;
  skos:broader :c_b7d8c7ee;
  skos:definition "An entrance which a visitor not familiar with the building would normally expect to approach. "@en;
  skos:inScheme :conceptScheme_751925ed;
  skos:prefLabel "principal entrance"@en .

:c_b45c8cb2 a skos:Concept;
  dct:modified "2020-10-25T09:02:21.630Z"^^xsd:dateTime;
  skos:broader :c_b7d8c7ee;
  skos:definition "A gangway at an angle to the rows of seats/wheelchair spaces or a stepped gangway in tiered seating."@en;
  skos:inScheme :conceptScheme_751925ed;
  skos:prefLabel "radial gangway"@en .

:c_49fde689 a skos:Concept;
  dct:modified "2020-10-25T09:02:39.736Z"^^xsd:dateTime;
  skos:broader :c_b7d8c7ee;
  skos:definition "A slope steeper than 1:20, on which a pedestrian or wheelchair user can move from one level to another (see Section 2)."@en;
  skos:inScheme :conceptScheme_751925ed;
  skos:prefLabel "ramp"@en .

:c_5e6f602a a skos:Concept;
  dct:modified "2020-10-25T09:02:33.682Z"^^xsd:dateTime;
  skos:broader :c_b7d8c7ee;
  skos:definition "The height between consecutive treads (see paragraphs 1.2 and 1.3). For ramps: the vertical distance between each end of the ramp flight."@en;
  skos:inScheme :conceptScheme_751925ed;
  skos:prefLabel "rise"@en .

:c_a5feab63 a skos:Concept;
  dct:modified "2020-10-25T09:02:15.606Z"^^xsd:dateTime;
  skos:broader :c_b7d8c7ee;
  skos:definition "A stair in a helix around a central column (see paragraph 1.28)."@en;
  skos:inScheme :conceptScheme_751925ed;
  skos:prefLabel "spiral stair"@en .

:c_78459267 a skos:Concept;
  dct:modified "2020-10-25T09:02:05.570Z"^^xsd:dateTime;
  skos:broader :c_b7d8c7ee;
  skos:definition "The clear width between the walls or balustrades. "@en;
  skos:inScheme :conceptScheme_751925ed;
  skos:prefLabel "stair width"@en .

:c_272d3c0a a skos:Concept;
  dct:modified "2020-10-25T09:02:59.137Z"^^xsd:dateTime;
  skos:broader :c_b7d8c7ee;
  skos:definition "A step in which the going reduces from one side to the other (see paragraphs 1.25–1.27). "@en;
  skos:inScheme :conceptScheme_751925ed;
  skos:prefLabel "tapered tread"@en .

:c_4010d5b9 a skos:Concept;
  dct:modified "2020-10-25T09:02:02.615Z"^^xsd:dateTime;
  skos:broader :c_b7d8c7ee;
  skos:definition "A flat gangway parallel to the rows of seating/wheelchair spaces."@en;
  skos:inScheme :conceptScheme_751925ed;
  skos:prefLabel "transverse gangway"@en .

:c_f2f44aa9 a skos:Concept;
  dct:modified "2020-10-25T09:02:24.856Z"^^xsd:dateTime;
  skos:broader :c_b7d8c7ee;
  skos:definition "A stair used for escape, access for maintenance, or purposes other than as the usual route for moving between levels on a day-to-day basis."@en;
  skos:inScheme :conceptScheme_751925ed;
  skos:prefLabel "utility stair"@en .

:c_2ca7a450 a skos:Concept;
  dct:modified "2020-10-25T09:03:11.860Z"^^xsd:dateTime;
  skos:broader :c_b7d8c7ee;
  skos:definition "Storey exits provided within the body of a seating layout."@en;
  skos:inScheme :conceptScheme_751925ed;
  skos:prefLabel "vomitory exits"@en .

:c_b93c6e7e dct:modified "2020-10-25T09:02:42.445Z"^^xsd:dateTime;
  skos:inScheme :conceptScheme_751925ed .

:c_c9535965 dct:modified "2020-10-25T09:02:47.854Z"^^xsd:dateTime;
  skos:inScheme :conceptScheme_751925ed .

:c_22ca257a dct:modified "2020-10-25T09:02:50.221Z"^^xsd:dateTime;
  skos:inScheme :conceptScheme_751925ed .

:c_bf5868a2 dct:modified "2020-10-28T14:50:01.345Z"^^xsd:dateTime;
  skos:inScheme :conceptScheme_751925ed .

:c_2d35a0e4 dct:modified "2020-10-26T07:30:16.215Z"^^xsd:dateTime;
  skos:inScheme :conceptScheme_751925ed .

:c_d3c63474 dct:modified "2020-10-25T09:03:07.980Z"^^xsd:dateTime;
  skos:inScheme :conceptScheme_751925ed .

:c_5d93d9fd dct:modified "2020-10-25T09:03:15.218Z"^^xsd:dateTime;
  skos:inScheme :conceptScheme_751925ed .

:c_b7d8c7ee dct:modified "2020-10-25T09:04:42.246Z"^^xsd:dateTime;
  skos:narrower :c_22ca257a, :c_272d3c0a, :c_28dbd28f, :c_2ca7a450, :c_2d35a0e4, :c_3c4ca936,
    :c_4010d5b9, :c_49fde689, :c_4bf44d19, :c_4c4cb482, :c_5d93d9fd, :c_5e6f602a, :c_78459267,
    :c_a5feab63, :c_a9d47a76, :c_b21555ba, :c_b45c8cb2, :c_b93c6e7e, :c_bf5868a2, :c_c412c788,
    :c_c67b07d9, :c_c9535965, :c_d287c321, :c_d3c63474, :c_f2f44aa9, :c_f902cb9b .

:skosCollection_50d4bd2e skos:member :c_07abc5c2, :c_0c33e781, :c_0db511ab, :c_1166f883,
    :c_22ca257a, :c_272d3c0a, :c_28dbd28f, :c_2a1002d3, :c_2bb3748c, :c_3262a30a, :c_345811e8,
    :c_34c7d4e3, :c_3b310e19, :c_3b5778ee, :c_3c4ca936, :c_3d888dc1, :c_3fc6a13d, :c_4010d5b9,
    :c_438bd78a, :c_49fde689, :c_4b4c9739, :c_4bf44d19, :c_4c4cb482, :c_4cb28fa4, :c_4f47aeea,
    :c_588bf28f, :c_5aa42901, :c_5bb42f0e, :c_5d93d9fd, :c_5e6f602a, :c_61aec10c, :c_6badbeaf,
    :c_6ed11205, :c_70a0403c, :c_78459267, :c_8144317d, :c_81482951, :c_895306c7, :c_8abc2fd9,
    :c_8c6a9923, :c_8f476b03, :c_93488b6d, :c_95d3756f, :c_9a21f5a2, :c_a9d47a76, :c_aa316632,
    :c_ac95ba41, :c_b21555ba, :c_b3eb4d7b, :c_b4273037, :c_b45c8cb2, :c_b93c6e7e, :c_bf5868a2,
    :c_c13a7c46, :c_c2902dec, :c_c412c788, :c_c57961a6, :c_c67b07d9, :c_c8566bf0, :c_c878dbda,
    :c_c9535965, :c_cbfc0947, :c_d26ff5d2, :c_d287c321, :c_d3c63474, :c_d68c8ade, :c_da4b364b,
    :c_e43f1fcb, :c_e6d846bf, :c_e85e2d31, :c_f213d52c, :c_f2f44aa9, :c_f3cee240, :c_f40ac57b,
    :c_f902cb9b, :c_fa726c7b .

:c_e7aee361 a skos:Concept;
  dct:created "2020-10-26T05:33:49.239Z"^^xsd:dateTime;
  dct:modified "2020-10-26T07:04:15.510Z"^^xsd:dateTime;
  skos:broader :c_f68328a2;
  skos:inScheme :conceptScheme_751925ed;
  skos:narrower :c_70908a07, :c_ae74ec82 .

:c_29cf7b46 dct:modified "2020-10-26T07:00:50.727Z"^^xsd:dateTime;
  skos:broader :c_70908a07;
  skos:inScheme :conceptScheme_751925ed;
  skos:note """Note: Sub-paragraph c means that, for example, the presence of a small flat for a manager in a large non-domestic building does not result in the whole building being treated as a dwelling.
Similarly, if a room is used as an office or utility space within a dwelling, that does not mean that the building should not be treated as a dwelling."""@en .

:c_f68328a2 skos:definition """* This approved document gives guidance for compliance with the Building Regulations for
building work carried out in England. It also applies to building work carried out on excepted
energy buildings in Wales as defined in the Welsh Ministers (Transfer of Functions) (No.2) Order
2009. This approved document also gives guidance applying to buildings of statutory undertakers
and of the Crown or carried out by Crown authorities in both England and Wales in respect of
regulations 25, 25A, 25B and 26."""@en;
  skos:narrower :c_e7aee361 .

:c_ae74ec82 a skos:Concept;
  dct:created "2020-10-26T05:36:13.809Z"^^xsd:dateTime;
  skos:broader :c_e7aee361;
  skos:inScheme :conceptScheme_751925ed;
  skos:narrower :c_2bb3748c, :c_4487e3fd, :c_4e2f4fd0;
  skos:note "The following are key terms used in this document:"@en;
  skos:prefLabel "appendix a: key terms and abbreviations"@en .

:c_70908a07 a skos:Concept;
  dct:created "2020-10-26T06:10:39.834Z"^^xsd:dateTime;
  skos:broader :c_e7aee361;
  skos:inScheme :conceptScheme_751925ed;
  skos:note "This approved document gives guidance on what, in ordinary circumstances, may be considered reasonable provision to comply with the requirements of regulations 26, 26A and 40 of, and Part L of Schedule 1 to, the Building Regulations for those creating new dwellings. In addition, this approved document gives guidance on how to comply with regulations 25A, 27, 27A, 43 and 44 of the Building Regulations and regulation 20 of the Building (Approved Inspectors etc.) Regulations 2010 where an approved inspector is the BCB."@en;
  skos:prefLabel "appendix b: types of work covered by this approved document"@en .

:c_9397feee a skos:Concept;
  dct:modified "2020-10-26T07:41:56.725Z"^^xsd:dateTime;
  skos:broader :c_ae74ec82;
  skos:definition "is the physical property used to measure airtightness of the building fabric. It is defined as air leakage rate per hour per square metre of envelope area at the test reference pressure differential of 50 pascals (50 N/m2). The envelope area, or measured part of the building, is the total area of all floors, walls and ceilings bordering the internal volume that is the subject of the pressure test. This includes walls and floors below external ground level. Overall internal dimensions are used to calculate this envelope area and no subtractions are made for the area of the junctions of internal walls, floors and ceilings with exterior walls, floors and ceilings."@en;
  skos:inScheme :conceptScheme_751925ed;
  skos:prefLabel "air permeability"@en .

:c_21b61df0 a skos:Concept;
  dct:modified "2020-10-28T15:16:56.596Z"^^xsd:dateTime;
  skos:broader :c_ae74ec82;
  skos:definition "is the worst allowable air permeability."@en;
  skos:inScheme :conceptScheme_751925ed;
  skos:prefLabel "limiting air permeability"@en-GB .

:c_75d877dd a skos:Concept;
  dct:modified "2020-10-26T07:44:00.398Z"^^xsd:dateTime;
  skos:broader :c_ae74ec82;
  skos:definition "is the target value set at the design stage, and must always be no worse than the limiting value."@en;
  skos:inScheme :conceptScheme_751925ed;
  skos:prefLabel "design air permeability"@en .

:c_c65780e9 a skos:Concept;
  dct:modified "2020-10-26T07:22:42.768Z"^^xsd:dateTime;
  skos:broader :c_ae74ec82;
  skos:definition "is the value used in establishing the DER and the DFEE rate, and is based on a specific measurement of the dwelling concerned or on measurements of other dwellings of the same dwelling type."@en;
  skos:inScheme :conceptScheme_751925ed;
  skos:note "NOTE: The envelope area of a terraced house includes the party wall(s). The envelope area of a flat in a multiple-storey building includes the floors, walls and ceilings which are shared with adjacent flats."@en;
  skos:prefLabel "assessed air permeability"@en .

:c_e3217f0c a skos:Concept;
  dct:modified "2020-10-26T06:50:06.671Z"^^xsd:dateTime;
  skos:broader :c_ae74ec82;
  skos:definition "is the advancement of a fixed building service after all or part of the system has been installed, replaced or altered. The system is taken from a state of static completion to working order. Testing and adjusting, as necessary, ensure that the whole system uses no more fuel and power than  is reasonable in the circumstances, without compromising the need to comply with health and safety requirements. For each system, commissioning includes the following: setting-to-work; regulation (that is, testing and adjusting repetitively) to achieve the specified performance; calibration, setting up and testing of the associated automatic control systems; and recording of the system settings and the performance test results that have been accepted as satisfactory."@en;
  skos:inScheme :conceptScheme_751925ed;
  skos:prefLabel "commissioning"@en .

:c_13c7985e a skos:Concept;
  dct:modified "2020-10-26T06:49:56.942Z"^^xsd:dateTime;
  skos:broader :c_ae74ec82;
  skos:definition "is the Dwelling CO2 Emission Rate expressed as kgCO2/(m2 year)."@en;
  skos:inScheme :conceptScheme_751925ed;
  skos:prefLabel "der"@en .

:c_96f4329c a skos:Concept;
  dct:modified "2020-10-26T07:21:08.623Z"^^xsd:dateTime;
  skos:broader :c_ae74ec82;
  skos:definition "is the dwelling fabric energy efficiency rate expressed as kWh/(m2.year). Dwelling means a self-contained unit designed to accommodate a single household."@en;
  skos:inScheme :conceptScheme_751925ed;
  skos:note "NOTE: Buildings exclusively containing rooms for residential purposes, such as nursing homes, student accommodation and similar, are not dwellings, and in such cases, Approved Document L2A applies."@en;
  skos:prefLabel "dfee rate"@en .

:c_63561321 a skos:Concept;
  dct:modified "2020-10-26T06:49:15.510Z"^^xsd:dateTime;
  skos:broader :c_ae74ec82;
  skos:definition "is the particular group allocated to each dwelling on a development to provide the basis for assessing the pressure testing regime. The allocation of each dwelling to a dwelling type should be the responsibility of the person carrying out the pressure testing. To be classed as of the same type, dwellings should: i. be of the same generic form (i.e. detached, semi-detached, end terrace, mid-terrace, ground- floor flat (including ground-floor maisonette), mid-floor flat, top-floor flat (including top-floor maisonette); iii. include the same number of storeys; iii have the same design air permeability; iiii have similar adjacency to unheated spaces such as stairwells, integral garages etc. v. have the same principal construction details vi. have a similar (i.e. 1) number of significant penetrations, i.e. for windows, doors, flues/ chimneys, supply/exhaust terminals, waste water pipes; vii. have envelope areas that do not differ by more than 10 per cent (see air permeability for a definition of envelope area)."@en;
  skos:inScheme :conceptScheme_751925ed;
  skos:prefLabel "dwelling type"@en .

:c_e382854e a skos:Concept;
  dct:modified "2020-10-26T06:49:53.674Z"^^xsd:dateTime;
  skos:broader :c_ae74ec82;
  skos:definition "is the Target CO2 Emission Rate expressed as kgCO2/(m2 year)."@en;
  skos:inScheme :conceptScheme_751925ed;
  skos:prefLabel "ter"@en .

:c_4487e3fd a skos:Concept;
  dct:modified "2020-10-26T06:49:12.580Z"^^xsd:dateTime;
  skos:broader :c_ae74ec82;
  skos:definition " is the Target Fabric Energy Efficiency rate expressed as kWh/(m2.year)."@en;
  skos:inScheme :conceptScheme_751925ed;
  skos:prefLabel "tfee"@en .

:c_42f32053 a skos:Concept;
  dct:modified "2020-10-26T06:50:15.968Z"^^xsd:dateTime;
  skos:broader :c_ae74ec82;
  skos:inScheme :conceptScheme_751925ed;
  skos:notation "brukl"@en;
  skos:prefLabel "building regulations uk part l"@en .

:c_63f653cb a skos:Concept;
  dct:modified "2020-10-26T06:49:36.714Z"^^xsd:dateTime;
  skos:broader :c_ae74ec82;
  skos:inScheme :conceptScheme_751925ed;
  skos:notation "ukas"@en;
  skos:prefLabel "united kingdom accreditation service"@en .

:c_2bb3748c a skos:Concept;
  dct:modified "2020-10-26T06:49:39.743Z"^^xsd:dateTime;
  skos:broader :c_ae74ec82;
  skos:inScheme :conceptScheme_751925ed;
  skos:notation "tfa"@en;
  skos:prefLabel "total floor area"@en .

:c_4e2f4fd0 a skos:Concept;
  dct:modified "2020-10-26T06:50:12.992Z"^^xsd:dateTime;
  skos:broader :c_ae74ec82;
  skos:inScheme :conceptScheme_751925ed;
  skos:notation "tmp"@en;
  skos:prefLabel "thermal mass parameter"@en .

:c_5ecea38f a skos:Concept;
  dct:modified "2020-10-26T07:25:43.946Z"^^xsd:dateTime;
  skos:broader :c_ae74ec82;
  skos:inScheme :conceptScheme_751925ed;
  skos:notation "sedbuk"@en;
  skos:prefLabel "seasonal efficiency of domestic boilers in the uk"@en .

:c_716e9379 a skos:Concept;
  dct:modified "2020-10-26T06:49:18.591Z"^^xsd:dateTime;
  skos:broader :c_ae74ec82;
  skos:inScheme :conceptScheme_751925ed;
  skos:notation "co2"@en;
  skos:prefLabel "carbon dioxide"@en .

:c_b9d06847 a skos:Concept;
  dct:modified "2020-10-28T15:19:52.989Z"^^xsd:dateTime;
  skos:broader :c_ae74ec82;
  skos:definition "The act of erecting a new dwelling is not a material change of use. Approved Document L1B applies where a dwelling is being created in an existing building as the result of a material change of use of all or part of the building."@en;
  skos:inScheme :conceptScheme_751925ed;
  skos:prefLabel "material changes of use"@en-GB .

:c_ab063a87 a skos:Concept;
  dct:modified "2020-10-26T06:58:33.948Z"^^xsd:dateTime;
  skos:broader :c_70908a07;
  skos:definition "When constructing a dwelling as part of a larger building that contains other types of accommodation, sometimes called a mixed-use development, use this Approved Document L1A for guidance in relation to each individual dwelling. Approved Document L2A gives guidance relating to the non-dwelling parts of such buildings, such as heated common areas, and in the case of mixed-use developments, the commercial or retail space."@en;
  skos:inScheme :conceptScheme_751925ed;
  skos:prefLabel "mixed-use developments"@en .

:c_1c9c5904 a skos:Concept;
  dct:modified "2020-10-26T06:58:50.851Z"^^xsd:dateTime;
  skos:broader :c_70908a07;
  skos:definition "The act of erecting a new dwelling is not a material change of use. Approved Document L1B applies where a dwelling is being created in an existing building as the result of a material change of use of all or part of the building."@en;
  skos:inScheme :conceptScheme_751925ed;
  skos:prefLabel "material changes of use"@en .

:c_ae74ec82 skos:narrower :c_13c7985e, :c_1c9c5904, :c_21b61df0, :c_42f32053, :c_5ecea38f,
    :c_63561321, :c_63f653cb, :c_716e9379, :c_75d877dd, :c_9397feee, :c_96f4329c, :c_ab063a87,
    :c_c65780e9, :c_e3217f0c, :c_e382854e .

:c_29cf7b46 a skos:Concept;
  skos:definition "If a unit contains both living accommodation and space to be used for commercial purposes (e.g. as a workshop or office), the whole unit should be treated as a dwelling, as long as the commercial part can revert to domestic use. This can be the case if, for example: a. there is direct access between the commercial space and the living accommodation; and b. both are contained within the same thermal envelope; and c. the living accommodation occupies a substantial proportion of the total area of the unit."@en;
  skos:prefLabel "live–work units"@en .

:c_e7aee361 skos:prefLabel "l1a conservation of fuel and power 2013 edition incorporating 2016 amendments – for use in England*"@en .

:c_70908a07 skos:narrower :c_1c9c5904, :c_29cf7b46 .

:c_a1430501 dct:modified "2020-10-26T07:17:54.434Z"^^xsd:dateTime;
  skos:prefLabel "controlled service or ﬁtting"@en .

:c_81ea9f13 skos:prefLabel "appendix a: key terms"@en .

:c_4161794e a skos:Concept;
  dct:created "2020-10-27T06:04:22.445Z"^^xsd:dateTime;
  skos:broader :c_f68328a2;
  skos:inScheme :conceptScheme_751925ed;
  skos:note """This Approved Document, which takes
effect on 1 October 2010, has been approved
and issued by the Secretary of State to provide
practical guidance on ways of complying with the
energy efficiency requirements (see Section 2)
and regulation 7 of the Building Regulations 2010
(SI 2010/2214) for England and Wales. Regulation
2(1) of the Building Regulations defines the energy
efficiency requirements as the requirements of
regulations 23, 25A, 25B, 26, 28 and 40 and Part
L of Schedule 1. The Building Regulations 2010
are referred to throughout the remainder of this
Document as ‘the Building Regulations’."""@en;
  skos:prefLabel "l2b conservation of fuel and power in existing buildings other than dwellings 2010 edition incorporating 2010, 2011, 2013 and 2016 amendments"@en .

:c_f68328a2 skos:narrower :c_4161794e .

:c_aca129a3 a skos:Concept;
  dct:created "2020-10-27T06:08:52.145Z"^^xsd:dateTime;
  skos:inScheme :conceptScheme_751925ed;
  skos:prefLabel "appendix a: key terms and abbreviations (l2a)"@en .

:skosCollection_50d4bd2e skos:member :c_5ecea38f, :c_e382854e, :c_f31dbf5c .

:c_13c34a40 a skos:Concept;
  dct:modified "2020-10-27T06:29:13.400Z"^^xsd:dateTime;
  skos:broader :c_aca129a3;
  skos:definition "is the worst allowable air permeability."@en;
  skos:inScheme :conceptScheme_751925ed;
  skos:prefLabel "limiting air permeability"@en .

:c_d64e2e84 a skos:Concept;
  dct:modified "2020-10-27T06:28:36.780Z"^^xsd:dateTime;
  skos:broader :c_aca129a3;
  skos:definition "is the Building CO2 Emission Rate expressed as kgCO2/(m2 year)."@en;
  skos:inScheme :conceptScheme_751925ed;
  skos:prefLabel "ber"@en .

:c_baf59db7 a skos:Concept;
  dct:modified "2020-10-27T06:28:48.281Z"^^xsd:dateTime;
  skos:broader :c_aca129a3;
  skos:definition "means an area of glazing, including glazed doors, intended for the display of products or services on offer within the building, positioned: a.at the external perimeter of the building; and b. at an access level; and c. immediately adjacent to a pedestrian thoroughfare. There should be no permanent workspace within one glazing height of the perimeter. Glazing more than 3 m above such an access level should not be considered part of a display window except: a. where the products on display require a greater height of glazing; b. in cases where building work involving changes to the façade and glazing requiring planning consent, where planners require a greater height of glazing, e.g. to fit with surrounding buildings or to match the character of the existing façade. It is expected that display windows will be found in planning Use Classes A1, A2, A3 and D2 as detailed in the table below."@en;
  skos:inScheme :conceptScheme_751925ed;
  skos:prefLabel "display window"@en .

:c_a6ddbdac a skos:Concept;
  dct:modified "2020-10-27T06:29:10.530Z"^^xsd:dateTime;
  skos:broader :c_aca129a3;
  skos:definition "means lighting intended to highlight displays of exhibits or merchandise, or lighting used in spaces for public leisure and entertainment such as dance halls, auditoria, conference halls, restaurants and cinemas"@en;
  skos:inScheme :conceptScheme_751925ed;
  skos:prefLabel "display lighting"@en .

:c_e85468f5 a skos:Concept;
  dct:modified "2020-10-27T06:28:58.203Z"^^xsd:dateTime;
  skos:broader :c_aca129a3;
  skos:definition "includes a dwelling-house and a flat and means a self-contained unit designed to accommodate a single household. Buildings exclusively containing rooms for residential purposes such as nursing homes, student accommodation and similar are not dwellings, and in such cases, this Approved Document L2A applies."@en;
  skos:inScheme :conceptScheme_751925ed;
  skos:prefLabel "dwelling (l2a)"@en .

:c_b468fcc4 a skos:Concept;
  dct:modified "2020-10-27T06:28:39.478Z"^^xsd:dateTime;
  skos:broader :c_aca129a3;
  skos:definition "means that part of emergency lighting that provides illumination for  the safety of people leaving an area or attempting to terminate a dangerous process before leaving an area"@en;
  skos:inScheme :conceptScheme_751925ed;
  skos:note "NOTE: In respect of new buildings other than dwellings, the applicable requirements are those of Part L and regulations 25A and 26"@en;
  skos:prefLabel "emergency escape lighting"@en .

:c_7e8f8302 a skos:Concept;
  dct:modified "2020-10-27T06:29:01.259Z"^^xsd:dateTime;
  skos:broader :c_aca129a3;
  skos:definition "means that work needed to complete the partitioning and building services within the external fabric of the building (the shell) to meet the specific needs of incoming occupiers. fit-out work can be carried out in whole or in parts: a. a. in the same project and time frame as the construction of the building shell; or b. a. at some time after the shell has been completed."@en;
  skos:inScheme :conceptScheme_751925ed;
  skos:prefLabel "fit-out work"@en .

:c_74e681f9 a skos:Concept;
  dct:modified "2020-10-27T06:28:55.440Z"^^xsd:dateTime;
  skos:broader :c_aca129a3;
  skos:definition "means a door to an entrance primarily for the use of people that is expected to experience large volumes of traffic, and where robustness and/or powered operation is the main performance requirement. To qualify as a high-usage entrance door, the door should be equipped with automatic closers and, except where operational requirements preclude it, be protected by a lobby."@en;
  skos:inScheme :conceptScheme_751925ed;
  skos:prefLabel "high-usage entrance door"@en .

:c_3350a84a a skos:Concept;
  dct:modified "2020-10-27T06:28:42.277Z"^^xsd:dateTime;
  skos:broader :c_aca129a3;
  skos:definition "means lighting intended to illuminate specialist tasks within a space, rather than the space itself. It could include theatre spotlights, projection equipment, lighting in TV and photographic studios, medical lighting in operating theatres and doctors’ and dentists’ surgeries, illuminated signs, coloured or stroboscopic lighting, and art objects with integral lighting such as sculptures, decorative fountains and chandeliers."@en;
  skos:inScheme :conceptScheme_751925ed;
  skos:prefLabel "specialist process lighting"@en .

:c_06d9104f a skos:Concept;
  dct:modified "2020-10-28T15:16:24.235Z"^^xsd:dateTime;
  skos:broader :c_aca129a3;
  skos:definition "is the total area of all enclosed spaces measured to the internal face of the external walls. In this convention: a. a. the area of sloping surfaces such as staircases, galleries, raked auditoria and tiered terraces should be taken as their area on plan; and b. a. areas that are not enclosed such as open floors, covered ways and balconies are excluded."@en;
  skos:inScheme :conceptScheme_751925ed;
  skos:note "NOTE: This area is the gross floor area as measured in accordance with the guidance issued to surveyors by the Royal Institution of Chartered Surveyors (RICS)."@en;
  skos:prefLabel "total useful floor area"@en-GB .

:c_9e56cd49 a skos:Concept;
  dct:modified "2020-10-27T06:29:27.009Z"^^xsd:dateTime;
  skos:broader :c_aca129a3;
  skos:inScheme :conceptScheme_751925ed;
  skos:notation "HVAC"@en;
  skos:prefLabel "heating, ventilation and air-conditioning"@en .

:c_2a4fc22e a skos:Concept;
  dct:modified "2020-10-27T06:29:04.683Z"^^xsd:dateTime;
  skos:broader :c_aca129a3;
  skos:inScheme :conceptScheme_751925ed;
  skos:notation "LZC"@en;
  skos:prefLabel "low and zero carbon"@en .

:c_6badbeaf a skos:Concept;
  dct:modified "2020-10-27T06:29:23.993Z"^^xsd:dateTime;
  skos:broader :c_aca129a3;
  skos:inScheme :conceptScheme_751925ed;
  skos:notation "SFP"@en;
  skos:prefLabel "specific fan power"@en .

:c_5d579e20 a skos:Concept;
  dct:modified "2020-10-27T06:29:16.391Z"^^xsd:dateTime;
  skos:broader :c_aca129a3;
  skos:inScheme :conceptScheme_751925ed;
  skos:notation "SEER"@en;
  skos:prefLabel "seasonal energy efficiency ratio"@en .

:c_f31dbf5c a skos:Concept;
  dct:modified "2020-10-27T08:35:50.450Z"^^xsd:dateTime;
  skos:broader :c_aca129a3;
  skos:inScheme :conceptScheme_751925ed;
  skos:notation "SSEER"@en .

:c_5e92bf81 a skos:Concept;
  dct:modified "2020-10-27T06:29:07.605Z"^^xsd:dateTime;
  skos:broader :c_aca129a3;
  skos:inScheme :conceptScheme_751925ed;
  skos:notation "FF"@en;
  skos:prefLabel "frame factor"@en .

:c_ba365c10 a skos:Concept;
  dct:modified "2020-10-27T06:28:45.149Z"^^xsd:dateTime;
  skos:broader :c_aca129a3;
  skos:inScheme :conceptScheme_751925ed;
  skos:notation "DX"@en;
  skos:prefLabel "direct exchange"@en .

:c_7abc215a skos:inScheme :conceptScheme_751925ed .

:c_aca129a3 dct:modified "2020-10-27T06:43:09.984Z"^^xsd:dateTime;
  skos:broader :c_8f28ad6e;
  skos:narrower :c_06d9104f, :c_13c34a40, :c_2a4fc22e, :c_3350a84a, :c_5d579e20, :c_5e92bf81,
    :c_6badbeaf, :c_74e681f9, :c_7e8f8302, :c_9e56cd49, :c_a6ddbdac, :c_b468fcc4, :c_ba365c10,
    :c_baf59db7, :c_d64e2e84, :c_e85468f5, :c_f31dbf5c .

:skosCollection_50d4bd2e skos:member :c_06d9104f, :c_13c34a40, :c_13c7985e, :c_1c9c5904,
    :c_1cfc2b23, :c_21b61df0, :c_247e4247, :c_2a4fc22e, :c_3350a84a, :c_352a7ba0, :c_42f32053,
    :c_4487e3fd, :c_4e2f4fd0, :c_5d579e20, :c_5e92bf81, :c_63561321, :c_63f653cb, :c_716e9379,
    :c_74e681f9, :c_75d877dd, :c_7e8f8302, :c_9397feee, :c_96f4329c, :c_9e56cd49, :c_a6ddbdac,
    :c_ab063a87, :c_b468fcc4, :c_b9d06847, :c_ba365c10, :c_baf59db7, :c_bb0d6dd0, :c_c65780e9,
    :c_d64e2e84, :c_e3217f0c, :c_e448e5c3, :c_e85468f5 .

:c_8f28ad6e a skos:Concept;
  dct:created "2020-10-27T06:38:09.688Z"^^xsd:dateTime;
  skos:broader :c_f68328a2;
  skos:inScheme :conceptScheme_751925ed;
  skos:prefLabel "l2a Conservation of fuel and power in new buildings other than dwellings 2013 edition incorporating 2016 amendments – for use in england*"@en .

:c_4161794e dct:modified "2020-10-27T06:48:26.172Z"^^xsd:dateTime;
  skos:narrowMatch :c_0aaf684b .

:c_f68328a2 dct:modified "2020-10-27T06:38:32.899Z"^^xsd:dateTime;
  skos:narrower :c_8f28ad6e .

:c_0aaf684b a skos:Concept;
  dct:created "2020-10-27T06:47:51.399Z"^^xsd:dateTime;
  skos:broader :c_4161794e;
  skos:inScheme :conceptScheme_751925ed;
  skos:prefLabel "key terms (l2b)"@en .

:c_247e4247 a skos:Concept;
  dct:modified "2020-10-27T07:01:19.763Z"^^xsd:dateTime;
  skos:broader :c_0aaf684b;
  skos:definition "means those energy efficiency improvements required by regulation 28."@en;
  skos:inScheme :conceptScheme_751925ed;
  skos:prefLabel "consequential improvements"@en .

:c_1cfc2b23 a skos:Concept;
  dct:modified "2020-10-27T08:36:16.565Z"^^xsd:dateTime;
  skos:broader :c_0aaf684b;
  skos:definition "means the amount of time it  will take to recover the initial investment through energy savings, and is calculated by dividing the marginal additional cost of implementing an energy efficiency measure by the value of the annual energy savings achieved by that measure taking no account of VAT. When making this calculation, the following guidance should be used:"@en;
  skos:inScheme :conceptScheme_751925ed;
  skos:prefLabel "simple payback"@en .

:c_352a7ba0 a skos:Concept;
  dct:modified "2020-10-27T08:36:43.215Z"^^xsd:dateTime;
  skos:broader :c_0aaf684b;
  skos:definition "means the work necessary to achieve the client’s purposes in extending the building and/or increasing the installed capacity of any fixed building services. The value of the principal works is the basis for determining a reasonable provision of consequential improvements. a. The marginal additional cost is the additional cost (materials and labour) of incorporating (e.g.) additional insulation, not the whole cost of the work. b. The cost of implementing the measure should be based on prices current at the date the proposals are made known to the BCB and be confirmed in a report signed by a suitably qualified person. c. The annual energy savings should be estimated using an energy calculation tool approved by the Secretary of State pursuant to regulation 24. d. For the purposes of this Approved Document, the energy prices that are current at the time of the application to building control should be used when evaluating the annual energy savings. Current energy prices can be obtained from the DECC website1."@en;
  skos:inScheme :conceptScheme_751925ed;
  skos:prefLabel "principal works"@en .

:c_e448e5c3 a skos:Concept;
  dct:modified "2020-10-27T08:36:03.272Z"^^xsd:dateTime;
  skos:broader :c_0aaf684b;
  skos:definition "is the total area of all enclosed spaces measured to the internal face  of the external walls, that is to say it is the gross floor area as measured in accordance with the guidance issued to surveyors by the RICS. In this convention: a. a. the area of sloping surfaces such as staircases, galleries, raked auditoria, and tiered terraces should be taken as their area on plan; and b. b. areas that are not enclosed such as open floors, covered ways and balconies are excluded. This equates to the gross floor area as measured in accordance with the guidance issued to surveyors by the RICS."@en;
  skos:inScheme :conceptScheme_751925ed;
  skos:note "Note that this definition encompasses the walls and floor of a swimming pool basin where this is part of an existing building"@en;
  skos:prefLabel "total useful floor area"@en .

:c_6a1a3775 a skos:Concept;
  dct:created "2020-10-27T07:03:59.856Z"^^xsd:dateTime;
  dct:modified "2020-10-27T07:58:25.743Z"^^xsd:dateTime;
  skos:broader :c_a20cbb62;
  skos:inScheme :conceptScheme_751925ed;
  skos:narrower :c_3cf43794;
  skos:prefLabel "access to and use of buildings volume 1: dwellings 2015 edition incorporating 2016 amendments for use in england*"@en .

:c_a20cbb62 skos:narrower :c_6a1a3775 .

:c_0109c085 dct:created "2020-10-27T16:36:09.588Z"^^xsd:dateTime .

:c_3cf43794 a skos:Concept;
  dct:created "2020-10-27T07:15:01.792Z"^^xsd:dateTime;
  skos:broader :c_6a1a3775;
  skos:inScheme :conceptScheme_751925ed;
  skos:note "Note: Terms shown with * are definition legislation, either in the Building Act 1984 or the Building Regulations 2010, where the definition may be fuller than the  definition given here."@en;
  skos:prefLabel "appendix a: key terms (adm1)"@en .

:c_7003e65c a skos:Concept;
  skos:broader :c_3cf43794;
  skos:definition "A threshold that is level or, if raised, has a total height of not more than 15mm, a minimum number of upstands and slopes and with any upstands higher than 5mm chamfered. Other acceptable solutions are described in Accessible thresholds in new housing – Guidance for house builders and developers, The Stationery Offi e Ltd. ISBN 0 11 702333 3. 1999."@en;
  skos:note "Note: Terms shown with * are definition legislation, either in the Building Act 1984 or the Building Regulations 2010, where the definition may be fuller than the  definition given here."@en;
  skos:prefLabel "accessible threshold"@en .

:c_6bf8d62f a skos:Concept;
  skos:broader :c_3cf43794;
  skos:definition "Internal or external path or corridor usually leading to the principal private entrance of a dwelling from a defined starting point (typically the pavement immediately outside of the curtilage or plot boundary)."@en;
  skos:prefLabel "approach route"@en .

:c_b630c168 a skos:Concept;
  skos:broader :c_3cf43794;
  skos:definition "A suitable sleeping area for one person. (A single bedroom provides one bedspace and a double or twin bedroom provides two bedspaces where these rooms also meet any other requirements for the relevant category of dwelling)."@en;
  skos:prefLabel "bedspace"@en .

:c_1d89066b a skos:Concept;
  skos:broader :c_3cf43794;
  skos:definition "Clear, unobstructed ‘pathway’ to access a window or other feature. Localised obstructions are not permitted unless specifically stated."@en;
  skos:prefLabel "clear access route"@en .

:c_f21d57e8 a skos:Concept;
  skos:broader :c_3cf43794;
  skos:definition "Clear, unobstructed space for access or manoeuvring. Localised obstructions are not permitted unless specifically stated."@en;
  skos:prefLabel "clear access zone"@en .

:c_7d70a254 a skos:Concept;
  skos:broader :c_3cf43794;
  skos:definition "Clear distance measured between the inside face of the doorframe (or door stop) and the face of the door when open at 90 degrees. Door furniture and ironmongery may be disregarded when measuring the clear opening width."@en;
  skos:prefLabel "clear opening width"@en .

:c_08556adc a skos:Concept;
  skos:broader :c_3cf43794;
  skos:definition "Clear floor space, represented by a circle, or an ellipse, that allows a wheelchair user to turn independently in a single movement. A door swing is permitted within a clear turning space unless stated otherwise."@en;
  skos:prefLabel "clear turning circle"@en .

:c_fcd25267 a skos:Concept;
  skos:broader :c_3cf43794;
  skos:definition "Clear distance measured between walls or other fixed obstructions (except permitted localised obstructions) or across a path. Skirtings totalling up to 50mm total thickness and shallow projecting ducts or casings above 1800mm may be discounted when measuring clear width."@en;
  skos:prefLabel "clear width"@en .

:c_09ab5f8e a skos:Concept;
  skos:broader :c_3cf43794;
  skos:definition "Shared area accessed by, or intended for the use of, more than one dwelling."@en;
  skos:prefLabel "communal or common (area, facilities or entrances)"@en .

:c_3d9928e0 a skos:Concept;
  skos:broader :c_3cf43794;
  skos:definition "The floor level (of the dwelling) on which the principal private entrance is located."@en;
  skos:prefLabel "entrance storey"@en .

:c_6dcae9b3 a skos:Concept;
  skos:broader :c_3cf43794;
  skos:definition "A house or flat. Student accommodation is treated as hotel/motel accommodation."@en;
  skos:notation "*"@en;
  skos:prefLabel "dwelling (adm1)"@en .

:c_5fcbc183 a skos:Concept;
  skos:broader :c_3cf43794;
  skos:definition "The surface of a door which follows into (or faces away from) the room or space into which the door is being opened – sometimes referred to as ‘the push side’."@en;
  skos:prefLabel "following edge (of door)"@en .

:c_00b6a69e a skos:Concept;
  skos:broader :c_3cf43794;
  skos:definition "Gradient between 1:60 and 1:20"@en;
  skos:prefLabel "gently sloping"@en .

:c_44e39791 a skos:Concept;
  dct:modified "2020-10-27T07:40:41.627Z"^^xsd:dateTime;
  skos:broader :c_3cf43794;
  skos:definition "Step-free area with no lips or upstands, suitable for showering, with a floor laid to shallow falls towards a floor gulley connected to the drainage system."@en;
  skos:inScheme :conceptScheme_751925ed;
  skos:prefLabel "installed level access shower"@en .

:c_283297ae a skos:Concept;
  skos:broader :c_3cf43794;
  skos:definition "The surface of a door which leads into (or faces) the room or space into which the door is being opened – sometimes referred to as ‘the pull side’"@en;
  skos:prefLabel "leading edge (of door)"@en .

:c_728f0bd1 a skos:Concept;
  dct:modified "2020-10-27T07:40:54.077Z"^^xsd:dateTime;
  skos:broader :c_3cf43794;
  skos:definition "Gradient not exceeding 1:60"@en;
  skos:inScheme :conceptScheme_751925ed;
  skos:prefLabel "level"@en .

:c_a5ffe780 a skos:Concept;
  skos:broader :c_3cf43794;
  skos:definition "Vertical route linking all floors of a dwelling accommodating (or capable of accommodating) a lift or lifting platform."@en;
  skos:prefLabel "liftway"@en .

:c_572989c8 a skos:Concept;
  dct:modified "2020-10-27T07:40:57.316Z"^^xsd:dateTime;
  skos:broader :c_3cf43794;
  skos:definition "Short, fixed element, such as a bollard lighting column or radiator, not more than 150mm deep that may intrude into a path, route, or corridor, that does not unduly restrict the passage of a wheelchair user."@en;
  skos:inScheme :conceptScheme_751925ed;
  skos:prefLabel "localised obstruction"@en .

:c_e0b7bab3 a skos:Concept;
  dct:modified "2020-10-27T07:41:00.019Z"^^xsd:dateTime;
  skos:broader :c_3cf43794;
  skos:definition "Clear floor space, represented by a rectangle which allows a wheelchair user to turn independently in a series of manoeuvres. A door swing is permitted within a clear manoeuvring space unless stated otherwise"@en;
  skos:inScheme :conceptScheme_751925ed;
  skos:prefLabel "manoeuvring space"@en .

:c_a3306811 a skos:Concept;
  skos:broader :c_3cf43794;
  skos:definition "A line that connects the nosing of the treads of a stair."@en;
  skos:prefLabel "pitch line"@en .

:c_8bff5d6c a skos:Concept;
  dct:modified "2020-10-27T07:40:38.057Z"^^xsd:dateTime;
  skos:broader :c_3cf43794;
  skos:definition "The gradient measured between the entrance storey finished floor level of the dwelling and the point of access."@en;
  skos:inScheme :conceptScheme_751925ed;
  skos:prefLabel "plot gradient"@en .

:c_cb235281 a skos:Concept;
  dct:modified "2020-10-27T07:41:03.084Z"^^xsd:dateTime;
  skos:broader :c_3cf43794;
  skos:definition "The point at which a person visiting a dwelling would normally get out of a car before approaching the dwelling. The point of access may be within or outside the plot."@en;
  skos:inScheme :conceptScheme_751925ed;
  skos:prefLabel "point of access"@en .

:c_917ae1af a skos:Concept;
  dct:modified "2020-10-27T07:41:23.006Z"^^xsd:dateTime;
  skos:broader :c_3cf43794;
  skos:definition "Space capable of providing a level access shower without the need to move walls, remove screed  or other solid flooring. It should include a capped- off floor gulley, set at an appropriate level and connected to the drainage system. (Usually provided within a wet room)."@en;
  skos:inScheme :conceptScheme_751925ed;
  skos:prefLabel "potential level access shower"@en .

:c_bb0d6dd0 a skos:Concept;
  dct:modified "2020-10-27T07:41:53.346Z"^^xsd:dateTime;
  skos:broader :c_3cf43794;
  skos:definition "The communal entrance (to the core of the building containing the dwelling) which a visitor not familiar with the building would normally expect to approach (usually the common entrance to the core of a block of flats)."@en;
  skos:inScheme :conceptScheme_751925ed;
  skos:prefLabel "principal communal entrance"@en .

:c_f90cac15 a skos:Concept;
  dct:modified "2020-10-27T07:41:29.163Z"^^xsd:dateTime;
  skos:broader :c_3cf43794;
  skos:definition "The entrance to the individual dwelling that a visitor not familiar with the dwelling would normally approach (usually the ‘front door’ to a house or ground floor flat)."@en;
  skos:inScheme :conceptScheme_751925ed;
  skos:prefLabel "principal private entrance"@en .

:c_b9882564 a skos:Concept;
  dct:modified "2020-10-27T07:41:37.993Z"^^xsd:dateTime;
  skos:broader :c_3cf43794;
  skos:definition "The floor level (of the dwelling) on which the main living space is located, where this is not the entrance storey."@en;
  skos:inScheme :conceptScheme_751925ed;
  skos:prefLabel "principal storey"@en .

:c_8a096c20 a skos:Concept;
  dct:modified "2020-10-27T07:42:06.138Z"^^xsd:dateTime;
  skos:broader :c_3cf43794;
  skos:definition "Area belonging to an individual dwelling."@en;
  skos:inScheme :conceptScheme_751925ed;
  skos:prefLabel "private (area, facilities or entrances)"@en .

:c_c12dc11d a skos:Concept;
  dct:modified "2020-10-27T07:40:29.092Z"^^xsd:dateTime;
  skos:broader :c_3cf43794;
  skos:definition "Gradient between 1:20 and 1:12"@en;
  skos:inScheme :conceptScheme_751925ed;
  skos:prefLabel "ramped"@en .

:c_089706ad a skos:Concept;
  dct:modified "2020-10-27T07:42:15.960Z"^^xsd:dateTime;
  skos:broader :c_3cf43794;
  skos:definition "A parking bay 2.4m wide x 4.8m long"@en;
  skos:inScheme :conceptScheme_751925ed;
  skos:prefLabel "standard parking bay"@en .

:c_d4fd4da6 a skos:Concept;
  dct:modified "2020-10-27T07:41:09.137Z"^^xsd:dateTime;
  skos:broader :c_3cf43794;
  skos:definition "A plot where the gradient exceeds 1:15."@en;
  skos:inScheme :conceptScheme_751925ed;
  skos:prefLabel "steeply sloping plot"@en .

:c_4eca6bbf a skos:Concept;
  dct:modified "2020-10-27T07:40:47.779Z"^^xsd:dateTime;
  skos:broader :c_3cf43794;
  skos:definition "Route without steps but that may include a ramp or a lift suitable for a wheelchair user."@en;
  skos:inScheme :conceptScheme_751925ed;
  skos:prefLabel "step-free"@en .

:c_0bf85e96 a skos:Concept;
  dct:modified "2020-10-27T07:41:17.160Z"^^xsd:dateTime;
  skos:broader :c_3cf43794;
  skos:definition "External ground surface that is firm, even, smooth enough to be wheeled over, is not covered with loose laid materials such as gravel and shingle, and has a maximum crossfall of 1:40."@en;
  skos:inScheme :conceptScheme_751925ed;
  skos:prefLabel "suitable ground surface"@en .

:c_1ca5a508 a skos:Concept;
  dct:modified "2020-10-27T07:41:34.935Z"^^xsd:dateTime;
  skos:broader :c_3cf43794;
  skos:definition "Nosings that conform with one of the options shown in Diagram 1.2 of Approved Document K"@en;
  skos:inScheme :conceptScheme_751925ed;
  skos:prefLabel "suitable tread nosings"@en .

:c_9797ec63 a skos:Concept;
  dct:modified "2020-10-27T07:42:09.634Z"^^xsd:dateTime;
  skos:broader :c_3cf43794;
  skos:definition "Category 3 dwelling constructed to be suitable for immediate occupation by a wheelchair user where the planning authority specifies that optional requirement M4(3)(2)(b) applies."@en;
  skos:inScheme :conceptScheme_751925ed;
  skos:prefLabel "wheelchair accessible"@en .

:c_2eabf3c7 a skos:Concept;
  dct:modified "2020-10-27T07:42:12.922Z"^^xsd:dateTime;
  skos:broader :c_3cf43794;
  skos:definition "Category 3 dwelling constructed with the potential to be adapted for occupation by a wheelchair user where optional requirement M4(3)(2)(a) applies."@en;
  skos:inScheme :conceptScheme_751925ed;
  skos:prefLabel "wheelchair adaptable"@en .

:c_db39fc1a a skos:Concept;
  dct:modified "2020-10-28T15:18:11.490Z"^^xsd:dateTime;
  skos:broader :c_3cf43794;
  skos:definition "WC or bathroom compartment with tanking and drainage laid to fall to a connected gulley capable of draining the floor area when used as a shower."@en;
  skos:inScheme :conceptScheme_751925ed;
  skos:prefLabel "wet room"@en-GB .

:c_b630c168 dct:modified "2020-10-27T07:40:31.921Z"^^xsd:dateTime;
  skos:inScheme :conceptScheme_751925ed .

:c_6dcae9b3 dct:modified "2020-10-27T07:40:35.360Z"^^xsd:dateTime;
  skos:inScheme :conceptScheme_751925ed .

:c_1d89066b dct:modified "2020-10-27T07:40:45.038Z"^^xsd:dateTime;
  skos:inScheme :conceptScheme_751925ed .

:c_fcd25267 dct:modified "2020-10-27T07:40:51.011Z"^^xsd:dateTime;
  skos:inScheme :conceptScheme_751925ed .

:c_09ab5f8e dct:modified "2020-10-27T07:41:06.232Z"^^xsd:dateTime;
  skos:inScheme :conceptScheme_751925ed .

:c_5fcbc183 dct:modified "2020-10-27T07:41:11.850Z"^^xsd:dateTime;
  skos:inScheme :conceptScheme_751925ed .

:c_7003e65c dct:modified "2020-10-27T07:41:14.583Z"^^xsd:dateTime;
  skos:inScheme :conceptScheme_751925ed .

:c_6bf8d62f dct:modified "2020-10-27T07:41:20.070Z"^^xsd:dateTime;
  skos:inScheme :conceptScheme_751925ed .

:c_3d9928e0 dct:modified "2020-10-27T07:41:25.887Z"^^xsd:dateTime;
  skos:inScheme :conceptScheme_751925ed .

:c_08556adc dct:modified "2020-10-27T07:41:40.864Z"^^xsd:dateTime;
  skos:inScheme :conceptScheme_751925ed .

:c_00b6a69e dct:modified "2020-10-27T07:41:43.644Z"^^xsd:dateTime;
  skos:inScheme :conceptScheme_751925ed .

:c_7d70a254 dct:modified "2020-10-27T07:41:47.023Z"^^xsd:dateTime;
  skos:inScheme :conceptScheme_751925ed .

:c_a3306811 dct:modified "2020-10-27T07:41:49.761Z"^^xsd:dateTime;
  skos:inScheme :conceptScheme_751925ed .

:c_a5ffe780 dct:modified "2020-10-27T07:41:56.380Z"^^xsd:dateTime;
  skos:inScheme :conceptScheme_751925ed .

:c_f21d57e8 dct:modified "2020-10-27T07:41:59.665Z"^^xsd:dateTime;
  skos:inScheme :conceptScheme_751925ed .

:c_283297ae dct:modified "2020-10-27T07:42:02.710Z"^^xsd:dateTime;
  skos:inScheme :conceptScheme_751925ed .

:c_3cf43794 dct:modified "2020-10-27T07:44:07.827Z"^^xsd:dateTime;
  skos:narrower :c_00b6a69e, :c_08556adc, :c_089706ad, :c_09ab5f8e, :c_0bf85e96, :c_1ca5a508,
    :c_1d89066b, :c_283297ae, :c_2eabf3c7, :c_3d9928e0, :c_44e39791, :c_4eca6bbf, :c_572989c8,
    :c_5fcbc183, :c_6bf8d62f, :c_6dcae9b3, :c_7003e65c, :c_728f0bd1, :c_7d70a254, :c_8a096c20,
    :c_8bff5d6c, :c_917ae1af, :c_9797ec63, :c_a3306811, :c_a5ffe780, :c_b630c168, :c_b9882564,
    :c_bb0d6dd0, :c_c12dc11d, :c_cb235281, :c_d4fd4da6, :c_db39fc1a, :c_e0b7bab3, :c_f21d57e8,
    :c_f90cac15, :c_fcd25267 .

:skosCollection_50d4bd2e skos:member :c_00b6a69e, :c_08556adc, :c_089706ad, :c_09ab5f8e,
    :c_0bf85e96, :c_1ca5a508, :c_283297ae, :c_2eabf3c7, :c_3d9928e0, :c_44e39791, :c_4eca6bbf,
    :c_572989c8, :c_5fcbc183, :c_6bf8d62f, :c_6dcae9b3, :c_7003e65c, :c_728f0bd1, :c_7d70a254,
    :c_8a096c20, :c_8bff5d6c, :c_917ae1af, :c_9797ec63, :c_a3306811, :c_a5ffe780, :c_b630c168,
    :c_b9882564, :c_c12dc11d, :c_cb235281, :c_d4fd4da6, :c_db39fc1a, :c_e0b7bab3, :c_f21d57e8,
    :c_f90cac15, :c_fcd25267 .

:c_7abc215a a skos:Concept;
  skos:broader :c_3da44764;
  skos:definition "‘should’ is used to indicate what to do to comply with legal requirements which are qualified by terms such as ‘so far as reasonably practicable’."@en;
  skos:prefLabel "should"@en .

:c_aae4241b a skos:Concept;
  dct:modified "2020-10-28T15:21:51.311Z"^^xsd:dateTime;
  skos:broader :c_3da44764;
  skos:definition "management of health and safety at work regulations 1999"@en;
  skos:inScheme :conceptScheme_751925ed;
  skos:prefLabel "the management regulations"@en .

:c_58bdb729 skos:inScheme :conceptScheme_751925ed;
  skos:notation "LWIT"@en;
  skos:prefLabel "leadership and worker involvement toolkit"@en .

:c_2689a172 a skos:Concept;
  skos:broader :c_3da44764;
  skos:definition "SSIP"@en;
  skos:inScheme :conceptScheme_751925ed;
  skos:prefLabel "safety schemes in procurement"@en .

:c_da4c39b1 a skos:Concept;
  skos:broader :c_3da44764;
  skos:inScheme :conceptScheme_751925ed;
  skos:notation "ORR"@en;
  skos:prefLabel "office of rail regulation"@en .

:c_366cf430 a skos:Concept;
  dct:modified "2020-10-28T15:22:15.744Z"^^xsd:dateTime;
  skos:broader :c_3da44764;
  skos:definition "balancing the level of risk against the measures needed to control the real risk in terms of money, time or trouble. However, you do not need to take action if it would be grossly disproportionate to the level of risk (see www.gov.uk/risk/faq.htm for the most up-to-date explanation of what ‘reasonably practicable’ means.)"@en;
  skos:inScheme :conceptScheme_751925ed;
  skos:prefLabel "reasonably practicable"@en .

:c_a9823a22 skos:prefLabel "responsible person"@en .

:c_3454d214 a skos:Concept;
  skos:broader :c_3da44764;
  skos:definition "‘must’ is used only where there is an absolute duty, ie an explicit legal requirement to take a certain action which is not qualified by terms such as ‘so far as reasonably practicable’"@en;
  skos:inScheme :conceptScheme_751925ed;
  skos:prefLabel "must"@en .

:c_08eb88d2 a skos:Concept;
  dct:modified "2020-10-28T15:21:36.143Z"^^xsd:dateTime;
  skos:broader :c_3da44764;
  skos:definition "means the belt of waters extending from the coast of Great Britain up to 12 nautical miles."@en;
  skos:inScheme :conceptScheme_751925ed;
  skos:prefLabel "territorial sea"@en .

:c_a20cbb62 dct:modified "2020-10-27T07:57:16.414Z"^^xsd:dateTime;
  skos:narrower :c_781b2410 .

:c_781b2410 a skos:Concept;
  dct:created "2020-10-27T07:56:56.364Z"^^xsd:dateTime;
  dct:modified "2020-10-27T08:02:27.391Z"^^xsd:dateTime;
  skos:broader :c_a20cbb62;
  skos:inScheme :conceptScheme_751925ed;
  skos:narrower :c_e41ef2d9;
  skos:prefLabel "access to and use of buildings volume 2 – buildings other than dwellings 2015 edition for use in england*"@en .

:c_e41ef2d9 a skos:Concept;
  dct:created "2020-10-27T08:01:59.653Z"^^xsd:dateTime;
  dct:modified "2020-10-27T08:28:37.886Z"^^xsd:dateTime;
  skos:broader :c_781b2410;
  skos:definition "The following meanings apply to terms throughout this Approved Document."@en;
  skos:inScheme :conceptScheme_751925ed;
  skos:notation "1.26"@en;
  skos:prefLabel "definitions"@en .

:c_cf85f340 a skos:Concept;
  dct:modified "2020-10-28T15:20:54.369Z"^^xsd:dateTime;
  skos:broader :c_3da44764;
  skos:definition "Workplace (Health, Safety and Welfare) Regulations 1992."@en;
  skos:inScheme :conceptScheme_751925ed;
  skos:prefLabel "workplace regulations"@en .

:c_fad4ccd1 skos:prefLabel "thermal element"@en .

:c_d996e4f9 a skos:Concept;
  skos:broader :c_3da44764;
  skos:inScheme :conceptScheme_751925ed;
  skos:notation "ONR"@en;
  skos:prefLabel "office for nuclear regulation"@en .

:c_8883ce73 a skos:Concept;
  dct:modified "2020-10-28T15:21:08.210Z"^^xsd:dateTime;
  skos:broader :c_3da44764;
  skos:definition "areas outside the territorial sea designated for the exploration or exploitation of energy from water or winds (see section 84 of the Energy Act 2004)."@en;
  skos:inScheme :conceptScheme_751925ed;
  skos:prefLabel "renewable energy zone"@en .

:c_9243074f a skos:Concept;
  skos:broader :c_3da44764;
  skos:inScheme :conceptScheme_751925ed;
  skos:notation "PAS 91 "@en;
  skos:prefLabel "publicly available specification 91"@en .

:c_33cf3a6e skos:prefLabel "building"@en-GB .

:c_c53e946f a skos:Concept;
  dct:modified "2020-10-28T15:20:41.020Z"^^xsd:dateTime;
  skos:broader :c_3da44764;
  skos:definition "not necessarily those that involve the greatest risks, but those (including health risks) that are not likely to be obvious, are unusual, or likely to be difficult to manage effectively."@en;
  skos:inScheme :conceptScheme_751925ed;
  skos:prefLabel "significant risks"@en .

:c_f31dbf5c skos:prefLabel "seasonal system energy efficiency ratio"@en .

:c_8100dcd2 a skos:Concept;
  dct:created "2020-10-27T08:39:03.287Z"^^xsd:dateTime;
  dct:modified "2020-10-27T08:42:10.485Z"^^xsd:dateTime;
  skos:broader :c_2a34c0b8;
  skos:inScheme :conceptScheme_751925ed;
  skos:narrower :c_63f863a5;
  skos:prefLabel "p1 design and installation of electrical installations2013 edition – for use in england*"@en .

:c_2a34c0b8 dct:modified "2020-10-27T08:39:29.824Z"^^xsd:dateTime;
  skos:narrower :c_8100dcd2 .

:c_63f863a5 a skos:Concept;
  dct:created "2020-10-27T08:41:20.704Z"^^xsd:dateTime;
  dct:modified "2020-10-28T14:45:34.435Z"^^xsd:dateTime;
  skos:broader :c_8100dcd2;
  skos:inScheme :conceptScheme_751925ed;
  skos:narrower :c_1361b988, :c_7c734287, :c_82b1caf3, :c_835978b6, :c_9f89ffaf, :c_cca40edf;
  skos:prefLabel "appendix a: key terms (adp)"@en .

:c_cca40edf a skos:Concept;
  dct:modified "2020-10-27T08:47:18.121Z"^^xsd:dateTime;
  skos:broader :c_8100dcd2;
  skos:definition "A certificate issued by an installer registered with an authorised competent person self-certification scheme, or by a certifier registered with an authorised third-party certification scheme stating that the work described in the certificate complies with regulations 4 and 7 of the Building Regulations 2010 (that is, the work complies with all applicable requirements in the Building Regulations)"@en;
  skos:inScheme :conceptScheme_751925ed;
  skos:prefLabel "building regulations compliance certificate"@en .

:c_82b1caf3 a skos:Concept;
  dct:modified "2020-10-27T08:47:21.041Z"^^xsd:dateTime;
  skos:broader :c_8100dcd2;
  skos:definition "Fixed electric cables or fixed electrical equipment located on the consumer’s side of the electricity supply meter"@en;
  skos:inScheme :conceptScheme_751925ed;
  skos:note "NOTE: *Terms defined in regulation 2 of the Building Regulations 2010"@en;
  skos:prefLabel "electrical installation*"@en .

:c_9f89ffaf a skos:Concept;
  dct:modified "2020-10-27T08:47:26.374Z"^^xsd:dateTime;
  skos:broader :c_8100dcd2;
  skos:definition "A voltage not exceeding 50V ac or 120V ripple-free dc, whether between conductors or to earth"@en;
  skos:inScheme :conceptScheme_751925ed;
  skos:note "NOTE: *Terms defined in regulation 2 of the Building Regulations 2010"@en;
  skos:prefLabel "extra-low voltage*"@en .

:c_1361b988 a skos:Concept;
  dct:modified "2020-10-27T08:47:29.156Z"^^xsd:dateTime;
  skos:broader :c_8100dcd2;
  skos:definition "A voltage exceeding extra-low voltage but not exceeding 1000V ac or 1500V dc between conductors, or 600V ac or 900V dc between conductors and earth"@en;
  skos:inScheme :conceptScheme_751925ed;
  skos:note "NOTE: *Terms defined in regulation 2 of the Building Regulations 2010"@en;
  skos:prefLabel "low voltage*"@en .

:c_7c734287 a skos:Concept;
  dct:modified "2020-10-27T08:47:23.814Z"^^xsd:dateTime;
  skos:broader :c_8100dcd2;
  skos:definition "A competent person registered with a Part P competent person self-certification scheme"@en;
  skos:inScheme :conceptScheme_751925ed;
  skos:prefLabel "registered competent person"@en .

:c_835978b6 a skos:Concept;
  skos:broader :c_8100dcd2;
  skos:definition "A competent person registered with a Part P competent person third-party certification scheme"@en;
  skos:inScheme :conceptScheme_751925ed;
  skos:prefLabel "registered third-party certifier"@en .

:skosCollection_50d4bd2e skos:member :c_1361b988, :c_15b9d927, :c_33cf3a6e, :c_33f8635d,
    :c_4e5f287b, :c_63f863a5, :c_67243ba7, :c_6eb9d2c5, :c_7c734287, :c_7f8ff8de, :c_82b1caf3,
    :c_835978b6, :c_9f89ffaf, :c_ae0f295c, :c_c46bfd51, :c_cca40edf, :c_da4c39b1 .

:c_c66a31b4 a skos:Concept;
  dct:created "2020-10-27T16:08:22.110Z"^^xsd:dateTime;
  skos:broader :c_5ffbc967;
  skos:inScheme :conceptScheme_751925ed;
  skos:narrower :c_6eb9d2c5;
  skos:prefLabel "q1 unauthorised access 2015 edition – for use in england*"@en .

:c_5ffbc967 dct:modified "2020-10-27T16:08:50.227Z"^^xsd:dateTime;
  skos:narrower :c_c66a31b4 .

:c_6eb9d2c5 a skos:Concept;
  dct:created "2020-10-27T16:10:02.767Z"^^xsd:dateTime;
  dct:modified "2020-10-27T16:21:33.349Z"^^xsd:dateTime;
  skos:broader :c_c66a31b4;
  skos:inScheme :conceptScheme_751925ed;
  skos:narrower :c_15b9d927, :c_33f8635d, :c_67243ba7, :c_7f8ff8de, :c_ae0f295c, :c_c46bfd51;
  skos:prefLabel "appendix a: key terms (adq)"@en .

:c_c46bfd51 a skos:Concept;
  dct:modified "2020-10-27T16:20:05.217Z"^^xsd:dateTime;
  skos:broader :c_c66a31b4;
  skos:definition "A complete door assembly, assembled on site or delivered as a completed assembly, consisting of the door frame, door leaf or leaves, essential hardware and any integral side panel or fanlight (but excluding coupled assemblies)."@en;
  skos:inScheme :conceptScheme_751925ed;
  skos:prefLabel "doorset"@en .

:c_7f8ff8de a skos:Concept;
  dct:modified "2020-10-27T16:19:51.515Z"^^xsd:dateTime;
  skos:broader :c_c66a31b4;
  skos:definition "Windows, rooflights, roof windows and similar."@en;
  skos:inScheme :conceptScheme_751925ed;
  skos:prefLabel "window"@en .

:c_4e5f287b a skos:Concept;
  dct:modified "2020-10-27T16:19:56.873Z"^^xsd:dateTime;
  skos:broader :c_c66a31b4;
  skos:definition "Either: a doorset that is proven to resist physical attack by a casual or opportunist burglar, or a bespoke doorset incorporating construction features that are proven to reduce crime."@en;
  skos:inScheme :conceptScheme_751925ed;
  skos:prefLabel "secure doorset"@en .

:c_15b9d927 a skos:Concept;
  dct:modified "2020-10-27T16:20:07.951Z"^^xsd:dateTime;
  skos:broader :c_c66a31b4;
  skos:definition "Either: a window that is proven to resist criminal attack, or • a bespoke window incorporating construction features that are proven to reduce crime."@en;
  skos:inScheme :conceptScheme_751925ed;
  skos:prefLabel "secure window"@en .

:c_67243ba7 a skos:Concept;
  dct:modified "2020-10-27T16:19:59.664Z"^^xsd:dateTime;
  skos:broader :c_c66a31b4;
  skos:definition "Either: a window or doorway, any part of which is within 2m vertically of an accessible level surface  such as the ground or basement level, or an access balcony, or a window within 2m vertically of a flat or sloping roof (with a pitch of less than 30°) that is within 3.5m of ground level."@en;
  skos:inScheme :conceptScheme_751925ed;
  skos:prefLabel "easily accessible"@en .

:c_33f8635d a skos:Concept;
  dct:modified "2020-10-27T16:20:02.506Z"^^xsd:dateTime;
  skos:broader :c_c66a31b4;
  skos:definition "A doorset and window that are supplied as separate self-contained frames and fixed together on site."@en;
  skos:inScheme :conceptScheme_751925ed;
  skos:prefLabel "coupled assembly"@en .

:c_ae0f295c a skos:Concept;
  dct:modified "2020-10-27T16:19:54.140Z"^^xsd:dateTime;
  skos:broader :c_c66a31b4;
  skos:definition "(In the context of secure doorsets and secure windows) – a product designed and constructed in accordance with a specification or design shown by test to be capable of meeting the required performance. Further information on materials and workmanship is given in Approved Document 7."@en;
  skos:inScheme :conceptScheme_751925ed;
  skos:note "NOTE 1: Laboratories accredited by the United Kingdom Accreditation Service (UKAS) or an equivalent European national accreditation body should have the necessary expertise to conduct the relevant tests NOTE 2: Any test evidence used to confirm the security of a construction should be carefully checked to ensure that it demonstrates compliance that is adequate and that applies to the intended use. Evidence passed from one organisation to another can become unreliable if important details are lost. Small differences in construction can significantly affect the performance of a doorset or window. NOTE 3: Schemes that certify compliance with PAS 24:2012 or other standards that offer similar or better performance may be acceptable for demonstrating compliance. A list of UKAS-accredited certification bodies is given on the UKAS website. Many recognised schemes are also listed in Secured by Design’s New Homes 2014, Section 2."@en;
  skos:prefLabel "proven"@en .

:c_502a871c dct:modified "2020-10-27T16:36:44.176Z"^^xsd:dateTime;
  skos:narrower :c_0109c085 .

:c_a9fc7032 a skos:Concept;
  dct:created "2020-10-27T16:38:04.682Z"^^xsd:dateTime;
  skos:broader :c_0109c085;
  skos:inScheme :conceptScheme_751925ed;
  skos:prefLabel "appendix i key terms"@en .

:c_63242aeb a skos:Concept;
  dct:created "2020-10-27T16:22:40.546Z"^^xsd:dateTime;
  dct:modified "2020-10-27T16:25:51.039Z"^^xsd:dateTime;
  skos:broader :c_b7bccf3d;
  skos:inScheme :conceptScheme_751925ed;
  skos:narrower :c_0e4cfb77;
  skos:prefLabel "r1 In-building physical infrastructure 2016 edition – for use in england*"@en .

:c_b7bccf3d dct:modified "2020-10-27T16:23:06.700Z"^^xsd:dateTime;
  skos:narrower :c_63242aeb .

:c_0e4cfb77 a skos:Concept;
  dct:created "2020-10-27T16:25:11.673Z"^^xsd:dateTime;
  dct:modified "2020-10-27T16:27:35.347Z"^^xsd:dateTime;
  skos:broader :c_63242aeb;
  skos:definition "The following are key terms used in this document and defined in regulation 44C of the Building Regulations 2010 (as amended):"@en;
  skos:inScheme :conceptScheme_751925ed;
  skos:prefLabel "appendix a: key terms (adr)"@en .

:c_67b341f4 a skos:Concept;
  dct:modified "2020-10-27T16:31:48.821Z"^^xsd:dateTime;
  skos:broader :c_0e4cfb77;
  skos:definition "A physical point, located inside or outside the building, accessible to undertakings providing or authorised to provide public communications networks, where connection to the high-speed- ready in-building physical infrastructure is made available."@en;
  skos:inScheme :conceptScheme_751925ed;
  skos:prefLabel "access point"@en .

:c_26e1919c a skos:Concept;
  dct:modified "2020-10-27T16:31:52.607Z"^^xsd:dateTime;
  skos:broader :c_0e4cfb77;
  skos:definition "An electronic communications network which is capable of delivering broadband access services at speeds of at least 30 Mbps."@en;
  skos:inScheme :conceptScheme_751925ed;
  skos:prefLabel "high-speed electronic communications network"@en .

:c_5e7bed84 a skos:Concept;
  dct:modified "2020-10-27T16:31:45.812Z"^^xsd:dateTime;
  skos:broader :c_0e4cfb77;
  skos:definition "In-building physical infrastructure intended to host elements, or enable delivery, of high-speed electronic communications networks."@en;
  skos:inScheme :conceptScheme_751925ed;
  skos:prefLabel "high-speed-ready in-building physical infrastructure"@en .

:c_99119e22 a skos:Concept;
  dct:modified "2020-10-27T16:31:58.708Z"^^xsd:dateTime;
  skos:broader :c_0e4cfb77;
  skos:definition "Physical infrastructure or installations at the end- user’s location, including elements under joint ownership, intended to host wired or wireless access networks, where such access networks are capable of delivering electronic communications services and connecting the building access point with the network termination point."@en;
  skos:inScheme :conceptScheme_751925ed;
  skos:prefLabel "in-building physical infrastructure"@en .

:c_af28f591 a skos:Concept;
  dct:modified "2020-10-27T16:31:55.572Z"^^xsd:dateTime;
  skos:broader :c_0e4cfb77;
  skos:definition "Works at the end-user’s location encompassing structural modifications of the entire in-building physical infrastructure, or of a significant part of it."@en;
  skos:inScheme :conceptScheme_751925ed;
  skos:prefLabel "major renovation works"@en .

:c_2a5aa469 a skos:Concept;
  skos:broader :c_0e4cfb77;
  skos:definition "A physical point at which an occupier is provided with access to high-speed electronic communications networks."@en;
  skos:inScheme :conceptScheme_751925ed;
  skos:note "NOTE: The ‘occupier’ is the subscriber to the broadband service. The termination point is typically inside the building, but may be outside the building for wireless connections."@en;
  skos:prefLabel "network termination point"@en .

:skosCollection_50d4bd2e skos:member :c_26e1919c, :c_2a5aa469, :c_5e7bed84, :c_67b341f4,
    :c_99119e22, :c_af28f591 .

:c_0109c085 a skos:Concept;
  dct:modified "2020-10-27T16:38:34.982Z"^^xsd:dateTime;
  skos:narrower :c_a9fc7032;
  skos:prefLabel "manual to the building regulations"@en .

:c_d4970b41 a skos:Concept;
  skos:broader :c_a9fc7032;
  skos:definition "followed by a number refers to a regulation in the Building Regulations 2010."@en;
  skos:note "Terms relating to the structure of legislation:"@en;
  skos:prefLabel "regulation"@en .

:c_89c887d6 a skos:Concept;
  skos:broader :c_a9fc7032;
  skos:definition "refers to a schedule contained in the Building Regulations 2010, for example Schedule 1 to the Building Regulations."@en;
  skos:note "Terms relating to the structure of legislation:"@en;
  skos:prefLabel "schedule"@en .

:c_325fa285 a skos:Concept;
  skos:broader :c_a9fc7032;
  skos:definition "refers to a section of the Building Act 1984."@en;
  skos:note "Terms relating to the structure of legislation:"@en;
  skos:prefLabel "section"@en .

:c_345c095e a skos:Concept;
  skos:broader :c_a9fc7032;
  skos:definition "refers to a change of the scope of an initial notice. For further information see Chapter E."@en;
  skos:prefLabel "amendment notice"@en .

:c_66d06a87 a skos:Concept;
  skos:broader :c_a9fc7032;
  skos:definition "refers to a document approved by government that provides practical guidance on how the Building Regulations can be satisfied in some common situations. Approved documents are given legal status by the Building Act 1984."@en;
  skos:prefLabel "approved document"@en .

:c_9e9fac9d a skos:Concept;
  skos:broader :c_a9fc7032;
  skos:definition "are companies or individuals authorised under the Building Act 1984 to carry out building control work in England and Wales. They must be registered with the Construction Industry Council Approved Inspectors Register (CICAIR), which provides a list of approved inspectors. https://www.cicair.org.uk/approved-inspectors-register/"@en;
  skos:prefLabel "approved inspectors"@en .

:c_4aee7770 a skos:Concept;
  skos:broader :c_a9fc7032;
  skos:definition "refers to the Building (Approved Inspectors etc.) Regulations 2010."@en;
  skos:prefLabel "approved inspectors regulations"@en .

:c_33cf3a6e a skos:Concept;
  dct:modified "2020-10-28T15:16:40.282Z"^^xsd:dateTime;
  skos:broader :c_a9fc7032;
  skos:definition "is generally any permanent or temporary building. A reference to a building includes a reference to part of a building. Buildings include dwellings (houses, flats) and public buildings."@en;
  skos:inScheme :conceptScheme_751925ed .

:c_77212558 a skos:Concept;
  skos:broader :c_a9fc7032;
  skos:definition "refers to the Building Act 1984."@en;
  skos:inScheme :conceptScheme_751925ed;
  skos:prefLabel "building act"@en .

:c_0775280b a skos:Concept;
  skos:broader :c_a9fc7032;
  skos:definition "is a local authority building control department or an approved inspector."@en;
  skos:inScheme :conceptScheme_751925ed;
  skos:prefLabel "building control body"@en .

:c_616fbf78 a skos:Concept;
  skos:broader :c_a9fc7032;
  skos:definition "is a route to Building Regulations approval using local authority building control. Refer to Chapter D for details."@en;
  skos:inScheme :conceptScheme_751925ed;
  skos:prefLabel "building notice"@en .

:c_d4486d47 a skos:Concept;
  skos:broader :c_a9fc7032;
  skos:definition "refers to the Building Regulations 2010."@en;
  skos:inScheme :conceptScheme_751925ed;
  skos:prefLabel "building regulations"@en .

:c_a00c11cf a skos:Concept;
  skos:broader :c_a9fc7032;
  skos:definition "includes erecting or extending a building, providing or extending a controlled service or fitting in or in connection with a building, and the material alteration of a building or a controlled service or fitting."@en;
  skos:inScheme :conceptScheme_751925ed;
  skos:prefLabel "building work"@en .

:c_22a21142 a skos:Concept;
  skos:broader :c_a9fc7032;
  skos:definition "under the Construction Products Regulation (305/2011/EU-CPR). The Construction Products Regulation requires that construction products on the EU market covered by a harmonised European product standard normally have a CE marking. Refer to Chapter F for details."@en;
  skos:inScheme :conceptScheme_751925ed;
  skos:prefLabel "ce marking"@en .

:c_0f6ef18a a skos:Concept;
  skos:broader :c_a9fc7032;
  skos:definition "allow tradespeople to demonstrate their ability to carry out certain work to required standards instead of the work going through a building control body approval process. Refer to Chapter 5 and Chapter C."@en;
  skos:inScheme :conceptScheme_751925ed;
  skos:prefLabel "competent person schemes"@en .

:c_e8d281dd a skos:Concept;
  skos:broader :c_a9fc7032;
  skos:definition "are issued by the local authority to confirm that it has taken reasonable steps to ensure that there is evidence, but not necessarily conclusive evidence, that the work complies with the relevant requirements of the Building Regulations."@en;
  skos:inScheme :conceptScheme_751925ed;
  skos:prefLabel "completion certificates"@en .

:c_6b4d8aa6 a skos:Concept;
  skos:broader :c_a9fc7032;
  skos:definition "include a service or fitting subject to Schedule 1 (to the Building Regulations) requirements in respect of sanitation, hot water safety, water efficiency, drainage and waste disposal, combustion appliances and fuel storage, conservation of fuel or power, and electrical safety."@en;
  skos:inScheme :conceptScheme_751925ed;
  skos:prefLabel "controlled services or fittings"@en .

:c_24fd49d7 a skos:Concept;
  skos:broader :c_a9fc7032;
  skos:definition "refers to the certificate issued by the approved inspector to the person carrying out the work and the local authority and confirms that the work in the initial notice is complete and that the approved inspector is satisfied that it complies with the relevant requirements of the Building Regulations."@en;
  skos:inScheme :conceptScheme_751925ed;
  skos:prefLabel "final certificate"@en .

:c_43607495 a skos:Concept;
  skos:broader :c_a9fc7032;
  skos:definition "refers to the route to Building Regulations approval using local authority building control. Refer to Chapter D for details."@en;
  skos:inScheme :conceptScheme_751925ed;
  skos:prefLabel "full plans"@en .

:c_7a693319 a skos:Concept;
  skos:broader :c_a9fc7032;
  skos:definition "refers to the notice served on the local authority jointly by the client and the approved inspector when an approved inspector is selected as the building control body."@en;
  skos:inScheme :conceptScheme_751925ed;
  skos:prefLabel "initial notice"@en .

:c_ab86b8aa a skos:Concept;
  skos:broader :c_a9fc7032;
  skos:definition "operates in addition to normal planning controls under the  Planning (Listed Buildings and Conservation Areas) Act 1990. Listed building consent is likely to be required for any alteration to a listed building."@en;
  skos:inScheme :conceptScheme_751925ed;
  skos:prefLabel "listed building consent"@en .

:c_3f20a780 a skos:Concept;
  skos:broader :c_a9fc7032;
  skos:definition "is the building control department of the local authority."@en;
  skos:inScheme :conceptScheme_751925ed;
  skos:prefLabel "local authority building control"@en .

:c_8eaab627 a skos:Concept;
  skos:broader :c_a9fc7032;
  skos:definition "is defined in Approved Document L1B, 5.6A and L2B, 3.1."@en;
  skos:inScheme :conceptScheme_751925ed;
  skos:prefLabel "major renovation"@en .

:c_58d3c1e1 a skos:Concept;
  skos:broader :c_a9fc7032;
  skos:definition "is defined under Regulation 3 of the Building Regulations. An alteration is a material alteration if the proposed building work would make a building less safe structurally, more at risk from fire or less accessible for disabled people."@en;
  skos:inScheme :conceptScheme_751925ed;
  skos:prefLabel "material alteration"@en .

:c_fd257378 a skos:Concept;
  skos:broader :c_a9fc7032;
  skos:definition "include: manufactured products, such as components, fittings, items of equipment and systems; naturally occurring materials, such as stone, timber and thatch; and    backfilling for excavations in connection with building work."@en;
  skos:inScheme :conceptScheme_751925ed;
  skos:prefLabel "materials"@en .

:c_2da98c6b a skos:Concept;
  skos:broader :c_a9fc7032;
  skos:definition "is approval to carry out building work from a town and country planning point of view. It is typically required to construct or extend a building or change the use of a building. The local planning authority decides whether a project will need planning permission."@en;
  skos:inScheme :conceptScheme_751925ed;
  skos:prefLabel "planning permission"@en .

:c_6c87e49d a skos:Concept;
  skos:broader :c_a9fc7032;
  skos:definition "can be used to demonstrate that detailed plans of the work or a part of it comply with the Building Regulations. They are described in Regulations 14 and 15 of the Approved Inspectors Regulations and Section 50 of the Building Act."@en;
  skos:inScheme :conceptScheme_751925ed;
  skos:prefLabel "plans certificates"@en .

:c_c463b9ee a skos:Concept;
  skos:broader :c_a9fc7032;
  skos:definition "can be issued by local authorities retrospectively to indicate that work started after 11 November 1985 which has been completed complies with the Building Regulations which applied at the time the works were done."@en;
  skos:inScheme :conceptScheme_751925ed;
  skos:prefLabel "regularisation certificates"@en .

:c_646e9bae a skos:Concept;
  skos:broader :c_a9fc7032;
  skos:definition "(in relation to a thermal element) is defined in Approved Document L1B, 5.6A and L2B, 3.1."@en;
  skos:inScheme :conceptScheme_751925ed;
  skos:prefLabel "renovation"@en .

:c_a9823a22 a skos:Concept;
  dct:modified "2020-10-28T15:21:20.969Z"^^xsd:dateTime;
  skos:broader :c_a9fc7032;
  skos:definition "is the person defined in article 3 of the Regulatory Reform (Fire Safety) Order 2005 and having the duties for compliance with the Order as prescribed in article 5."@en;
  skos:inScheme :conceptScheme_751925ed .

:c_fad4ccd1 a skos:Concept;
  dct:modified "2020-10-28T15:22:02.306Z"^^xsd:dateTime;
  skos:broader :c_a9fc7032;
  skos:definition "is a material that contributes to the thermal performance of a building’s thermal envelope, such as any element of a wall, floor or roof but not a door or window. Thermal element is defined in Regulation 2(3) of the Building Regulations."@en;
  skos:inScheme :conceptScheme_751925ed .

:c_d4970b41 skos:inScheme :conceptScheme_751925ed .

:c_89c887d6 skos:inScheme :conceptScheme_751925ed .

:c_325fa285 skos:inScheme :conceptScheme_751925ed .

:c_345c095e skos:inScheme :conceptScheme_751925ed .

:c_66d06a87 skos:inScheme :conceptScheme_751925ed .

:c_9e9fac9d skos:inScheme :conceptScheme_751925ed .

:c_4aee7770 skos:inScheme :conceptScheme_751925ed .

:c_a9fc7032 dct:modified "2020-10-27T16:54:37.631Z"^^xsd:dateTime;
  skos:narrower :c_0775280b, :c_0f6ef18a, :c_1b060096, :c_22a21142, :c_24fd49d7, :c_2da98c6b,
    :c_325fa285, :c_33cf3a6e, :c_345c095e, :c_3f20a780, :c_43607495, :c_4aee7770, :c_58d3c1e1,
    :c_616fbf78, :c_646e9bae, :c_66d06a87, :c_6b4d8aa6, :c_6c87e49d, :c_77212558, :c_7a693319,
    :c_89c887d6, :c_8eaab627, :c_9e9fac9d, :c_a00c11cf, :c_a9823a22, :c_ab86b8aa, :c_c463b9ee,
    :c_d4486d47, :c_d4970b41, :c_e8d281dd, :c_fad4ccd1, :c_fd257378 .

:skosCollection_50d4bd2e skos:member :c_0775280b, :c_0f6ef18a, :c_22a21142, :c_24fd49d7,
    :c_2da98c6b, :c_325fa285, :c_345c095e, :c_3f20a780, :c_43607495, :c_58d3c1e1, :c_616fbf78,
    :c_646e9bae, :c_66d06a87, :c_6b4d8aa6, :c_6c87e49d, :c_77212558, :c_7a693319, :c_89c887d6,
    :c_8eaab627, :c_9e9fac9d, :c_a00c11cf, :c_a9823a22, :c_ab86b8aa, :c_c463b9ee, :c_d4486d47,
    :c_d4970b41, :c_e8d281dd, :c_fad4ccd1, :c_fd257378 .

:c_37246cae dct:modified "2020-10-27T17:03:26.447Z"^^xsd:dateTime;
  skos:broader :c_502a871c;
  skos:narrower :c_3da44764 .

:c_3da44764 a skos:Concept;
  dct:created "2020-10-27T17:03:12.864Z"^^xsd:dateTime;
  skos:broader :c_37246cae;
  skos:inScheme :conceptScheme_751925ed;
  skos:narrower :c_4775ba65, :c_547611a3, :c_c92ba3dc, :c_c984b189, :c_fe309bb8;
  skos:prefLabel "glossary of acronyms and terms"@en .

:c_fe309bb8 a skos:Concept;
  skos:broader :c_3da44764;
  skos:inScheme :conceptScheme_751925ed;
  skos:notation "ACOP"@en;
  skos:prefLabel "approved code of practice"@en .

:c_6e741d9b a skos:Concept;
  skos:broader :c_3da44764;
  skos:inScheme :conceptScheme_751925ed;
  skos:notation "AOGBO 2013 "@en;
  skos:prefLabel "application to areas outside great britain order 2013"@en .

:c_547611a3 a skos:Concept;
  skos:broader :c_3da44764;
  skos:inScheme :conceptScheme_751925ed;
  skos:notation "CDM 2007 "@en;
  skos:prefLabel "construction (design and management) regulations 2007"@en .

:c_c92ba3dc a skos:Concept;
  dct:modified "2020-10-28T15:17:58.161Z"^^xsd:dateTime;
  skos:broader :c_3da44764;
  skos:inScheme :conceptScheme_751925ed;
  skos:notation "CDM 2015 "@en;
  skos:prefLabel "construction (design and management) regulations 2015"@en-GB .

:c_4775ba65 a skos:Concept;
  skos:broader :c_3da44764;
  skos:inScheme :conceptScheme_751925ed;
  skos:notation "CITB"@en;
  skos:prefLabel "construction industry training board"@en .

:c_0af8118b a skos:Concept;
  skos:broader :c_3da44764;
  skos:inScheme :conceptScheme_751925ed;
  skos:notation "HSE"@en;
  skos:prefLabel "health and safety executive"@en .

:c_c984b189 a skos:Concept;
  skos:broader :c_3da44764;
  skos:inScheme :conceptScheme_751925ed;
  skos:notation "HSWA"@en;
  skos:prefLabel "health and safety at work etc act 1974"@en .

:c_58bdb729 a skos:Concept;
  skos:broader :c_3da44764 .
